@prefix dct: <http://purl.org/dc/terms/> .
@prefix dpv: <https://w3id.org/dpv#> .
@prefix owl: <http://www.w3.org/2002/07/owl#> .
@prefix rdfs: <http://www.w3.org/2000/01/rdf-schema#> .
@prefix risk: <https://w3id.org/dpv/risk#> .
@prefix skos: <http://www.w3.org/2004/02/skos/core#> .
@prefix sw: <http://www.w3.org/2003/06/sw-vocab-status/ns#> .
@prefix vann: <http://purl.org/vocab/vann/> .
@prefix xsd: <http://www.w3.org/2001/XMLSchema#> .

<https://w3id.org/dpv/risk> a owl:Ontology ;
    dct:abstract "Risk Extension for DPV"@en ;
    dct:contributor "Beatriz Esteves",
        "Georg P Krog",
        "Harshvardhan J. Pandit",
        "Julian Flake",
        "Paul Ryan" ;
    dct:created "2022-08-14"^^xsd:date ;
    dct:creator "Harshvardhan J. Pandit" ;
    dct:description "The Risk extension to Data Privacy Vocabulary provides terms (classes and properties) related to risk management, assessment, and consequences."@en ;
    dct:license <https://www.w3.org/Consortium/Legal/2015/doc-license> ;
    dct:modified "2022-08-14"^^xsd:date ;
    dct:source <https://www.w3.org/community/dpvcg/> ;
    dct:title "Risk Extension for DPV"@en ;
    vann:preferredNamespacePrefix "risk" ;
    vann:preferredNamespaceUri "https://w3id.org/dpv/risk#"^^xsd:string ;
    owl:versionInfo "0.8"^^xsd:string .

risk:ConsequencesConcepts a skos:Collection ;
    skos:member risk:AttackonPrivateLife,
        risk:Blackmail,
        risk:BusinessPerformanceImpairment,
        risk:Businessdisruption,
        risk:ConfidentialityBreach,
        risk:CorruptionData,
        risk:CostAcquisition,
        risk:CostBackup,
        risk:CostConfiguration,
        risk:CostInstallation,
        risk:CostJudicialPenalties,
        risk:CostJudicialProceedings,
        risk:CostOperationInterruption,
        risk:CostSuspendedOperations,
        risk:CyberSpying,
        risk:CyberStalking,
        risk:DangertoCustomers,
        risk:DangertoPersonnel,
        risk:DataBreach,
        risk:DenialServiceAttack,
        risk:DistributedDenialServiceAttack,
        risk:Eavesdropping,
        risk:EnvironmentalSafetyEndangerment,
        risk:EquipmentFailure,
        risk:EquipmentMalfunction,
        risk:ErrornousUse,
        risk:FinancialEquipmentCosts,
        risk:FinancialInvestigationCosts,
        risk:FinancialLoss,
        risk:FinancialPersonnelCosts,
        risk:FinancialRepairCosts,
        risk:Fraud,
        risk:GovernmentCrisis,
        risk:IllegalProcessingData,
        risk:ImpacttoRights,
        risk:IncreaseInternalCost,
        risk:IndustrialCrisis,
        risk:Injury,
        risk:InterceptionCommunications,
        risk:InternalOperationDisruption,
        risk:LawEnforcementAdverseEffects,
        risk:LossAssets,
        risk:LossCompetitiveAdvantage,
        risk:LossCredibility,
        risk:LossCustomerConfidence,
        risk:LossCustomers,
        risk:LossFunds,
        risk:LossGoods,
        risk:LossGoodwill,
        risk:LossNegotiatingCapacity,
        risk:LossOpportunity,
        risk:LossProprietaryInformation,
        risk:LossReputation,
        risk:LossSuppliers,
        risk:LossTechnologicalAdvantage,
        risk:LossTrust,
        risk:MisuseBreachedInformation,
        risk:OrganisationDisruption,
        risk:PersonalSafetyEndangerment,
        risk:PhysicalAssault,
        risk:PhysicalSpying,
        risk:PhysicalStalking,
        risk:PsychologicalHarm,
        risk:PublicOrderBreach,
        risk:RansomDemand,
        risk:RemoteSpying,
        risk:ReplacementCosts,
        risk:RetrievalDeletedData,
        risk:RetrievalDiscardedEquipment,
        risk:Scam,
        risk:SecurityBreach,
        risk:ServiceInterruption,
        risk:SoftwareMalfunction,
        risk:Spoofing,
        risk:Spying,
        risk:Stalking,
        risk:Terrorism,
        risk:Theft,
        risk:TheftEquipment,
        risk:TheftMedia,
        risk:ThirdPartyOperationDisruption,
        risk:UnauthorisedAccesstoPremises,
        risk:UnauthorisedDisclosureData,
        risk:UnauthorisedImpersonation,
        risk:UnauthorisedSystemAccess,
        risk:UnauthorisedUseEquipment,
        risk:UnwantedDeletionData,
        risk:UnwantedDisclosureData,
        risk:ViolationCodeConduct,
        risk:ViolationContractualObligations,
        risk:ViolationEthicalCode,
        risk:ViolationRegulatoryObligations,
        risk:ViolationStatutoryObligations,
        risk:VulnerabilityCreated ;
    skos:prefLabel "Consequences Concepts"^^xsd:string .

risk:Risk_AssessmentConcepts a skos:Collection ;
    skos:member risk:ALARA,
        risk:ALARP,
        risk:BayesianAnalysis,
        risk:BayesianNetworks,
        risk:BowTie,
        risk:Brainstorming,
        risk:BusinessImpactAnalysis,
        risk:CVaR,
        risk:CausalMapping,
        risk:CauseConsequenceAnalysis,
        risk:Checklists,
        risk:Cindynic,
        risk:Classifications,
        risk:CostBenefitAnalysis,
        risk:CrossImpactAnalysis,
        risk:DPIA,
        risk:DecisionTreeAnalysis,
        risk:DelphiTechnique,
        risk:EventTreeAnalysis,
        risk:FMEA,
        risk:FMECA,
        risk:FNDiagrams,
        risk:FaultTreeAnalysis,
        risk:Fishbone,
        risk:GameTheory,
        risk:HACCP,
        risk:HAZOP,
        risk:HumanReliabilityAnalysis,
        risk:InfluenceDiagrams,
        risk:Interviews,
        risk:LOPA,
        risk:MCA,
        risk:MarkovAnalysis,
        risk:MonteCarloSimulation,
        risk:NominalGroupTechnique,
        risk:PIA,
        risk:ParetoCharts,
        risk:QualitativeRiskAssessmentTechnique,
        risk:QuantitativeRiskAssessmentTechnique,
        risk:ReliabilityCentredMaintenance,
        risk:RiskAssessmentTechnique,
        risk:RiskIndices,
        risk:RiskMatrix,
        risk:RiskRegisters,
        risk:SCurves,
        risk:SFAIRP,
        risk:SWIFT,
        risk:ScenarioAnalysis,
        risk:Surveys,
        risk:Taxonomies,
        risk:Toxicological,
        risk:VaR ;
    skos:prefLabel "Risk_Assessment Concepts"^^xsd:string .

risk:Risk_ControlsConcepts a skos:Collection ;
    skos:member risk:AvoidSource,
        risk:ChangeConsequence,
        risk:ChangeImpact,
        risk:ControlConsequence,
        risk:ControlMonitors,
        risk:ControlRiskSource,
        risk:HaltSource,
        risk:MonitorConsequence,
        risk:MonitorImpact,
        risk:MonitorRisk,
        risk:MonitorRiskControl,
        risk:MonitorRiskSource,
        risk:MonitorVulnerabilities,
        risk:ReduceLikelihood,
        risk:ReduceSeverity,
        risk:RemoveConsequence,
        risk:RemoveImpact,
        risk:RemoveSource,
        risk:ShareRisk ;
    skos:prefLabel "Risk_Controls Concepts"^^xsd:string .

risk:Risk_LevelsConcepts a skos:Collection ;
    skos:member risk:3LikelihoodLevels,
        risk:3RiskLevels,
        risk:3SeverityLevels,
        risk:5LikelihoodLevels,
        risk:5RiskLevels,
        risk:5SeverityLevels,
        risk:7LikelihoodLevels,
        risk:7RiskLevels,
        risk:7SeverityLevels,
        risk:ExtremelyHighLikelihood,
        risk:ExtremelyHighRisk,
        risk:ExtremelyHighSeverity,
        risk:ExtremelyLowLikelihood,
        risk:ExtremelyLowRisk,
        risk:ExtremelyLowSeverity,
        risk:HighLikelihood,
        risk:HighRisk,
        risk:HighSeverity,
        risk:LowLikelihood,
        risk:LowRisk,
        risk:LowSeverity,
        risk:ModerateLikelihood,
        risk:ModerateRisk,
        risk:ModerateSeverity,
        risk:VeryHighLikelihood,
        risk:VeryHighRisk,
        risk:VeryHighSeverity,
        risk:VeryLowLikelihood,
        risk:VeryLowRisk,
        risk:VeryLowSeverity ;
    skos:prefLabel "Risk_Levels Concepts"^^xsd:string .

risk:Risk_MatrixConcepts a skos:Collection ;
    skos:member risk:RM3x3,
        risk:RM3x3R1C1,
        risk:RM3x3R1C2,
        risk:RM3x3R1C3,
        risk:RM3x3R2C1,
        risk:RM3x3R2C2,
        risk:RM3x3R2C3,
        risk:RM3x3R3C1,
        risk:RM3x3R3C2,
        risk:RM3x3R3C3,
        risk:RM5x5,
        risk:RM5x5R1C1,
        risk:RM5x5R1C2,
        risk:RM5x5R1C3,
        risk:RM5x5R1C4,
        risk:RM5x5R1C5,
        risk:RM5x5R2C1,
        risk:RM5x5R2C2,
        risk:RM5x5R2C3,
        risk:RM5x5R2C4,
        risk:RM5x5R2C5,
        risk:RM5x5R3C1,
        risk:RM5x5R3C2,
        risk:RM5x5R3C3,
        risk:RM5x5R3C4,
        risk:RM5x5R3C5,
        risk:RM5x5R4C1,
        risk:RM5x5R4C2,
        risk:RM5x5R4C3,
        risk:RM5x5R4C4,
        risk:RM5x5R4C5,
        risk:RM5x5R5C1,
        risk:RM5x5R5C2,
        risk:RM5x5R5C3,
        risk:RM5x5R5C4,
        risk:RM5x5R5C5,
        risk:RM7x7,
        risk:RM7x7R1C1,
        risk:RM7x7R1C2,
        risk:RM7x7R1C3,
        risk:RM7x7R1C4,
        risk:RM7x7R1C5,
        risk:RM7x7R1C6,
        risk:RM7x7R1C7,
        risk:RM7x7R2C1,
        risk:RM7x7R2C2,
        risk:RM7x7R2C3,
        risk:RM7x7R2C4,
        risk:RM7x7R2C5,
        risk:RM7x7R2C6,
        risk:RM7x7R2C7,
        risk:RM7x7R3C1,
        risk:RM7x7R3C2,
        risk:RM7x7R3C3,
        risk:RM7x7R3C4,
        risk:RM7x7R3C5,
        risk:RM7x7R3C6,
        risk:RM7x7R3C7,
        risk:RM7x7R4C1,
        risk:RM7x7R4C2,
        risk:RM7x7R4C3,
        risk:RM7x7R4C4,
        risk:RM7x7R4C5,
        risk:RM7x7R4C6,
        risk:RM7x7R4C7,
        risk:RM7x7R5C1,
        risk:RM7x7R5C2,
        risk:RM7x7R5C3,
        risk:RM7x7R5C4,
        risk:RM7x7R5C5,
        risk:RM7x7R5C6,
        risk:RM7x7R5C7,
        risk:RM7x7R6C1,
        risk:RM7x7R6C2,
        risk:RM7x7R6C3,
        risk:RM7x7R6C4,
        risk:RM7x7R6C5,
        risk:RM7x7R6C6,
        risk:RM7x7R6C7,
        risk:RM7x7R7C1,
        risk:RM7x7R7C2,
        risk:RM7x7R7C3,
        risk:RM7x7R7C4,
        risk:RM7x7R7C5,
        risk:RM7x7R7C6,
        risk:RM7x7R7C7 ;
    skos:prefLabel "Risk_Matrix Concepts"^^xsd:string .

risk:ALARA a skos:Concept,
        dpv:Concept ;
    dct:created ""^^xsd:date ;
    dct:source <https://www.iso.org/standard/72140.html> ;
    rdfs:isDefinedBy risk: ;
    sw:term_status "accepted"@en ;
    skos:definition "As Low as Resonably Achievable (ALARP) - A criteria for deciding significance of risk and means of evaluating tolerability of risk"@en ;
    skos:inScheme risk: ;
    skos:prefLabel "ALARA"@en ;
    dpv:isInstanceOf risk:QualitativeRiskAssessmentTechnique,
        risk:QuantitativeRiskAssessmentTechnique .

risk:ALARP a skos:Concept,
        dpv:Concept ;
    dct:created ""^^xsd:date ;
    dct:source <https://www.iso.org/standard/72140.html> ;
    rdfs:isDefinedBy risk: ;
    sw:term_status "accepted"@en ;
    skos:definition "As Low as Resonably Possible (ALARP) - A criteria for deciding significance of risk and means of evaluating tolerability of risk"@en ;
    skos:inScheme risk: ;
    skos:prefLabel "ALARP"@en ;
    dpv:isInstanceOf risk:QualitativeRiskAssessmentTechnique,
        risk:QuantitativeRiskAssessmentTechnique .

risk:AttackonPrivateLife a skos:Concept,
        dpv:Concept ;
    dct:created ""^^xsd:date ;
    dct:source <https://www.iso.org/standard/75281.html> ;
    rdfs:isDefinedBy risk: ;
    sw:term_status "accepted"@en ;
    skos:definition ""@en ;
    skos:inScheme risk: ;
    skos:prefLabel "Attack on Private Life"@en ;
    dpv:isSubTypeOf dpv:Harm .

risk:AvoidSource a skos:Concept,
        dpv:Concept ;
    dct:created ""^^xsd:date ;
    rdfs:isDefinedBy risk: ;
    sw:term_status "accepted"@en ;
    skos:definition "Risk Control that avoids the risk source"@en ;
    skos:inScheme risk: ;
    skos:prefLabel "Avoid Source"@en ;
    dpv:isSubTypeOf risk:ControlRiskSource .

risk:BayesianAnalysis a skos:Concept,
        dpv:Concept ;
    dct:created ""^^xsd:date ;
    dct:source <https://www.iso.org/standard/72140.html> ;
    rdfs:isDefinedBy risk: ;
    sw:term_status "accepted"@en ;
    skos:definition "A means of making inference about model parameters using Bayes' theorem which has the capability of incorporating empirical data into prior judgements about probabilities"@en ;
    skos:inScheme risk: ;
    skos:prefLabel "Bayesian Analysis"@en ;
    dpv:isInstanceOf risk:QuantitativeRiskAssessmentTechnique .

risk:BayesianNetworks a skos:Concept,
        dpv:Concept ;
    dct:created ""^^xsd:date ;
    dct:source <https://www.iso.org/standard/72140.html> ;
    rdfs:isDefinedBy risk: ;
    sw:term_status "accepted"@en ;
    skos:definition "A graphical model of variables and their cause-effect relationships expressed using probabilities"@en ;
    skos:inScheme risk: ;
    skos:prefLabel "Bayesian Networks"@en ;
    dpv:isInstanceOf risk:QuantitativeRiskAssessmentTechnique .

risk:Blackmail a skos:Concept,
        dpv:Concept ;
    dct:created ""^^xsd:date ;
    dct:source <https://www.iso.org/standard/75281.html> ;
    rdfs:isDefinedBy risk: ;
    sw:term_status "accepted"@en ;
    skos:definition ""@en ;
    skos:inScheme risk: ;
    skos:prefLabel "Blackmail"@en ;
    dpv:isSubTypeOf dpv:Harm .

risk:BowTie a skos:Concept,
        dpv:Concept ;
    dct:created ""^^xsd:date ;
    dct:source <https://www.iso.org/standard/72140.html> ;
    rdfs:isDefinedBy risk: ;
    sw:term_status "accepted"@en ;
    skos:definition "A diagrammatic way of describing the pathways from sources of risk to outcomes, and of reviewing controls"@en ;
    skos:inScheme risk: ;
    skos:prefLabel "Bow Tie Analysis"@en ;
    dpv:isInstanceOf risk:QualitativeRiskAssessmentTechnique,
        risk:QuantitativeRiskAssessmentTechnique .

risk:Brainstorming a skos:Concept,
        dpv:Concept ;
    dct:created ""^^xsd:date ;
    dct:source <https://www.iso.org/standard/72140.html> ;
    rdfs:isDefinedBy risk: ;
    sw:term_status "accepted"@en ;
    skos:definition "Technique used in workshops to encourage imaginative thinking"@en ;
    skos:inScheme risk: ;
    skos:prefLabel "Brainstorming"@en ;
    dpv:isInstanceOf risk:QualitativeRiskAssessmentTechnique .

risk:BusinessImpactAnalysis a skos:Concept,
        dpv:Concept ;
    dct:created ""^^xsd:date ;
    dct:source <https://www.iso.org/standard/72140.html> ;
    rdfs:isDefinedBy risk: ;
    sw:term_status "accepted"@en ;
    skos:definition "A process that analyses the consequences of a disruptive incident on the organization which determines the recovery priorities of an organization's products and services and, thereby, the priorities of the activities and resources which deliver them"@en ;
    skos:inScheme risk: ;
    skos:prefLabel "Business Impact Analysis"@en ;
    dpv:isInstanceOf risk:QualitativeRiskAssessmentTechnique,
        risk:QuantitativeRiskAssessmentTechnique .

risk:BusinessPerformanceImpairment a skos:Concept,
        dpv:Concept ;
    dct:created ""^^xsd:date ;
    dct:source <https://www.iso.org/standard/75281.html> ;
    rdfs:isDefinedBy risk: ;
    sw:term_status "accepted"@en ;
    skos:definition ""@en ;
    skos:inScheme risk: ;
    skos:prefLabel "Business Performance Impairment"@en ;
    dpv:isSubTypeOf dpv:Detriment .

risk:Businessdisruption a skos:Concept,
        dpv:Concept ;
    dct:created ""^^xsd:date ;
    dct:source <https://www.iso.org/standard/75281.html> ;
    rdfs:isDefinedBy risk: ;
    sw:term_status "accepted"@en ;
    skos:definition ""@en ;
    skos:inScheme risk: ;
    skos:prefLabel "Business disruption"@en ;
    dpv:isSubTypeOf dpv:Detriment .

risk:CVaR a skos:Concept,
        dpv:Concept ;
    dct:created ""^^xsd:date ;
    dct:source <https://www.iso.org/standard/72140.html> ;
    rdfs:isDefinedBy risk: ;
    sw:term_status "accepted"@en ;
    skos:definition "A measure of the expected loss from a financial portfolio in the worst a % of cases. Also called expected shortfall (ES)"@en ;
    skos:inScheme risk: ;
    skos:prefLabel "Conditional Value at Risk (CVaR)"@en ;
    dpv:isInstanceOf risk:QuantitativeRiskAssessmentTechnique .

risk:CausalMapping a skos:Concept,
        dpv:Concept ;
    dct:created ""^^xsd:date ;
    dct:source <https://www.iso.org/standard/72140.html> ;
    rdfs:isDefinedBy risk: ;
    sw:term_status "accepted"@en ;
    skos:definition "A network diagram representing events, causes and effects and their relationships."@en ;
    skos:inScheme risk: ;
    skos:prefLabel "Causal Mapping"@en ;
    dpv:isInstanceOf risk:QualitativeRiskAssessmentTechnique .

risk:CauseConsequenceAnalysis a skos:Concept,
        dpv:Concept ;
    dct:created ""^^xsd:date ;
    dct:source <https://www.iso.org/standard/72140.html> ;
    rdfs:isDefinedBy risk: ;
    sw:term_status "accepted"@en ;
    skos:definition "A combination of fault and event tree analysis that allows inclusion of time delays. Both causes and consequences of an initiating event are considered."@en ;
    skos:inScheme risk: ;
    skos:prefLabel "Cause-Consequence Analysis"@en ;
    dpv:isInstanceOf risk:QuantitativeRiskAssessmentTechnique .

risk:ChangeConsequence a skos:Concept,
        dpv:Concept ;
    dct:created ""^^xsd:date ;
    rdfs:isDefinedBy risk: ;
    sw:term_status "accepted"@en ;
    skos:definition "Risk Control that changes Consequence"@en ;
    skos:inScheme risk: ;
    skos:prefLabel "Change Consequence"@en ;
    dpv:isSubTypeOf risk:ControlConsequence .

risk:ChangeImpact a skos:Concept,
        dpv:Concept ;
    dct:created ""^^xsd:date ;
    rdfs:isDefinedBy risk: ;
    sw:term_status "accepted"@en ;
    skos:definition "Risk Control that changes Impact"@en ;
    skos:inScheme risk: ;
    skos:prefLabel "Change Impact"@en ;
    dpv:isSubTypeOf risk:ControlConsequence .

risk:Checklists a skos:Concept,
        dpv:Concept ;
    dct:created ""^^xsd:date ;
    dct:source <https://www.iso.org/standard/72140.html> ;
    rdfs:isDefinedBy risk: ;
    sw:term_status "accepted"@en ;
    skos:definition "A checklist based on experience or on concepts and models that can be used to help identify risks or controls."@en ;
    skos:inScheme risk: ;
    skos:prefLabel "Checklists"@en ;
    dpv:isInstanceOf risk:QualitativeRiskAssessmentTechnique .

risk:Cindynic a skos:Concept,
        dpv:Concept ;
    dct:created ""^^xsd:date ;
    dct:source <https://www.iso.org/standard/72140.html> ;
    rdfs:isDefinedBy risk: ;
    sw:term_status "accepted"@en ;
    skos:definition "Considers goals, values, rules, data and models of stakeholders and identifies inconsistencies, ambiguities, omissions and ignorance. These form systemic sources and drivers of risk."@en ;
    skos:inScheme risk: ;
    skos:prefLabel "Cindynic Approach"@en ;
    dpv:isInstanceOf risk:QualitativeRiskAssessmentTechnique .

risk:Classifications a skos:Concept,
        dpv:Concept ;
    dct:created ""^^xsd:date ;
    dct:source <https://www.iso.org/standard/72140.html> ;
    rdfs:isDefinedBy risk: ;
    sw:term_status "accepted"@en ;
    skos:definition "A classification list based on experience or on concepts and models that can be used to help identify risks or controls."@en ;
    skos:inScheme risk: ;
    skos:prefLabel "Classifications"@en ;
    dpv:isInstanceOf risk:QualitativeRiskAssessmentTechnique .

risk:ConfidentialityBreach a skos:Concept,
        dpv:Concept ;
    dct:created ""^^xsd:date ;
    dct:source <https://www.iso.org/standard/75281.html> ;
    rdfs:isDefinedBy risk: ;
    sw:term_status "accepted"@en ;
    skos:definition ""@en ;
    skos:inScheme risk: ;
    skos:prefLabel "Confidentiality Breach"@en ;
    dpv:isSubTypeOf dpv:Detriment .

risk:CorruptionData a skos:Concept,
        dpv:Concept ;
    dct:created ""^^xsd:date ;
    dct:source <https://www.iso.org/standard/75281.html> ;
    rdfs:isDefinedBy risk: ;
    sw:term_status "accepted"@en ;
    skos:definition ""@en ;
    skos:inScheme risk: ;
    skos:prefLabel "Corruption of Data"@en ;
    dpv:isSubTypeOf dpv:Damage .

risk:CostAcquisition a skos:Concept,
        dpv:Concept ;
    dct:created ""^^xsd:date ;
    dct:source <https://www.iso.org/standard/75281.html> ;
    rdfs:isDefinedBy risk: ;
    sw:term_status "accepted"@en ;
    skos:definition ""@en ;
    skos:inScheme risk: ;
    skos:prefLabel "Cost of Acquisition"@en ;
    dpv:isSubTypeOf dpv:Detriment .

risk:CostBackup a skos:Concept,
        dpv:Concept ;
    dct:created ""^^xsd:date ;
    dct:source <https://www.iso.org/standard/75281.html> ;
    rdfs:isDefinedBy risk: ;
    sw:term_status "accepted"@en ;
    skos:definition ""@en ;
    skos:inScheme risk: ;
    skos:prefLabel "Cost of Backup"@en ;
    dpv:isSubTypeOf dpv:Detriment .

risk:CostBenefitAnalysis a skos:Concept,
        dpv:Concept ;
    dct:created ""^^xsd:date ;
    dct:source <https://www.iso.org/standard/72140.html> ;
    rdfs:isDefinedBy risk: ;
    sw:term_status "accepted"@en ;
    skos:definition "Uses money as a scale for estimating positive and negative, tangible and intangible, consequences of different options."@en ;
    skos:inScheme risk: ;
    skos:prefLabel "Cost/benefit Analysis"@en ;
    dpv:isInstanceOf risk:QuantitativeRiskAssessmentTechnique .

risk:CostConfiguration a skos:Concept,
        dpv:Concept ;
    dct:created ""^^xsd:date ;
    dct:source <https://www.iso.org/standard/75281.html> ;
    rdfs:isDefinedBy risk: ;
    sw:term_status "accepted"@en ;
    skos:definition ""@en ;
    skos:inScheme risk: ;
    skos:prefLabel "Cost of Configuration"@en ;
    dpv:isSubTypeOf dpv:Detriment .

risk:CostInstallation a skos:Concept,
        dpv:Concept ;
    dct:created ""^^xsd:date ;
    dct:source <https://www.iso.org/standard/75281.html> ;
    rdfs:isDefinedBy risk: ;
    sw:term_status "accepted"@en ;
    skos:definition ""@en ;
    skos:inScheme risk: ;
    skos:prefLabel "Cost of Installation"@en ;
    dpv:isSubTypeOf dpv:Detriment .

risk:CostJudicialPenalties a skos:Concept,
        dpv:Concept ;
    dct:created ""^^xsd:date ;
    dct:source <https://www.iso.org/standard/75281.html> ;
    rdfs:isDefinedBy risk: ;
    sw:term_status "accepted"@en ;
    skos:definition ""@en ;
    skos:inScheme risk: ;
    skos:prefLabel "Cost of Judicial Penalties"@en ;
    dpv:isSubTypeOf dpv:Detriment .

risk:CostJudicialProceedings a skos:Concept,
        dpv:Concept ;
    dct:created ""^^xsd:date ;
    dct:source <https://www.iso.org/standard/75281.html> ;
    rdfs:isDefinedBy risk: ;
    sw:term_status "accepted"@en ;
    skos:definition ""@en ;
    skos:inScheme risk: ;
    skos:prefLabel "Cost of Judicial Proceedings"@en ;
    dpv:isSubTypeOf dpv:Detriment .

risk:CostOperationInterruption a skos:Concept,
        dpv:Concept ;
    dct:created ""^^xsd:date ;
    dct:source <https://www.iso.org/standard/75281.html> ;
    rdfs:isDefinedBy risk: ;
    sw:term_status "accepted"@en ;
    skos:definition ""@en ;
    skos:inScheme risk: ;
    skos:prefLabel "Cost of Operation Interruption"@en ;
    dpv:isSubTypeOf dpv:Detriment .

risk:CostSuspendedOperations a skos:Concept,
        dpv:Concept ;
    dct:created ""^^xsd:date ;
    dct:source <https://www.iso.org/standard/75281.html> ;
    rdfs:isDefinedBy risk: ;
    sw:term_status "accepted"@en ;
    skos:definition ""@en ;
    skos:inScheme risk: ;
    skos:prefLabel "Cost of Suspended Operations"@en ;
    dpv:isSubTypeOf dpv:Detriment .

risk:CrossImpactAnalysis a skos:Concept,
        dpv:Concept ;
    dct:created ""^^xsd:date ;
    dct:source <https://www.iso.org/standard/72140.html> ;
    rdfs:isDefinedBy risk: ;
    sw:term_status "accepted"@en ;
    skos:definition "Evaluates changes in the probability of the occurrence of a given set of events consequent on the actual occurrence of one of them."@en ;
    skos:inScheme risk: ;
    skos:prefLabel "Cross Impact Analysis"@en ;
    dpv:isInstanceOf risk:QuantitativeRiskAssessmentTechnique .

risk:CyberSpying a skos:Concept,
        dpv:Concept ;
    dct:created ""^^xsd:date ;
    dct:source <https://www.iso.org/standard/75281.html> ;
    rdfs:isDefinedBy risk: ;
    sw:term_status "accepted"@en ;
    skos:definition ""@en ;
    skos:inScheme risk: ;
    skos:prefLabel "Cyber Spying"@en ;
    dpv:isSubTypeOf dpv:NonMaterialDamage .

risk:CyberStalking a skos:Concept,
        dpv:Concept ;
    dct:created ""^^xsd:date ;
    dct:source <https://www.iso.org/standard/75281.html> ;
    rdfs:isDefinedBy risk: ;
    sw:term_status "accepted"@en ;
    skos:definition ""@en ;
    skos:inScheme risk: ;
    skos:prefLabel "Cyber Stalking"@en ;
    dpv:isSubTypeOf dpv:NonMaterialDamage .

risk:DPIA a skos:Concept,
        dpv:Concept ;
    dct:created ""^^xsd:date ;
    dct:source <https://www.iso.org/standard/72140.html> ;
    rdfs:isDefinedBy risk: ;
    sw:term_status "accepted"@en ;
    skos:definition "Analyses how incidents and events could affect the protection of data and its effects on persons and identifies and quantifies the capabilities that would be needed to manage it."@en ;
    skos:inScheme risk: ;
    skos:prefLabel "Data Protection Impact Assessment (DPIA)"@en ;
    dpv:isInstanceOf risk:QualitativeRiskAssessmentTechnique .

risk:DangertoCustomers a skos:Concept,
        dpv:Concept ;
    dct:created ""^^xsd:date ;
    dct:source <https://www.iso.org/standard/75281.html> ;
    rdfs:isDefinedBy risk: ;
    sw:term_status "accepted"@en ;
    skos:definition ""@en ;
    skos:inScheme risk: ;
    skos:prefLabel "Danger to Customers"@en ;
    dpv:isSubTypeOf dpv:Harm .

risk:DangertoPersonnel a skos:Concept,
        dpv:Concept ;
    dct:created ""^^xsd:date ;
    dct:source <https://www.iso.org/standard/75281.html> ;
    rdfs:isDefinedBy risk: ;
    sw:term_status "accepted"@en ;
    skos:definition ""@en ;
    skos:inScheme risk: ;
    skos:prefLabel "Danger to Personnel"@en ;
    dpv:isSubTypeOf dpv:Harm .

risk:DataBreach a skos:Concept,
        dpv:Concept ;
    dct:created ""^^xsd:date ;
    dct:source <https://www.iso.org/standard/75281.html> ;
    rdfs:isDefinedBy risk: ;
    sw:term_status "accepted"@en ;
    skos:definition ""@en ;
    skos:inScheme risk: ;
    skos:prefLabel "Data Breach"@en ;
    dpv:isSubTypeOf dpv:Damage .

risk:DecisionTreeAnalysis a skos:Concept,
        dpv:Concept ;
    dct:created ""^^xsd:date ;
    dct:source <https://www.iso.org/standard/72140.html> ;
    rdfs:isDefinedBy risk: ;
    sw:term_status "accepted"@en ;
    skos:definition "Uses a tree-like representation or model of decisions and their possible consequences. Outcomes are usually expressed in monetary terms or in terms of utility."@en ;
    skos:inScheme risk: ;
    skos:prefLabel "Decision Tree Analysis"@en ;
    dpv:isInstanceOf risk:QuantitativeRiskAssessmentTechnique .

risk:DelphiTechnique a skos:Concept,
        dpv:Concept ;
    dct:created ""^^xsd:date ;
    dct:source <https://www.iso.org/standard/72140.html> ;
    rdfs:isDefinedBy risk: ;
    sw:term_status "accepted"@en ;
    skos:definition "Collects judgements through a set of sequential questionnaires. People participate individually but receive feedback on the responses of others after each set of questions."@en ;
    skos:inScheme risk: ;
    skos:prefLabel "Delphi Technique"@en ;
    dpv:isInstanceOf risk:QualitativeRiskAssessmentTechnique .

risk:DenialServiceAttack a skos:Concept,
        dpv:Concept ;
    dct:created ""^^xsd:date ;
    dct:source <https://www.iso.org/standard/75281.html> ;
    rdfs:isDefinedBy risk: ;
    sw:term_status "accepted"@en ;
    skos:definition ""@en ;
    skos:inScheme risk: ;
    skos:prefLabel "Denial of Service Attack"@en ;
    dpv:isSubTypeOf dpv:Detriment .

risk:DistributedDenialServiceAttack a skos:Concept,
        dpv:Concept ;
    dct:created ""^^xsd:date ;
    dct:source <https://www.iso.org/standard/75281.html> ;
    rdfs:isDefinedBy risk: ;
    sw:term_status "accepted"@en ;
    skos:definition ""@en ;
    skos:inScheme risk: ;
    skos:prefLabel "Distributed Denial of Service Attack"@en ;
    dpv:isSubTypeOf dpv:Detriment .

risk:Eavesdropping a skos:Concept,
        dpv:Concept ;
    dct:created ""^^xsd:date ;
    dct:source <https://www.iso.org/standard/75281.html> ;
    rdfs:isDefinedBy risk: ;
    sw:term_status "accepted"@en ;
    skos:definition ""@en ;
    skos:inScheme risk: ;
    skos:prefLabel "Eavesdropping"@en ;
    dpv:isSubTypeOf dpv:NonMaterialDamage .

risk:EnvironmentalSafetyEndangerment a skos:Concept,
        dpv:Concept ;
    dct:created ""^^xsd:date ;
    dct:source <https://www.iso.org/standard/75281.html> ;
    rdfs:isDefinedBy risk: ;
    sw:term_status "accepted"@en ;
    skos:definition ""@en ;
    skos:inScheme risk: ;
    skos:prefLabel "Environmental Safety Endangerment"@en ;
    dpv:isSubTypeOf dpv:Harm .

risk:EquipmentFailure a skos:Concept,
        dpv:Concept ;
    dct:created ""^^xsd:date ;
    dct:source <https://www.iso.org/standard/75281.html> ;
    rdfs:isDefinedBy risk: ;
    sw:term_status "accepted"@en ;
    skos:definition ""@en ;
    skos:inScheme risk: ;
    skos:prefLabel "Equipment Failure"@en ;
    dpv:isSubTypeOf dpv:Damage .

risk:EquipmentMalfunction a skos:Concept,
        dpv:Concept ;
    dct:created ""^^xsd:date ;
    dct:source <https://www.iso.org/standard/75281.html> ;
    rdfs:isDefinedBy risk: ;
    sw:term_status "accepted"@en ;
    skos:definition ""@en ;
    skos:inScheme risk: ;
    skos:prefLabel "Equipment Malfunction"@en ;
    dpv:isSubTypeOf dpv:Detriment .

risk:ErrornousUse a skos:Concept,
        dpv:Concept ;
    dct:created ""^^xsd:date ;
    dct:source <https://www.iso.org/standard/75281.html> ;
    rdfs:isDefinedBy risk: ;
    sw:term_status "accepted"@en ;
    skos:definition ""@en ;
    skos:inScheme risk: ;
    skos:prefLabel "Errornous Use"@en ;
    dpv:isSubTypeOf dpv:Detriment .

risk:EventTreeAnalysis a skos:Concept,
        dpv:Concept ;
    dct:created ""^^xsd:date ;
    dct:source <https://www.iso.org/standard/72140.html> ;
    rdfs:isDefinedBy risk: ;
    sw:term_status "accepted"@en ;
    skos:definition "Models the possible outcomes from a given initiating event and the status of controls thus analysing the frequency or probability of the various possible outcomes."@en ;
    skos:inScheme risk: ;
    skos:prefLabel "Event Tree Analysis"@en ;
    dpv:isInstanceOf risk:QualitativeRiskAssessmentTechnique,
        risk:QuantitativeRiskAssessmentTechnique .

risk:ExtremelyHighLikelihood a skos:Concept,
        dpv:Concept ;
    dct:created ""^^xsd:date ;
    rdfs:isDefinedBy risk: ;
    sw:term_status "accepted"@en ;
    skos:definition "Level where Likelihood is Extremely High"@en ;
    skos:inScheme risk: ;
    skos:note "The suggested quantitative value for this concept is 0.99 on a scale of 0 to 1"@en ;
    skos:prefLabel "Extremely High Likelihood"@en ;
    dpv:isInstanceOf dpv:Likelihood,
        risk:7LikelihoodLevels .

risk:ExtremelyHighRisk a skos:Concept,
        dpv:Concept ;
    dct:created ""^^xsd:date ;
    rdfs:isDefinedBy risk: ;
    sw:term_status "accepted"@en ;
    skos:definition "Level where Risk is Extremely High"@en ;
    skos:inScheme risk: ;
    skos:note "The suggested quantitative value for this concept is 0.99 on a scale of 0 to 1"@en ;
    skos:prefLabel "Extremely High Risk"@en ;
    dpv:isInstanceOf dpv:RiskLevel,
        risk:7RiskLevels .

risk:ExtremelyHighSeverity a skos:Concept,
        dpv:Concept ;
    dct:created ""^^xsd:date ;
    rdfs:isDefinedBy risk: ;
    sw:term_status "accepted"@en ;
    skos:definition "Level where Severity is Extremely High"@en ;
    skos:inScheme risk: ;
    skos:note "The suggested quantitative value for this concept is 0.99 on a scale of 0 to 1"@en ;
    skos:prefLabel "Extremely High Severity"@en ;
    dpv:isInstanceOf dpv:Severity,
        risk:7SeverityLevels .

risk:ExtremelyLowLikelihood a skos:Concept,
        dpv:Concept ;
    dct:created ""^^xsd:date ;
    rdfs:isDefinedBy risk: ;
    sw:term_status "accepted"@en ;
    skos:definition "Level where Likelihood is Extremely Low"@en ;
    skos:inScheme risk: ;
    skos:note "The suggested quantitative value for this concept is 0.01 on a scale of 0 to 1"@en ;
    skos:prefLabel "Extremely Low Likelihood"@en ;
    dpv:isInstanceOf dpv:Likelihood,
        risk:7LikelihoodLevels .

risk:ExtremelyLowRisk a skos:Concept,
        dpv:Concept ;
    dct:created ""^^xsd:date ;
    rdfs:isDefinedBy risk: ;
    sw:term_status "accepted"@en ;
    skos:definition "Level where Risk is Extremely Low"@en ;
    skos:inScheme risk: ;
    skos:note "The suggested quantitative value for this concept is 0.01 on a scale of 0 to 1"@en ;
    skos:prefLabel "Extremely Low Risk"@en ;
    dpv:isInstanceOf dpv:RiskLevel,
        risk:7RiskLevels .

risk:ExtremelyLowSeverity a skos:Concept,
        dpv:Concept ;
    dct:created ""^^xsd:date ;
    rdfs:isDefinedBy risk: ;
    sw:term_status "accepted"@en ;
    skos:definition "Level where Severity is Extremely Low"@en ;
    skos:inScheme risk: ;
    skos:note "The suggested quantitative value for this concept is 0.01 on a scale of 0 to 1"@en ;
    skos:prefLabel "Extremely Low Severity"@en ;
    dpv:isInstanceOf dpv:Severity,
        risk:7SeverityLevels .

risk:FMEA a skos:Concept,
        dpv:Concept ;
    dct:created ""^^xsd:date ;
    dct:source <https://www.iso.org/standard/72140.html> ;
    rdfs:isDefinedBy risk: ;
    sw:term_status "accepted"@en ;
    skos:definition "Considers the ways in which each component of a system might fail and the failure causes and effects."@en ;
    skos:inScheme risk: ;
    skos:prefLabel "Failure Modes And Effects Analysis (FMEA)"@en ;
    dpv:isInstanceOf risk:QualitativeRiskAssessmentTechnique,
        risk:QuantitativeRiskAssessmentTechnique .

risk:FMECA a skos:Concept,
        dpv:Concept ;
    dct:created ""^^xsd:date ;
    dct:source <https://www.iso.org/standard/72140.html> ;
    rdfs:isDefinedBy risk: ;
    sw:term_status "accepted"@en ;
    skos:definition "Considers the ways in which each component of a system might fail and the failure causes and effects. FMEA followed by a criticality analysis which defines the significance of each failure mode (FMECA)."@en ;
    skos:inScheme risk: ;
    skos:prefLabel "Failure Modes And Effects And Criticality Analysis (FMECA)"@en ;
    dpv:isInstanceOf risk:QualitativeRiskAssessmentTechnique,
        risk:QuantitativeRiskAssessmentTechnique .

risk:FNDiagrams a skos:Concept,
        dpv:Concept ;
    dct:created ""^^xsd:date ;
    dct:source <https://www.iso.org/standard/72140.html> ;
    rdfs:isDefinedBy risk: ;
    sw:term_status "accepted"@en ;
    skos:definition "Special case of quantitative consequence/likelihood graph applied to consideration of tolerability of risk to human life."@en ;
    skos:inScheme risk: ;
    skos:prefLabel "F-N Diagrams"@en ;
    dpv:isInstanceOf risk:QuantitativeRiskAssessmentTechnique .

risk:FaultTreeAnalysis a skos:Concept,
        dpv:Concept ;
    dct:created ""^^xsd:date ;
    dct:source <https://www.iso.org/standard/72140.html> ;
    rdfs:isDefinedBy risk: ;
    sw:term_status "accepted"@en ;
    skos:definition "Analyses causes of a focus event using Boolean logic to describe combinations of faults. Variations include a success tree where the top event is desired and a cause tree used to investigate past events."@en ;
    skos:inScheme risk: ;
    skos:prefLabel "Fault Tree Analysis"@en ;
    dpv:isInstanceOf risk:QualitativeRiskAssessmentTechnique,
        risk:QuantitativeRiskAssessmentTechnique .

risk:FinancialEquipmentCosts a skos:Concept,
        dpv:Concept ;
    dct:created ""^^xsd:date ;
    dct:source <https://www.iso.org/standard/75281.html> ;
    rdfs:isDefinedBy risk: ;
    sw:term_status "accepted"@en ;
    skos:definition ""@en ;
    skos:inScheme risk: ;
    skos:prefLabel "Financial Equipment Costs"@en ;
    dpv:isSubTypeOf dpv:Detriment .

risk:FinancialInvestigationCosts a skos:Concept,
        dpv:Concept ;
    dct:created ""^^xsd:date ;
    dct:source <https://www.iso.org/standard/75281.html> ;
    rdfs:isDefinedBy risk: ;
    sw:term_status "accepted"@en ;
    skos:definition ""@en ;
    skos:inScheme risk: ;
    skos:prefLabel "Financial Investigation Costs"@en ;
    dpv:isSubTypeOf dpv:Detriment .

risk:FinancialLoss a skos:Concept,
        dpv:Concept ;
    dct:created ""^^xsd:date ;
    dct:source <https://www.iso.org/standard/75281.html> ;
    rdfs:isDefinedBy risk: ;
    sw:term_status "accepted"@en ;
    skos:definition ""@en ;
    skos:inScheme risk: ;
    skos:prefLabel "Financial Loss"@en ;
    dpv:isSubTypeOf dpv:Damage .

risk:FinancialPersonnelCosts a skos:Concept,
        dpv:Concept ;
    dct:created ""^^xsd:date ;
    dct:source <https://www.iso.org/standard/75281.html> ;
    rdfs:isDefinedBy risk: ;
    sw:term_status "accepted"@en ;
    skos:definition ""@en ;
    skos:inScheme risk: ;
    skos:prefLabel "Financial Personnel Costs"@en ;
    dpv:isSubTypeOf dpv:Detriment .

risk:FinancialRepairCosts a skos:Concept,
        dpv:Concept ;
    dct:created ""^^xsd:date ;
    dct:source <https://www.iso.org/standard/75281.html> ;
    rdfs:isDefinedBy risk: ;
    sw:term_status "accepted"@en ;
    skos:definition ""@en ;
    skos:inScheme risk: ;
    skos:prefLabel "Financial Repair Costs"@en ;
    dpv:isSubTypeOf dpv:Detriment .

risk:Fishbone a skos:Concept,
        dpv:Concept ;
    dct:created ""^^xsd:date ;
    dct:source <https://www.iso.org/standard/72140.html> ;
    rdfs:isDefinedBy risk: ;
    sw:term_status "accepted"@en ;
    skos:definition "Identifies contributory factors to a defined outcome (wanted or unwanted). Contributory factors are usually divided into predefined categories and displayed in a tree structure or a fishbone diagram."@en ;
    skos:inScheme risk: ;
    skos:prefLabel "Ishikawa (Fishbone)"@en ;
    dpv:isInstanceOf risk:QualitativeRiskAssessmentTechnique .

risk:Fraud a skos:Concept,
        dpv:Concept ;
    dct:created ""^^xsd:date ;
    dct:source <https://www.iso.org/standard/75281.html> ;
    rdfs:isDefinedBy risk: ;
    sw:term_status "accepted"@en ;
    skos:definition ""@en ;
    skos:inScheme risk: ;
    skos:prefLabel "Fraud"@en ;
    dpv:isSubTypeOf dpv:Harm .

risk:GameTheory a skos:Concept,
        dpv:Concept ;
    dct:created ""^^xsd:date ;
    dct:source <https://www.iso.org/standard/72140.html> ;
    rdfs:isDefinedBy risk: ;
    sw:term_status "accepted"@en ;
    skos:definition "The study of strategic decision making to model the impact of the decisions of different players involved in the game. Example application area can be risk based pricing."@en ;
    skos:inScheme risk: ;
    skos:prefLabel "Game Theory"@en ;
    dpv:isInstanceOf risk:QuantitativeRiskAssessmentTechnique .

risk:GovernmentCrisis a skos:Concept,
        dpv:Concept ;
    dct:created ""^^xsd:date ;
    dct:source <https://www.iso.org/standard/75281.html> ;
    rdfs:isDefinedBy risk: ;
    sw:term_status "accepted"@en ;
    skos:definition ""@en ;
    skos:inScheme risk: ;
    skos:prefLabel "Government Crisis"@en ;
    dpv:isSubTypeOf dpv:Detriment .

risk:HACCP a skos:Concept,
        dpv:Concept ;
    dct:created ""^^xsd:date ;
    dct:source <https://www.iso.org/standard/72140.html> ;
    rdfs:isDefinedBy risk: ;
    sw:term_status "accepted"@en ;
    skos:definition "Analyses the risk reduction that can be achieved by various layers of protection."@en ;
    skos:inScheme risk: ;
    skos:prefLabel "Hazard Analysis And Critical Control Points (HACCP)"@en ;
    dpv:isInstanceOf risk:QualitativeRiskAssessmentTechnique .

risk:HAZOP a skos:Concept,
        dpv:Concept ;
    dct:created ""^^xsd:date ;
    dct:source <https://www.iso.org/standard/72140.html> ;
    rdfs:isDefinedBy risk: ;
    sw:term_status "accepted"@en ;
    skos:definition "A structured and systematic examination of a planned or existing process or operation in order to identify and evaluate problems that might represent risk to personnel or equipment, or prevent efficient operation"@en ;
    skos:inScheme risk: ;
    skos:prefLabel "Hazard And Operability Studies (HAZOP)"@en ;
    dpv:isInstanceOf risk:QualitativeRiskAssessmentTechnique .

risk:HaltSource a skos:Concept,
        dpv:Concept ;
    dct:created ""^^xsd:date ;
    rdfs:isDefinedBy risk: ;
    sw:term_status "accepted"@en ;
    skos:definition "Risk Control that halts the risk source or prevents it from materialising"@en ;
    skos:inScheme risk: ;
    skos:prefLabel "Halt Source"@en ;
    dpv:isSubTypeOf risk:ControlRiskSource .

risk:HighLikelihood a skos:Concept,
        dpv:Concept ;
    dct:created ""^^xsd:date ;
    rdfs:isDefinedBy risk: ;
    sw:term_status "accepted"@en ;
    skos:definition "Level where Likelihood is High"@en ;
    skos:inScheme risk: ;
    skos:note "The suggested quantitative value for this concept is 0.75 on a scale of 0 to 1"@en ;
    skos:prefLabel "High Likelihood"@en ;
    dpv:isInstanceOf dpv:Likelihood,
        risk:3LikelihoodLevels,
        risk:5LikelihoodLevels,
        risk:7LikelihoodLevels .

risk:HighRisk a skos:Concept,
        dpv:Concept ;
    dct:created ""^^xsd:date ;
    rdfs:isDefinedBy risk: ;
    sw:term_status "accepted"@en ;
    skos:definition "Level where Risk is High"@en ;
    skos:inScheme risk: ;
    skos:note "The suggested quantitative value for this concept is 0.75 on a scale of 0 to 1"@en ;
    skos:prefLabel "High Risk"@en ;
    dpv:isInstanceOf dpv:RiskLevel,
        risk:3RiskLevels,
        risk:5RiskLevels,
        risk:7RiskLevels .

risk:HighSeverity a skos:Concept,
        dpv:Concept ;
    dct:created ""^^xsd:date ;
    rdfs:isDefinedBy risk: ;
    sw:term_status "accepted"@en ;
    skos:definition "Level where Severity is High"@en ;
    skos:inScheme risk: ;
    skos:note "The suggested quantitative value for this concept is 0.75 on a scale of 0 to 1"@en ;
    skos:prefLabel "High Severity"@en ;
    dpv:isInstanceOf dpv:Severity,
        risk:3SeverityLevels,
        risk:5SeverityLevels,
        risk:7SeverityLevels .

risk:HumanReliabilityAnalysis a skos:Concept,
        dpv:Concept ;
    dct:created ""^^xsd:date ;
    dct:source <https://www.iso.org/standard/72140.html> ;
    rdfs:isDefinedBy risk: ;
    sw:term_status "accepted"@en ;
    skos:definition "A set of techniques for identifying the potential for human error and estimating the likelihood of failure."@en ;
    skos:inScheme risk: ;
    skos:prefLabel "Human Reliability Analysis"@en ;
    dpv:isInstanceOf risk:QualitativeRiskAssessmentTechnique,
        risk:QuantitativeRiskAssessmentTechnique .

risk:IllegalProcessingData a skos:Concept,
        dpv:Concept ;
    dct:created ""^^xsd:date ;
    dct:source <https://www.iso.org/standard/75281.html> ;
    rdfs:isDefinedBy risk: ;
    sw:term_status "accepted"@en ;
    skos:definition ""@en ;
    skos:inScheme risk: ;
    skos:prefLabel "Illegal Processing of Data"@en ;
    dpv:isSubTypeOf dpv:Damage .

risk:ImpacttoRights a skos:Concept,
        dpv:Concept ;
    dct:created ""^^xsd:date ;
    dct:source <https://www.iso.org/standard/75281.html> ;
    rdfs:isDefinedBy risk: ;
    sw:term_status "accepted"@en ;
    skos:definition ""@en ;
    skos:inScheme risk: ;
    skos:prefLabel "Impact to Rights"@en ;
    dpv:isSubTypeOf dpv:Impact .

risk:IncreaseInternalCost a skos:Concept,
        dpv:Concept ;
    dct:created ""^^xsd:date ;
    dct:source <https://www.iso.org/standard/75281.html> ;
    rdfs:isDefinedBy risk: ;
    sw:term_status "accepted"@en ;
    skos:definition ""@en ;
    skos:inScheme risk: ;
    skos:prefLabel "Increase Internal Cost"@en ;
    dpv:isSubTypeOf dpv:Detriment .

risk:IndustrialCrisis a skos:Concept,
        dpv:Concept ;
    dct:created ""^^xsd:date ;
    dct:source <https://www.iso.org/standard/75281.html> ;
    rdfs:isDefinedBy risk: ;
    sw:term_status "accepted"@en ;
    skos:definition ""@en ;
    skos:inScheme risk: ;
    skos:prefLabel "Industrial Crisis"@en ;
    dpv:isSubTypeOf dpv:Detriment .

risk:InfluenceDiagrams a skos:Concept,
        dpv:Concept ;
    dct:created ""^^xsd:date ;
    dct:source <https://www.iso.org/standard/72140.html> ;
    rdfs:isDefinedBy risk: ;
    sw:term_status "accepted"@en ;
    skos:definition "An extended version of Bayesian networks that includes variables representing uncertainties, consequences and actions"@en ;
    skos:inScheme risk: ;
    skos:prefLabel "Influence Diagrams"@en ;
    dpv:isInstanceOf risk:QuantitativeRiskAssessmentTechnique .

risk:Injury a skos:Concept,
        dpv:Concept ;
    dct:created ""^^xsd:date ;
    dct:source <https://www.iso.org/standard/75281.html> ;
    rdfs:isDefinedBy risk: ;
    sw:term_status "accepted"@en ;
    skos:definition ""@en ;
    skos:inScheme risk: ;
    skos:prefLabel "Injury"@en ;
    dpv:isSubTypeOf dpv:Harm .

risk:InterceptionCommunications a skos:Concept,
        dpv:Concept ;
    dct:created ""^^xsd:date ;
    dct:source <https://www.iso.org/standard/75281.html> ;
    rdfs:isDefinedBy risk: ;
    sw:term_status "accepted"@en ;
    skos:definition ""@en ;
    skos:inScheme risk: ;
    skos:prefLabel "Interception of Communications"@en ;
    dpv:isSubTypeOf dpv:Consequence .

risk:InternalOperationDisruption a skos:Concept,
        dpv:Concept ;
    dct:created ""^^xsd:date ;
    dct:source <https://www.iso.org/standard/75281.html> ;
    rdfs:isDefinedBy risk: ;
    sw:term_status "accepted"@en ;
    skos:definition ""@en ;
    skos:inScheme risk: ;
    skos:prefLabel "Internal Operation Disruption"@en ;
    dpv:isSubTypeOf dpv:Detriment .

risk:Interviews a skos:Concept,
        dpv:Concept ;
    dct:created ""^^xsd:date ;
    dct:source <https://www.iso.org/standard/72140.html> ;
    rdfs:isDefinedBy risk: ;
    sw:term_status "accepted"@en ;
    skos:definition "Structured or semi- structured one-to-one conversations to elicit views."@en ;
    skos:inScheme risk: ;
    skos:prefLabel "Interviews"@en ;
    dpv:isInstanceOf risk:QualitativeRiskAssessmentTechnique .

risk:LOPA a skos:Concept,
        dpv:Concept ;
    dct:created ""^^xsd:date ;
    dct:source <https://www.iso.org/standard/72140.html> ;
    rdfs:isDefinedBy risk: ;
    sw:term_status "accepted"@en ;
    skos:definition "Analyses the risk reduction that can be achieved by various layers of protection."@en ;
    skos:inScheme risk: ;
    skos:prefLabel "Layer Protection Analysis (LOPA)"@en ;
    dpv:isInstanceOf risk:QualitativeRiskAssessmentTechnique,
        risk:QuantitativeRiskAssessmentTechnique .

risk:LawEnforcementAdverseEffects a skos:Concept,
        dpv:Concept ;
    dct:created ""^^xsd:date ;
    dct:source <https://www.iso.org/standard/75281.html> ;
    rdfs:isDefinedBy risk: ;
    sw:term_status "accepted"@en ;
    skos:definition ""@en ;
    skos:inScheme risk: ;
    skos:prefLabel "Law Enforcement Adverse Effects"@en ;
    dpv:isSubTypeOf dpv:Detriment .

risk:LossAssets a skos:Concept,
        dpv:Concept ;
    dct:created ""^^xsd:date ;
    dct:source <https://www.iso.org/standard/75281.html> ;
    rdfs:isDefinedBy risk: ;
    sw:term_status "accepted"@en ;
    skos:definition ""@en ;
    skos:inScheme risk: ;
    skos:prefLabel "Loss of Assets"@en ;
    dpv:isSubTypeOf dpv:MaterialDamage .

risk:LossCompetitiveAdvantage a skos:Concept,
        dpv:Concept ;
    dct:created ""^^xsd:date ;
    dct:source <https://www.iso.org/standard/75281.html> ;
    rdfs:isDefinedBy risk: ;
    sw:term_status "accepted"@en ;
    skos:definition ""@en ;
    skos:inScheme risk: ;
    skos:prefLabel "Loss of Competitive Advantage"@en ;
    dpv:isSubTypeOf dpv:NonMaterialDamage .

risk:LossCredibility a skos:Concept,
        dpv:Concept ;
    dct:created ""^^xsd:date ;
    dct:source <https://www.iso.org/standard/75281.html> ;
    rdfs:isDefinedBy risk: ;
    sw:term_status "accepted"@en ;
    skos:definition ""@en ;
    skos:inScheme risk: ;
    skos:prefLabel "Loss of Credibility"@en ;
    dpv:isSubTypeOf dpv:Detriment .

risk:LossCustomerConfidence a skos:Concept,
        dpv:Concept ;
    dct:created ""^^xsd:date ;
    dct:source <https://www.iso.org/standard/75281.html> ;
    rdfs:isDefinedBy risk: ;
    sw:term_status "accepted"@en ;
    skos:definition ""@en ;
    skos:inScheme risk: ;
    skos:prefLabel "Loss of Customer Confidence"@en ;
    dpv:isSubTypeOf dpv:Detriment .

risk:LossCustomers a skos:Concept,
        dpv:Concept ;
    dct:created ""^^xsd:date ;
    dct:source <https://www.iso.org/standard/75281.html> ;
    rdfs:isDefinedBy risk: ;
    sw:term_status "accepted"@en ;
    skos:definition ""@en ;
    skos:inScheme risk: ;
    skos:prefLabel "Loss of Customers"@en ;
    dpv:isSubTypeOf dpv:NonMaterialDamage .

risk:LossFunds a skos:Concept,
        dpv:Concept ;
    dct:created ""^^xsd:date ;
    dct:source <https://www.iso.org/standard/75281.html> ;
    rdfs:isDefinedBy risk: ;
    sw:term_status "accepted"@en ;
    skos:definition ""@en ;
    skos:inScheme risk: ;
    skos:prefLabel "Loss of Funds"@en ;
    dpv:isSubTypeOf dpv:MaterialDamage .

risk:LossGoods a skos:Concept,
        dpv:Concept ;
    dct:created ""^^xsd:date ;
    dct:source <https://www.iso.org/standard/75281.html> ;
    rdfs:isDefinedBy risk: ;
    sw:term_status "accepted"@en ;
    skos:definition ""@en ;
    skos:inScheme risk: ;
    skos:prefLabel "Loss of Goods"@en ;
    dpv:isSubTypeOf dpv:MaterialDamage .

risk:LossGoodwill a skos:Concept,
        dpv:Concept ;
    dct:created ""^^xsd:date ;
    dct:source <https://www.iso.org/standard/75281.html> ;
    rdfs:isDefinedBy risk: ;
    sw:term_status "accepted"@en ;
    skos:definition ""@en ;
    skos:inScheme risk: ;
    skos:prefLabel "Loss of Goodwill"@en ;
    dpv:isSubTypeOf dpv:Detriment .

risk:LossNegotiatingCapacity a skos:Concept,
        dpv:Concept ;
    dct:created ""^^xsd:date ;
    dct:source <https://www.iso.org/standard/75281.html> ;
    rdfs:isDefinedBy risk: ;
    sw:term_status "accepted"@en ;
    skos:definition ""@en ;
    skos:inScheme risk: ;
    skos:prefLabel "Loss of Negotiating Capacity"@en ;
    dpv:isSubTypeOf dpv:Detriment .

risk:LossOpportunity a skos:Concept,
        dpv:Concept ;
    dct:created ""^^xsd:date ;
    dct:source <https://www.iso.org/standard/75281.html> ;
    rdfs:isDefinedBy risk: ;
    sw:term_status "accepted"@en ;
    skos:definition ""@en ;
    skos:inScheme risk: ;
    skos:prefLabel "Loss of Opportunity"@en ;
    dpv:isSubTypeOf dpv:Detriment .

risk:LossProprietaryInformation a skos:Concept,
        dpv:Concept ;
    dct:created ""^^xsd:date ;
    dct:source <https://www.iso.org/standard/75281.html> ;
    rdfs:isDefinedBy risk: ;
    sw:term_status "accepted"@en ;
    skos:definition ""@en ;
    skos:inScheme risk: ;
    skos:prefLabel "Loss of Proprietary Information"@en ;
    dpv:isSubTypeOf dpv:NonMaterialDamage .

risk:LossReputation a skos:Concept,
        dpv:Concept ;
    dct:created ""^^xsd:date ;
    dct:source <https://www.iso.org/standard/75281.html> ;
    rdfs:isDefinedBy risk: ;
    sw:term_status "accepted"@en ;
    skos:definition ""@en ;
    skos:inScheme risk: ;
    skos:prefLabel "Loss of Reputation"@en ;
    dpv:isSubTypeOf dpv:Detriment .

risk:LossSuppliers a skos:Concept,
        dpv:Concept ;
    dct:created ""^^xsd:date ;
    dct:source <https://www.iso.org/standard/75281.html> ;
    rdfs:isDefinedBy risk: ;
    sw:term_status "accepted"@en ;
    skos:definition ""@en ;
    skos:inScheme risk: ;
    skos:prefLabel "Loss of Suppliers"@en ;
    dpv:isSubTypeOf dpv:NonMaterialDamage .

risk:LossTechnologicalAdvantage a skos:Concept,
        dpv:Concept ;
    dct:created ""^^xsd:date ;
    dct:source <https://www.iso.org/standard/75281.html> ;
    rdfs:isDefinedBy risk: ;
    sw:term_status "accepted"@en ;
    skos:definition ""@en ;
    skos:inScheme risk: ;
    skos:prefLabel "Loss of Technological Advantage"@en ;
    dpv:isSubTypeOf dpv:NonMaterialDamage .

risk:LossTrust a skos:Concept,
        dpv:Concept ;
    dct:created ""^^xsd:date ;
    dct:source <https://www.iso.org/standard/75281.html> ;
    rdfs:isDefinedBy risk: ;
    sw:term_status "accepted"@en ;
    skos:definition ""@en ;
    skos:inScheme risk: ;
    skos:prefLabel "Loss of Trust"@en ;
    dpv:isSubTypeOf dpv:Detriment .

risk:LowLikelihood a skos:Concept,
        dpv:Concept ;
    dct:created ""^^xsd:date ;
    rdfs:isDefinedBy risk: ;
    sw:term_status "accepted"@en ;
    skos:definition "Level where Likelihood is Low"@en ;
    skos:inScheme risk: ;
    skos:note "The suggested quantitative value for this concept is 0.25 on a scale of 0 to 1"@en ;
    skos:prefLabel "Low Likelihood"@en ;
    dpv:isInstanceOf dpv:Likelihood,
        risk:3LikelihoodLevels,
        risk:5LikelihoodLevels,
        risk:7LikelihoodLevels .

risk:LowRisk a skos:Concept,
        dpv:Concept ;
    dct:created ""^^xsd:date ;
    rdfs:isDefinedBy risk: ;
    sw:term_status "accepted"@en ;
    skos:definition "Level where Risk is Low"@en ;
    skos:inScheme risk: ;
    skos:note "The suggested quantitative value for this concept is 0.25 on a scale of 0 to 1"@en ;
    skos:prefLabel "Low Risk"@en ;
    dpv:isInstanceOf dpv:RiskLevel,
        risk:3RiskLevels,
        risk:5RiskLevels,
        risk:7RiskLevels .

risk:LowSeverity a skos:Concept,
        dpv:Concept ;
    dct:created ""^^xsd:date ;
    rdfs:isDefinedBy risk: ;
    sw:term_status "accepted"@en ;
    skos:definition "Level where Severity is Low"@en ;
    skos:inScheme risk: ;
    skos:note "The suggested quantitative value for this concept is 0.25 on a scale of 0 to 1"@en ;
    skos:prefLabel "Low Severity"@en ;
    dpv:isInstanceOf dpv:Severity,
        risk:3SeverityLevels,
        risk:5SeverityLevels,
        risk:7SeverityLevels .

risk:MCA a skos:Concept,
        dpv:Concept ;
    dct:created ""^^xsd:date ;
    dct:source <https://www.iso.org/standard/72140.html> ;
    rdfs:isDefinedBy risk: ;
    sw:term_status "accepted"@en ;
    skos:definition "Compares options in a way that makes trade-offs explicit. Provides an alternative to cost/benefit analysis that does not need a monetary value to be allocated to all inputs."@en ;
    skos:inScheme risk: ;
    skos:prefLabel "Multi-criteria Analysis (MCA)"@en ;
    dpv:isInstanceOf risk:QualitativeRiskAssessmentTechnique .

risk:MarkovAnalysis a skos:Concept,
        dpv:Concept ;
    dct:created ""^^xsd:date ;
    dct:source <https://www.iso.org/standard/72140.html> ;
    rdfs:isDefinedBy risk: ;
    sw:term_status "accepted"@en ;
    skos:definition "Calculates the probability that a system that has the capacity to be in one of a number of states will be in a particular state at a time t in the future."@en ;
    skos:inScheme risk: ;
    skos:prefLabel "Markov Analysis"@en ;
    dpv:isInstanceOf risk:QuantitativeRiskAssessmentTechnique .

risk:MisuseBreachedInformation a skos:Concept,
        dpv:Concept ;
    dct:created ""^^xsd:date ;
    dct:source <https://www.iso.org/standard/75281.html> ;
    rdfs:isDefinedBy risk: ;
    sw:term_status "accepted"@en ;
    skos:definition ""@en ;
    skos:inScheme risk: ;
    skos:prefLabel "Misuse of Breached Information"@en ;
    dpv:isSubTypeOf dpv:Detriment .

risk:ModerateLikelihood a skos:Concept,
        dpv:Concept ;
    dct:created ""^^xsd:date ;
    rdfs:isDefinedBy risk: ;
    sw:term_status "accepted"@en ;
    skos:definition "Level where Likelihood is Moderate"@en ;
    skos:inScheme risk: ;
    skos:note "The suggested quantitative value for this concept is 0.5 on a scale of 0 to 1"@en ;
    skos:prefLabel "Moderate Likelihood"@en ;
    dpv:isInstanceOf dpv:Likelihood,
        risk:3LikelihoodLevels,
        risk:5LikelihoodLevels,
        risk:7LikelihoodLevels .

risk:ModerateRisk a skos:Concept,
        dpv:Concept ;
    dct:created ""^^xsd:date ;
    rdfs:isDefinedBy risk: ;
    sw:term_status "accepted"@en ;
    skos:definition "Level where Risk is Moderate"@en ;
    skos:inScheme risk: ;
    skos:note "The suggested quantitative value for this concept is 0.5 on a scale of 0 to 1"@en ;
    skos:prefLabel "Moderate Risk"@en ;
    dpv:isInstanceOf dpv:RiskLevel,
        risk:3RiskLevels,
        risk:5RiskLevels,
        risk:7RiskLevels .

risk:ModerateSeverity a skos:Concept,
        dpv:Concept ;
    dct:created ""^^xsd:date ;
    rdfs:isDefinedBy risk: ;
    sw:term_status "accepted"@en ;
    skos:definition "Level where Severity is Moderate"@en ;
    skos:inScheme risk: ;
    skos:note "The suggested quantitative value for this concept is 0.5 on a scale of 0 to 1"@en ;
    skos:prefLabel "Moderate Severity"@en ;
    dpv:isInstanceOf dpv:Severity,
        risk:3SeverityLevels,
        risk:5SeverityLevels,
        risk:7SeverityLevels .

risk:MonitorConsequence a skos:Concept,
        dpv:Concept ;
    dct:created ""^^xsd:date ;
    rdfs:isDefinedBy risk: ;
    sw:term_status "accepted"@en ;
    skos:definition "Risk Control that monitors a Risk Consequence"@en ;
    skos:inScheme risk: ;
    skos:prefLabel "Monitor Consequence"@en ;
    dpv:isSubTypeOf risk:ControlMonitors .

risk:MonitorImpact a skos:Concept,
        dpv:Concept ;
    dct:created ""^^xsd:date ;
    rdfs:isDefinedBy risk: ;
    sw:term_status "accepted"@en ;
    skos:definition "Risk Control that monitors a Risk Impact"@en ;
    skos:inScheme risk: ;
    skos:prefLabel "Monitor Impact"@en ;
    dpv:isSubTypeOf risk:ControlMonitors .

risk:MonitorRisk a skos:Concept,
        dpv:Concept ;
    dct:created ""^^xsd:date ;
    rdfs:isDefinedBy risk: ;
    sw:term_status "accepted"@en ;
    skos:definition "Risk Control that monitors a Risk"@en ;
    skos:inScheme risk: ;
    skos:prefLabel "Monitor Risk"@en ;
    dpv:isSubTypeOf risk:ControlMonitors .

risk:MonitorRiskControl a skos:Concept,
        dpv:Concept ;
    dct:created ""^^xsd:date ;
    rdfs:isDefinedBy risk: ;
    sw:term_status "accepted"@en ;
    skos:definition "Risk Control that monitors another Risk Control"@en ;
    skos:inScheme risk: ;
    skos:prefLabel "Monitor Risk Control"@en ;
    dpv:isSubTypeOf risk:ControlMonitors .

risk:MonitorRiskSource a skos:Concept,
        dpv:Concept ;
    dct:created ""^^xsd:date ;
    rdfs:isDefinedBy risk: ;
    sw:term_status "accepted"@en ;
    skos:definition "Risk Control that monitors a Risk Source"@en ;
    skos:inScheme risk: ;
    skos:prefLabel "Monitor Risk Source"@en ;
    dpv:isSubTypeOf risk:ControlMonitors .

risk:MonitorVulnerabilities a skos:Concept,
        dpv:Concept ;
    dct:created ""^^xsd:date ;
    rdfs:isDefinedBy risk: ;
    sw:term_status "accepted"@en ;
    skos:definition "Risk Control that monitors a Risk Vulnerability"@en ;
    skos:inScheme risk: ;
    skos:prefLabel "Monitor Vulnerabilities"@en ;
    dpv:isSubTypeOf risk:ControlMonitors .

risk:MonteCarloSimulation a skos:Concept,
        dpv:Concept ;
    dct:created ""^^xsd:date ;
    dct:source <https://www.iso.org/standard/72140.html> ;
    rdfs:isDefinedBy risk: ;
    sw:term_status "accepted"@en ;
    skos:definition "Calculates the probability of outcomes by running multiple simulations using random variables."@en ;
    skos:inScheme risk: ;
    skos:prefLabel "Monte Carlo Simulation"@en ;
    dpv:isInstanceOf risk:QuantitativeRiskAssessmentTechnique .

risk:NominalGroupTechnique a skos:Concept,
        dpv:Concept ;
    dct:created ""^^xsd:date ;
    dct:source <https://www.iso.org/standard/72140.html> ;
    rdfs:isDefinedBy risk: ;
    sw:term_status "accepted"@en ;
    skos:definition "Technique for eliciting views from a group of people where initial participation is as individuals with no interaction, then group discussion of ideas follows."@en ;
    skos:inScheme risk: ;
    skos:prefLabel "Nominal Group Technique"@en ;
    dpv:isInstanceOf risk:QualitativeRiskAssessmentTechnique .

risk:OrganisationDisruption a skos:Concept,
        dpv:Concept ;
    dct:created ""^^xsd:date ;
    dct:source <https://www.iso.org/standard/75281.html> ;
    rdfs:isDefinedBy risk: ;
    sw:term_status "accepted"@en ;
    skos:definition ""@en ;
    skos:inScheme risk: ;
    skos:prefLabel "Organisation Disruption"@en ;
    dpv:isSubTypeOf dpv:Detriment .

risk:PIA a skos:Concept,
        dpv:Concept ;
    dct:created ""^^xsd:date ;
    dct:source <https://www.iso.org/standard/72140.html> ;
    rdfs:isDefinedBy risk: ;
    sw:term_status "accepted"@en ;
    skos:definition "Analyses how incidents and events could affect a person's privacy and identifies and quantifies the capabilities that would be needed to manage it."@en ;
    skos:inScheme risk: ;
    skos:prefLabel "Privacy Impact Analysis (PIA)"@en ;
    dpv:isInstanceOf risk:QualitativeRiskAssessmentTechnique .

risk:ParetoCharts a skos:Concept,
        dpv:Concept ;
    dct:created ""^^xsd:date ;
    dct:source <https://www.iso.org/standard/72140.html> ;
    rdfs:isDefinedBy risk: ;
    sw:term_status "accepted"@en ;
    skos:definition "The Pareto principle (the 80–20 rule) states that, for many events, roughly 80 % of the effects come from 20 % of the causes."@en ;
    skos:inScheme risk: ;
    skos:prefLabel "Pareto Charts"@en ;
    dpv:isInstanceOf risk:QuantitativeRiskAssessmentTechnique .

risk:PersonalSafetyEndangerment a skos:Concept,
        dpv:Concept ;
    dct:created ""^^xsd:date ;
    dct:source <https://www.iso.org/standard/75281.html> ;
    rdfs:isDefinedBy risk: ;
    sw:term_status "accepted"@en ;
    skos:definition ""@en ;
    skos:inScheme risk: ;
    skos:prefLabel "Personal Safety Endangerment"@en ;
    dpv:isSubTypeOf dpv:Harm .

risk:PhysicalAssault a skos:Concept,
        dpv:Concept ;
    dct:created ""^^xsd:date ;
    dct:source <https://www.iso.org/standard/75281.html> ;
    rdfs:isDefinedBy risk: ;
    sw:term_status "accepted"@en ;
    skos:definition ""@en ;
    skos:inScheme risk: ;
    skos:prefLabel "Physical Assault"@en ;
    dpv:isSubTypeOf dpv:Harm .

risk:PhysicalSpying a skos:Concept,
        dpv:Concept ;
    dct:created ""^^xsd:date ;
    dct:source <https://www.iso.org/standard/75281.html> ;
    rdfs:isDefinedBy risk: ;
    sw:term_status "accepted"@en ;
    skos:definition ""@en ;
    skos:inScheme risk: ;
    skos:prefLabel "Physical Spying"@en ;
    dpv:isSubTypeOf dpv:NonMaterialDamage .

risk:PhysicalStalking a skos:Concept,
        dpv:Concept ;
    dct:created ""^^xsd:date ;
    dct:source <https://www.iso.org/standard/75281.html> ;
    rdfs:isDefinedBy risk: ;
    sw:term_status "accepted"@en ;
    skos:definition ""@en ;
    skos:inScheme risk: ;
    skos:prefLabel "Physical Stalking"@en ;
    dpv:isSubTypeOf dpv:NonMaterialDamage .

risk:PsychologicalHarm a skos:Concept,
        dpv:Concept ;
    dct:created ""^^xsd:date ;
    rdfs:isDefinedBy risk: ;
    sw:term_status "accepted"@en ;
    skos:definition ""@en ;
    skos:inScheme risk: ;
    skos:prefLabel "Psychological Harm"@en ;
    dpv:isSubTypeOf dpv:Harm .

risk:PublicOrderBreach a skos:Concept,
        dpv:Concept ;
    dct:created ""^^xsd:date ;
    dct:source <https://www.iso.org/standard/75281.html> ;
    rdfs:isDefinedBy risk: ;
    sw:term_status "accepted"@en ;
    skos:definition ""@en ;
    skos:inScheme risk: ;
    skos:prefLabel "Public Order Breach"@en ;
    dpv:isSubTypeOf dpv:Damage .

risk:RM3x3 a skos:Concept,
        dpv:Concept ;
    dct:created ""^^xsd:date ;
    rdfs:isDefinedBy risk: ;
    sw:term_status "accepted"@en ;
    skos:definition "A Risk Matrix with 3 Likelihood, 3 Severity, and 3 Risk Level types"@en ;
    skos:inScheme risk: ;
    skos:prefLabel "Risk Matrix 3x3"@en ;
    dpv:isSubTypeOf risk:RiskMatrix .

risk:RM3x3R1C1 a skos:Concept,
        dpv:Concept ;
    dct:created ""^^xsd:date ;
    rdfs:isDefinedBy risk: ;
    sw:term_status "accepted"@en ;
    skos:definition "Node (row: 1 col: 1) in 3x3 risk matrix with Risk Level: Low Severity: Low and Likelihood: Low"@en ;
    skos:inScheme risk: ;
    skos:prefLabel "Low Risk"@en ;
    skos:related "hasLikelihood"^^xsd:string,
        "hasRiskLevel"^^xsd:string,
        "hasSeverity"^^xsd:string ;
    dpv:isInstanceOf risk:RiskMatrix3x3 .

risk:RM3x3R1C2 a skos:Concept,
        dpv:Concept ;
    dct:created ""^^xsd:date ;
    rdfs:isDefinedBy risk: ;
    sw:term_status "accepted"@en ;
    skos:definition "Node (row: 1 col: 2) in 3x3 risk matrix with Risk Level: Low Severity: Moderate and Likelihood: Low"@en ;
    skos:inScheme risk: ;
    skos:prefLabel "Low Risk"@en ;
    dpv:isInstanceOf risk:RiskMatrix3x3 .

risk:RM3x3R1C3 a skos:Concept,
        dpv:Concept ;
    dct:created ""^^xsd:date ;
    rdfs:isDefinedBy risk: ;
    sw:term_status "accepted"@en ;
    skos:definition "Node (row: 1 col: 3) in 3x3 risk matrix with Risk Level: Moderate Severity: High and Likelihood: Low"@en ;
    skos:inScheme risk: ;
    skos:prefLabel "Moderate Risk"@en ;
    dpv:isInstanceOf risk:RiskMatrix3x3 .

risk:RM3x3R2C1 a skos:Concept,
        dpv:Concept ;
    dct:created ""^^xsd:date ;
    rdfs:isDefinedBy risk: ;
    sw:term_status "accepted"@en ;
    skos:definition "Node (row: 2 col: 1) in 3x3 risk matrix with Risk Level: Low Severity: Low and Likelihood: Moderate"@en ;
    skos:inScheme risk: ;
    skos:prefLabel "Low Risk"@en ;
    dpv:isInstanceOf risk:RiskMatrix3x3 .

risk:RM3x3R2C2 a skos:Concept,
        dpv:Concept ;
    dct:created ""^^xsd:date ;
    rdfs:isDefinedBy risk: ;
    sw:term_status "accepted"@en ;
    skos:definition "Node (row: 2 col: 2) in 3x3 risk matrix with Risk Level: Moderate Severity: Moderate and Likelihood: Moderate"@en ;
    skos:inScheme risk: ;
    skos:prefLabel "Moderate Risk"@en ;
    dpv:isInstanceOf risk:RiskMatrix3x3 .

risk:RM3x3R2C3 a skos:Concept,
        dpv:Concept ;
    dct:created ""^^xsd:date ;
    rdfs:isDefinedBy risk: ;
    sw:term_status "accepted"@en ;
    skos:definition "Node (row: 2 col: 3) in 3x3 risk matrix with Risk Level: High Severity: High and Likelihood: Moderate"@en ;
    skos:inScheme risk: ;
    skos:prefLabel "High Risk"@en ;
    dpv:isInstanceOf risk:RiskMatrix3x3 .

risk:RM3x3R3C1 a skos:Concept,
        dpv:Concept ;
    dct:created ""^^xsd:date ;
    rdfs:isDefinedBy risk: ;
    sw:term_status "accepted"@en ;
    skos:definition "Node (row: 3 col: 1) in 3x3 risk matrix with Risk Level: Moderate Severity: Low and Likelihood: High"@en ;
    skos:inScheme risk: ;
    skos:prefLabel "Moderate Risk"@en ;
    dpv:isInstanceOf risk:RiskMatrix3x3 .

risk:RM3x3R3C2 a skos:Concept,
        dpv:Concept ;
    dct:created ""^^xsd:date ;
    rdfs:isDefinedBy risk: ;
    sw:term_status "accepted"@en ;
    skos:definition "Node (row: 3 col: 2) in 3x3 risk matrix with Risk Level: High Severity: Moderate and Likelihood: High"@en ;
    skos:inScheme risk: ;
    skos:prefLabel "High Risk"@en ;
    dpv:isInstanceOf risk:RiskMatrix3x3 .

risk:RM3x3R3C3 a skos:Concept,
        dpv:Concept ;
    dct:created ""^^xsd:date ;
    rdfs:isDefinedBy risk: ;
    sw:term_status "accepted"@en ;
    skos:definition "Node (row: 3 col: 3) in 3x3 risk matrix with Risk Level: High Severity: High and Likelihood: High"@en ;
    skos:inScheme risk: ;
    skos:prefLabel "High Risk"@en ;
    dpv:isInstanceOf risk:RiskMatrix3x3 .

risk:RM5x5 a skos:Concept,
        dpv:Concept ;
    dct:created ""^^xsd:date ;
    rdfs:isDefinedBy risk: ;
    sw:term_status "accepted"@en ;
    skos:definition "A Risk Matrix with 5 Likelihood, 5 Severity, and 5 Risk Level types"@en ;
    skos:inScheme risk: ;
    skos:prefLabel "Risk Matrix 5x5"@en ;
    dpv:isSubTypeOf risk:RiskMatrix .

risk:RM5x5R1C1 a skos:Concept,
        dpv:Concept ;
    dct:created ""^^xsd:date ;
    rdfs:isDefinedBy risk: ;
    sw:term_status "accepted"@en ;
    skos:definition "Node (row: 1 col: 1) in 5x5 risk matrix with Risk Level: VeryLow Severity: VeryLow and Likelihood: VeryLow"@en ;
    skos:inScheme risk: ;
    skos:prefLabel "Very Low Risk"@en ;
    dpv:isInstanceOf risk:RiskMatrix5x5 .

risk:RM5x5R1C2 a skos:Concept,
        dpv:Concept ;
    dct:created ""^^xsd:date ;
    rdfs:isDefinedBy risk: ;
    sw:term_status "accepted"@en ;
    skos:definition "Node (row: 1 col: 2) in 5x5 risk matrix with Risk Level: VeryLow Severity: Low and Likelihood: VeryLow"@en ;
    skos:inScheme risk: ;
    skos:prefLabel "Very Low Risk"@en ;
    dpv:isInstanceOf risk:RiskMatrix5x5 .

risk:RM5x5R1C3 a skos:Concept,
        dpv:Concept ;
    dct:created ""^^xsd:date ;
    rdfs:isDefinedBy risk: ;
    sw:term_status "accepted"@en ;
    skos:definition "Node (row: 1 col: 3) in 5x5 risk matrix with Risk Level: VeryLow Severity: Moderate and Likelihood: VeryLow"@en ;
    skos:inScheme risk: ;
    skos:prefLabel "Very Low Risk"@en ;
    dpv:isInstanceOf risk:RiskMatrix5x5 .

risk:RM5x5R1C4 a skos:Concept,
        dpv:Concept ;
    dct:created ""^^xsd:date ;
    rdfs:isDefinedBy risk: ;
    sw:term_status "accepted"@en ;
    skos:definition "Node (row: 1 col: 4) in 5x5 risk matrix with Risk Level: Low Severity: High and Likelihood: VeryLow"@en ;
    skos:inScheme risk: ;
    skos:prefLabel "Low Risk"@en ;
    dpv:isInstanceOf risk:RiskMatrix5x5 .

risk:RM5x5R1C5 a skos:Concept,
        dpv:Concept ;
    dct:created ""^^xsd:date ;
    rdfs:isDefinedBy risk: ;
    sw:term_status "accepted"@en ;
    skos:definition "Node (row: 1 col: 5) in 5x5 risk matrix with Risk Level: Low Severity: VeryHigh and Likelihood: VeryLow"@en ;
    skos:inScheme risk: ;
    skos:prefLabel "Low Risk"@en ;
    dpv:isInstanceOf risk:RiskMatrix5x5 .

risk:RM5x5R2C1 a skos:Concept,
        dpv:Concept ;
    dct:created ""^^xsd:date ;
    rdfs:isDefinedBy risk: ;
    sw:term_status "accepted"@en ;
    skos:definition "Node (row: 2 col: 1) in 5x5 risk matrix with Risk Level: VeryLow Severity: VeryLow and Likelihood: Low"@en ;
    skos:inScheme risk: ;
    skos:prefLabel "Very Low Risk"@en ;
    dpv:isInstanceOf risk:RiskMatrix5x5 .

risk:RM5x5R2C2 a skos:Concept,
        dpv:Concept ;
    dct:created ""^^xsd:date ;
    rdfs:isDefinedBy risk: ;
    sw:term_status "accepted"@en ;
    skos:definition "Node (row: 2 col: 2) in 5x5 risk matrix with Risk Level: Low Severity: Low and Likelihood: Low"@en ;
    skos:inScheme risk: ;
    skos:prefLabel "Low Risk"@en ;
    dpv:isInstanceOf risk:RiskMatrix5x5 .

risk:RM5x5R2C3 a skos:Concept,
        dpv:Concept ;
    dct:created ""^^xsd:date ;
    rdfs:isDefinedBy risk: ;
    sw:term_status "accepted"@en ;
    skos:definition "Node (row: 2 col: 3) in 5x5 risk matrix with Risk Level: Moderate Severity: Moderate and Likelihood: Low"@en ;
    skos:inScheme risk: ;
    skos:prefLabel "Moderate Risk"@en ;
    dpv:isInstanceOf risk:RiskMatrix5x5 .

risk:RM5x5R2C4 a skos:Concept,
        dpv:Concept ;
    dct:created ""^^xsd:date ;
    rdfs:isDefinedBy risk: ;
    sw:term_status "accepted"@en ;
    skos:definition "Node (row: 2 col: 4) in 5x5 risk matrix with Risk Level: Moderate Severity: High and Likelihood: Low"@en ;
    skos:inScheme risk: ;
    skos:prefLabel "Moderate Risk"@en ;
    dpv:isInstanceOf risk:RiskMatrix5x5 .

risk:RM5x5R2C5 a skos:Concept,
        dpv:Concept ;
    dct:created ""^^xsd:date ;
    rdfs:isDefinedBy risk: ;
    sw:term_status "accepted"@en ;
    skos:definition "Node (row: 2 col: 5) in 5x5 risk matrix with Risk Level: High Severity: VeryHigh and Likelihood: Low"@en ;
    skos:inScheme risk: ;
    skos:prefLabel "High Risk"@en ;
    dpv:isInstanceOf risk:RiskMatrix5x5 .

risk:RM5x5R3C1 a skos:Concept,
        dpv:Concept ;
    dct:created ""^^xsd:date ;
    rdfs:isDefinedBy risk: ;
    sw:term_status "accepted"@en ;
    skos:definition "Node (row: 3 col: 1) in 5x5 risk matrix with Risk Level: VeryLow Severity: VeryLow and Likelihood: Moderate"@en ;
    skos:inScheme risk: ;
    skos:prefLabel "Very Low Risk"@en ;
    dpv:isInstanceOf risk:RiskMatrix5x5 .

risk:RM5x5R3C2 a skos:Concept,
        dpv:Concept ;
    dct:created ""^^xsd:date ;
    rdfs:isDefinedBy risk: ;
    sw:term_status "accepted"@en ;
    skos:definition "Node (row: 3 col: 2) in 5x5 risk matrix with Risk Level: Moderate Severity: Low and Likelihood: Moderate"@en ;
    skos:inScheme risk: ;
    skos:prefLabel "Moderate Risk"@en ;
    dpv:isInstanceOf risk:RiskMatrix5x5 .

risk:RM5x5R3C3 a skos:Concept,
        dpv:Concept ;
    dct:created ""^^xsd:date ;
    rdfs:isDefinedBy risk: ;
    sw:term_status "accepted"@en ;
    skos:definition "Node (row: 3 col: 3) in 5x5 risk matrix with Risk Level: Moderate Severity: Moderate and Likelihood: Moderate"@en ;
    skos:inScheme risk: ;
    skos:prefLabel "Moderate Risk"@en ;
    dpv:isInstanceOf risk:RiskMatrix5x5 .

risk:RM5x5R3C4 a skos:Concept,
        dpv:Concept ;
    dct:created ""^^xsd:date ;
    rdfs:isDefinedBy risk: ;
    sw:term_status "accepted"@en ;
    skos:definition "Node (row: 3 col: 4) in 5x5 risk matrix with Risk Level: High Severity: High and Likelihood: Moderate"@en ;
    skos:inScheme risk: ;
    skos:prefLabel "High Risk"@en ;
    dpv:isInstanceOf risk:RiskMatrix5x5 .

risk:RM5x5R3C5 a skos:Concept,
        dpv:Concept ;
    dct:created ""^^xsd:date ;
    rdfs:isDefinedBy risk: ;
    sw:term_status "accepted"@en ;
    skos:definition "Node (row: 3 col: 5) in 5x5 risk matrix with Risk Level: High Severity: VeryHigh and Likelihood: Moderate"@en ;
    skos:inScheme risk: ;
    skos:prefLabel "High Risk"@en ;
    dpv:isInstanceOf risk:RiskMatrix5x5 .

risk:RM5x5R4C1 a skos:Concept,
        dpv:Concept ;
    dct:created ""^^xsd:date ;
    rdfs:isDefinedBy risk: ;
    sw:term_status "accepted"@en ;
    skos:definition "Node (row: 4 col: 1) in 5x5 risk matrix with Risk Level: Low Severity: VeryLow and Likelihood: High"@en ;
    skos:inScheme risk: ;
    skos:prefLabel "Low Risk"@en ;
    dpv:isInstanceOf risk:RiskMatrix5x5 .

risk:RM5x5R4C2 a skos:Concept,
        dpv:Concept ;
    dct:created ""^^xsd:date ;
    rdfs:isDefinedBy risk: ;
    sw:term_status "accepted"@en ;
    skos:definition "Node (row: 4 col: 2) in 5x5 risk matrix with Risk Level: Moderate Severity: Low and Likelihood: High"@en ;
    skos:inScheme risk: ;
    skos:prefLabel "Moderate Risk"@en ;
    dpv:isInstanceOf risk:RiskMatrix5x5 .

risk:RM5x5R4C3 a skos:Concept,
        dpv:Concept ;
    dct:created ""^^xsd:date ;
    rdfs:isDefinedBy risk: ;
    sw:term_status "accepted"@en ;
    skos:definition "Node (row: 4 col: 3) in 5x5 risk matrix with Risk Level: High Severity: Moderate and Likelihood: High"@en ;
    skos:inScheme risk: ;
    skos:prefLabel "High Risk"@en ;
    dpv:isInstanceOf risk:RiskMatrix5x5 .

risk:RM5x5R4C4 a skos:Concept,
        dpv:Concept ;
    dct:created ""^^xsd:date ;
    rdfs:isDefinedBy risk: ;
    sw:term_status "accepted"@en ;
    skos:definition "Node (row: 4 col: 4) in 5x5 risk matrix with Risk Level: VeryHigh Severity: High and Likelihood: High"@en ;
    skos:inScheme risk: ;
    skos:prefLabel "Very High Risk"@en ;
    dpv:isInstanceOf risk:RiskMatrix5x5 .

risk:RM5x5R4C5 a skos:Concept,
        dpv:Concept ;
    dct:created ""^^xsd:date ;
    rdfs:isDefinedBy risk: ;
    sw:term_status "accepted"@en ;
    skos:definition "Node (row: 4 col: 5) in 5x5 risk matrix with Risk Level: VeryHigh Severity: VeryHigh and Likelihood: High"@en ;
    skos:inScheme risk: ;
    skos:prefLabel "Very High Risk"@en ;
    dpv:isInstanceOf risk:RiskMatrix5x5 .

risk:RM5x5R5C1 a skos:Concept,
        dpv:Concept ;
    dct:created ""^^xsd:date ;
    rdfs:isDefinedBy risk: ;
    sw:term_status "accepted"@en ;
    skos:definition "Node (row: 5 col: 1) in 5x5 risk matrix with Risk Level: Low Severity: VeryLow and Likelihood: VeryHigh"@en ;
    skos:inScheme risk: ;
    skos:prefLabel "Low Risk"@en ;
    dpv:isInstanceOf risk:RiskMatrix5x5 .

risk:RM5x5R5C2 a skos:Concept,
        dpv:Concept ;
    dct:created ""^^xsd:date ;
    rdfs:isDefinedBy risk: ;
    sw:term_status "accepted"@en ;
    skos:definition "Node (row: 5 col: 2) in 5x5 risk matrix with Risk Level: High Severity: Low and Likelihood: VeryHigh"@en ;
    skos:inScheme risk: ;
    skos:prefLabel "High Risk"@en ;
    dpv:isInstanceOf risk:RiskMatrix5x5 .

risk:RM5x5R5C3 a skos:Concept,
        dpv:Concept ;
    dct:created ""^^xsd:date ;
    rdfs:isDefinedBy risk: ;
    sw:term_status "accepted"@en ;
    skos:definition "Node (row: 5 col: 3) in 5x5 risk matrix with Risk Level: VeryHigh Severity: Moderate and Likelihood: VeryHigh"@en ;
    skos:inScheme risk: ;
    skos:prefLabel "Very High Risk"@en ;
    dpv:isInstanceOf risk:RiskMatrix5x5 .

risk:RM5x5R5C4 a skos:Concept,
        dpv:Concept ;
    dct:created ""^^xsd:date ;
    rdfs:isDefinedBy risk: ;
    sw:term_status "accepted"@en ;
    skos:definition "Node (row: 5 col: 4) in 5x5 risk matrix with Risk Level: VeryHigh Severity: High and Likelihood: VeryHigh"@en ;
    skos:inScheme risk: ;
    skos:prefLabel "Very High Risk"@en ;
    dpv:isInstanceOf risk:RiskMatrix5x5 .

risk:RM5x5R5C5 a skos:Concept,
        dpv:Concept ;
    dct:created ""^^xsd:date ;
    rdfs:isDefinedBy risk: ;
    sw:term_status "accepted"@en ;
    skos:definition "Node (row: 5 col: 5) in 5x5 risk matrix with Risk Level: VeryHigh Severity: VeryHigh and Likelihood: VeryHigh"@en ;
    skos:inScheme risk: ;
    skos:prefLabel "Very High Risk"@en ;
    dpv:isInstanceOf risk:RiskMatrix5x5 .

risk:RM7x7 a skos:Concept,
        dpv:Concept ;
    dct:created ""^^xsd:date ;
    rdfs:isDefinedBy risk: ;
    sw:term_status "accepted"@en ;
    skos:definition "A Risk Matrix with 7 Likelihood, 7 Severity, and 7 Risk Level types"@en ;
    skos:inScheme risk: ;
    skos:prefLabel "Risk Matrix 7x7"@en ;
    dpv:isSubTypeOf risk:RiskMatrix .

risk:RM7x7R1C1 a skos:Concept,
        dpv:Concept ;
    dct:created ""^^xsd:date ;
    rdfs:isDefinedBy risk: ;
    sw:term_status "accepted"@en ;
    skos:definition "Node (row: 1 col: 1) in 7x7 risk matrix with Risk Level: ExtremelyLow Severity: ExtremelyLow and Likelihood: ExtremelyLow"@en ;
    skos:inScheme risk: ;
    skos:prefLabel "Extremely Low Risk"@en ;
    dpv:isInstanceOf risk:RiskMatrix7x7 .

risk:RM7x7R1C2 a skos:Concept,
        dpv:Concept ;
    dct:created ""^^xsd:date ;
    rdfs:isDefinedBy risk: ;
    sw:term_status "accepted"@en ;
    skos:definition "Node (row: 1 col: 2) in 7x7 risk matrix with Risk Level: ExtremelyLow Severity: VeryLow and Likelihood: ExtremelyLow"@en ;
    skos:inScheme risk: ;
    skos:prefLabel "Extremely Low Risk"@en ;
    dpv:isInstanceOf risk:RiskMatrix7x7 .

risk:RM7x7R1C3 a skos:Concept,
        dpv:Concept ;
    dct:created ""^^xsd:date ;
    rdfs:isDefinedBy risk: ;
    sw:term_status "accepted"@en ;
    skos:definition "Node (row: 1 col: 3) in 7x7 risk matrix with Risk Level: ExtremelyLow Severity: Low and Likelihood: ExtremelyLow"@en ;
    skos:inScheme risk: ;
    skos:prefLabel "Extremely Low Risk"@en ;
    dpv:isInstanceOf risk:RiskMatrix7x7 .

risk:RM7x7R1C4 a skos:Concept,
        dpv:Concept ;
    dct:created ""^^xsd:date ;
    rdfs:isDefinedBy risk: ;
    sw:term_status "accepted"@en ;
    skos:definition "Node (row: 1 col: 4) in 7x7 risk matrix with Risk Level: ExtremelyLow Severity: Moderate and Likelihood: ExtremelyLow"@en ;
    skos:inScheme risk: ;
    skos:prefLabel "Extremely Low Risk"@en ;
    dpv:isInstanceOf risk:RiskMatrix7x7 .

risk:RM7x7R1C5 a skos:Concept,
        dpv:Concept ;
    dct:created ""^^xsd:date ;
    rdfs:isDefinedBy risk: ;
    sw:term_status "accepted"@en ;
    skos:definition "Node (row: 1 col: 5) in 7x7 risk matrix with Risk Level: VeryLow Severity: High and Likelihood: ExtremelyLow"@en ;
    skos:inScheme risk: ;
    skos:prefLabel "Very Low Risk"@en ;
    dpv:isInstanceOf risk:RiskMatrix7x7 .

risk:RM7x7R1C6 a skos:Concept,
        dpv:Concept ;
    dct:created ""^^xsd:date ;
    rdfs:isDefinedBy risk: ;
    sw:term_status "accepted"@en ;
    skos:definition "Node (row: 1 col: 6) in 7x7 risk matrix with Risk Level: VeryLow Severity: VeryHigh and Likelihood: ExtremelyLow"@en ;
    skos:inScheme risk: ;
    skos:prefLabel "Very Low Risk"@en ;
    dpv:isInstanceOf risk:RiskMatrix7x7 .

risk:RM7x7R1C7 a skos:Concept,
        dpv:Concept ;
    dct:created ""^^xsd:date ;
    rdfs:isDefinedBy risk: ;
    sw:term_status "accepted"@en ;
    skos:definition "Node (row: 1 col: 7) in 7x7 risk matrix with Risk Level: Low Severity: ExtremelyHigh and Likelihood: ExtremelyLow"@en ;
    skos:inScheme risk: ;
    skos:prefLabel "Low Risk"@en ;
    dpv:isInstanceOf risk:RiskMatrix7x7 .

risk:RM7x7R2C1 a skos:Concept,
        dpv:Concept ;
    dct:created ""^^xsd:date ;
    rdfs:isDefinedBy risk: ;
    sw:term_status "accepted"@en ;
    skos:definition "Node (row: 2 col: 1) in 7x7 risk matrix with Risk Level: ExtremelyLow Severity: ExtremelyLow and Likelihood: VeryLow"@en ;
    skos:inScheme risk: ;
    skos:prefLabel "Extremely Low Risk"@en ;
    dpv:isInstanceOf risk:RiskMatrix7x7 .

risk:RM7x7R2C2 a skos:Concept,
        dpv:Concept ;
    dct:created ""^^xsd:date ;
    rdfs:isDefinedBy risk: ;
    sw:term_status "accepted"@en ;
    skos:definition "Node (row: 2 col: 2) in 7x7 risk matrix with Risk Level: ExtremelyLow Severity: VeryLow and Likelihood: VeryLow"@en ;
    skos:inScheme risk: ;
    skos:prefLabel "Extremely Low Risk"@en ;
    dpv:isInstanceOf risk:RiskMatrix7x7 .

risk:RM7x7R2C3 a skos:Concept,
        dpv:Concept ;
    dct:created ""^^xsd:date ;
    rdfs:isDefinedBy risk: ;
    sw:term_status "accepted"@en ;
    skos:definition "Node (row: 2 col: 3) in 7x7 risk matrix with Risk Level: VeryLow Severity: Low and Likelihood: VeryLow"@en ;
    skos:inScheme risk: ;
    skos:prefLabel "Very Low Risk"@en ;
    dpv:isInstanceOf risk:RiskMatrix7x7 .

risk:RM7x7R2C4 a skos:Concept,
        dpv:Concept ;
    dct:created ""^^xsd:date ;
    rdfs:isDefinedBy risk: ;
    sw:term_status "accepted"@en ;
    skos:definition "Node (row: 2 col: 4) in 7x7 risk matrix with Risk Level: Low Severity: Moderate and Likelihood: VeryLow"@en ;
    skos:inScheme risk: ;
    skos:prefLabel "Low Risk"@en ;
    dpv:isInstanceOf risk:RiskMatrix7x7 .

risk:RM7x7R2C5 a skos:Concept,
        dpv:Concept ;
    dct:created ""^^xsd:date ;
    rdfs:isDefinedBy risk: ;
    sw:term_status "accepted"@en ;
    skos:definition "Node (row: 2 col: 5) in 7x7 risk matrix with Risk Level: Low Severity: High and Likelihood: VeryLow"@en ;
    skos:inScheme risk: ;
    skos:prefLabel "Low Risk"@en ;
    dpv:isInstanceOf risk:RiskMatrix7x7 .

risk:RM7x7R2C6 a skos:Concept,
        dpv:Concept ;
    dct:created ""^^xsd:date ;
    rdfs:isDefinedBy risk: ;
    sw:term_status "accepted"@en ;
    skos:definition "Node (row: 2 col: 6) in 7x7 risk matrix with Risk Level: Moderate Severity: VeryHigh and Likelihood: VeryLow"@en ;
    skos:inScheme risk: ;
    skos:prefLabel "Moderate Risk"@en ;
    dpv:isInstanceOf risk:RiskMatrix7x7 .

risk:RM7x7R2C7 a skos:Concept,
        dpv:Concept ;
    dct:created ""^^xsd:date ;
    rdfs:isDefinedBy risk: ;
    sw:term_status "accepted"@en ;
    skos:definition "Node (row: 2 col: 7) in 7x7 risk matrix with Risk Level: Moderate Severity: ExtremelyHigh and Likelihood: VeryLow"@en ;
    skos:inScheme risk: ;
    skos:prefLabel "Moderate Risk"@en ;
    dpv:isInstanceOf risk:RiskMatrix7x7 .

risk:RM7x7R3C1 a skos:Concept,
        dpv:Concept ;
    dct:created ""^^xsd:date ;
    rdfs:isDefinedBy risk: ;
    sw:term_status "accepted"@en ;
    skos:definition "Node (row: 3 col: 1) in 7x7 risk matrix with Risk Level: ExtremelyLow Severity: ExtremelyLow and Likelihood: Low"@en ;
    skos:inScheme risk: ;
    skos:prefLabel "Extremely Low Risk"@en ;
    dpv:isInstanceOf risk:RiskMatrix7x7 .

risk:RM7x7R3C2 a skos:Concept,
        dpv:Concept ;
    dct:created ""^^xsd:date ;
    rdfs:isDefinedBy risk: ;
    sw:term_status "accepted"@en ;
    skos:definition "Node (row: 3 col: 2) in 7x7 risk matrix with Risk Level: VeryLow Severity: VeryLow and Likelihood: Low"@en ;
    skos:inScheme risk: ;
    skos:prefLabel "Very Low Risk"@en ;
    dpv:isInstanceOf risk:RiskMatrix7x7 .

risk:RM7x7R3C3 a skos:Concept,
        dpv:Concept ;
    dct:created ""^^xsd:date ;
    rdfs:isDefinedBy risk: ;
    sw:term_status "accepted"@en ;
    skos:definition "Node (row: 3 col: 3) in 7x7 risk matrix with Risk Level: Low Severity: Low and Likelihood: Low"@en ;
    skos:inScheme risk: ;
    skos:prefLabel "Low Risk"@en ;
    dpv:isInstanceOf risk:RiskMatrix7x7 .

risk:RM7x7R3C4 a skos:Concept,
        dpv:Concept ;
    dct:created ""^^xsd:date ;
    rdfs:isDefinedBy risk: ;
    sw:term_status "accepted"@en ;
    skos:definition "Node (row: 3 col: 4) in 7x7 risk matrix with Risk Level: Moderate Severity: Moderate and Likelihood: Low"@en ;
    skos:inScheme risk: ;
    skos:prefLabel "Moderate Risk"@en ;
    dpv:isInstanceOf risk:RiskMatrix7x7 .

risk:RM7x7R3C5 a skos:Concept,
        dpv:Concept ;
    dct:created ""^^xsd:date ;
    rdfs:isDefinedBy risk: ;
    sw:term_status "accepted"@en ;
    skos:definition "Node (row: 3 col: 5) in 7x7 risk matrix with Risk Level: Moderate Severity: High and Likelihood: Low"@en ;
    skos:inScheme risk: ;
    skos:prefLabel "Moderate Risk"@en ;
    dpv:isInstanceOf risk:RiskMatrix7x7 .

risk:RM7x7R3C6 a skos:Concept,
        dpv:Concept ;
    dct:created ""^^xsd:date ;
    rdfs:isDefinedBy risk: ;
    sw:term_status "accepted"@en ;
    skos:definition "Node (row: 3 col: 6) in 7x7 risk matrix with Risk Level: High Severity: VeryHigh and Likelihood: Low"@en ;
    skos:inScheme risk: ;
    skos:prefLabel "High Risk"@en ;
    dpv:isInstanceOf risk:RiskMatrix7x7 .

risk:RM7x7R3C7 a skos:Concept,
        dpv:Concept ;
    dct:created ""^^xsd:date ;
    rdfs:isDefinedBy risk: ;
    sw:term_status "accepted"@en ;
    skos:definition "Node (row: 3 col: 7) in 7x7 risk matrix with Risk Level: High Severity: ExtremelyHigh and Likelihood: Low"@en ;
    skos:inScheme risk: ;
    skos:prefLabel "High Risk"@en ;
    dpv:isInstanceOf risk:RiskMatrix7x7 .

risk:RM7x7R4C1 a skos:Concept,
        dpv:Concept ;
    dct:created ""^^xsd:date ;
    rdfs:isDefinedBy risk: ;
    sw:term_status "accepted"@en ;
    skos:definition "Node (row: 4 col: 1) in 7x7 risk matrix with Risk Level: VeryLow Severity: ExtremelyLow and Likelihood: Moderate"@en ;
    skos:inScheme risk: ;
    skos:prefLabel "Very Low Risk"@en ;
    dpv:isInstanceOf risk:RiskMatrix7x7 .

risk:RM7x7R4C2 a skos:Concept,
        dpv:Concept ;
    dct:created ""^^xsd:date ;
    rdfs:isDefinedBy risk: ;
    sw:term_status "accepted"@en ;
    skos:definition "Node (row: 4 col: 2) in 7x7 risk matrix with Risk Level: Low Severity: VeryLow and Likelihood: Moderate"@en ;
    skos:inScheme risk: ;
    skos:prefLabel "Low Risk"@en ;
    dpv:isInstanceOf risk:RiskMatrix7x7 .

risk:RM7x7R4C3 a skos:Concept,
        dpv:Concept ;
    dct:created ""^^xsd:date ;
    rdfs:isDefinedBy risk: ;
    sw:term_status "accepted"@en ;
    skos:definition "Node (row: 4 col: 3) in 7x7 risk matrix with Risk Level: Moderate Severity: Low and Likelihood: Moderate"@en ;
    skos:inScheme risk: ;
    skos:prefLabel "Moderate Risk"@en ;
    dpv:isInstanceOf risk:RiskMatrix7x7 .

risk:RM7x7R4C4 a skos:Concept,
        dpv:Concept ;
    dct:created ""^^xsd:date ;
    rdfs:isDefinedBy risk: ;
    sw:term_status "accepted"@en ;
    skos:definition "Node (row: 4 col: 4) in 7x7 risk matrix with Risk Level: High Severity: Moderate and Likelihood: Moderate"@en ;
    skos:inScheme risk: ;
    skos:prefLabel "High Risk"@en ;
    dpv:isInstanceOf risk:RiskMatrix7x7 .

risk:RM7x7R4C5 a skos:Concept,
        dpv:Concept ;
    dct:created ""^^xsd:date ;
    rdfs:isDefinedBy risk: ;
    sw:term_status "accepted"@en ;
    skos:definition "Node (row: 4 col: 5) in 7x7 risk matrix with Risk Level: High Severity: High and Likelihood: Moderate"@en ;
    skos:inScheme risk: ;
    skos:prefLabel "High Risk"@en ;
    dpv:isInstanceOf risk:RiskMatrix7x7 .

risk:RM7x7R4C6 a skos:Concept,
        dpv:Concept ;
    dct:created ""^^xsd:date ;
    rdfs:isDefinedBy risk: ;
    sw:term_status "accepted"@en ;
    skos:definition "Node (row: 4 col: 6) in 7x7 risk matrix with Risk Level: VeryHigh Severity: VeryHigh and Likelihood: Moderate"@en ;
    skos:inScheme risk: ;
    skos:prefLabel "Very High Risk"@en ;
    dpv:isInstanceOf risk:RiskMatrix7x7 .

risk:RM7x7R4C7 a skos:Concept,
        dpv:Concept ;
    dct:created ""^^xsd:date ;
    rdfs:isDefinedBy risk: ;
    sw:term_status "accepted"@en ;
    skos:definition "Node (row: 4 col: 7) in 7x7 risk matrix with Risk Level: VeryHigh Severity: ExtremelyHigh and Likelihood: Moderate"@en ;
    skos:inScheme risk: ;
    skos:prefLabel "Very High Risk"@en ;
    dpv:isInstanceOf risk:RiskMatrix7x7 .

risk:RM7x7R5C1 a skos:Concept,
        dpv:Concept ;
    dct:created ""^^xsd:date ;
    rdfs:isDefinedBy risk: ;
    sw:term_status "accepted"@en ;
    skos:definition "Node (row: 5 col: 1) in 7x7 risk matrix with Risk Level: VeryLow Severity: ExtremelyLow and Likelihood: High"@en ;
    skos:inScheme risk: ;
    skos:prefLabel "Very Low Risk"@en ;
    dpv:isInstanceOf risk:RiskMatrix7x7 .

risk:RM7x7R5C2 a skos:Concept,
        dpv:Concept ;
    dct:created ""^^xsd:date ;
    rdfs:isDefinedBy risk: ;
    sw:term_status "accepted"@en ;
    skos:definition "Node (row: 5 col: 2) in 7x7 risk matrix with Risk Level: Low Severity: VeryLow and Likelihood: High"@en ;
    skos:inScheme risk: ;
    skos:prefLabel "Low Risk"@en ;
    dpv:isInstanceOf risk:RiskMatrix7x7 .

risk:RM7x7R5C3 a skos:Concept,
        dpv:Concept ;
    dct:created ""^^xsd:date ;
    rdfs:isDefinedBy risk: ;
    sw:term_status "accepted"@en ;
    skos:definition "Node (row: 5 col: 3) in 7x7 risk matrix with Risk Level: High Severity: Low and Likelihood: High"@en ;
    skos:inScheme risk: ;
    skos:prefLabel "High Risk"@en ;
    dpv:isInstanceOf risk:RiskMatrix7x7 .

risk:RM7x7R5C4 a skos:Concept,
        dpv:Concept ;
    dct:created ""^^xsd:date ;
    rdfs:isDefinedBy risk: ;
    sw:term_status "accepted"@en ;
    skos:definition "Node (row: 5 col: 4) in 7x7 risk matrix with Risk Level: High Severity: Moderate and Likelihood: High"@en ;
    skos:inScheme risk: ;
    skos:prefLabel "High Risk"@en ;
    dpv:isInstanceOf risk:RiskMatrix7x7 .

risk:RM7x7R5C5 a skos:Concept,
        dpv:Concept ;
    dct:created ""^^xsd:date ;
    rdfs:isDefinedBy risk: ;
    sw:term_status "accepted"@en ;
    skos:definition "Node (row: 5 col: 5) in 7x7 risk matrix with Risk Level: VeryHigh Severity: High and Likelihood: High"@en ;
    skos:inScheme risk: ;
    skos:prefLabel "Very High Risk"@en ;
    dpv:isInstanceOf risk:RiskMatrix7x7 .

risk:RM7x7R5C6 a skos:Concept,
        dpv:Concept ;
    dct:created ""^^xsd:date ;
    rdfs:isDefinedBy risk: ;
    sw:term_status "accepted"@en ;
    skos:definition "Node (row: 5 col: 6) in 7x7 risk matrix with Risk Level: VeryHigh Severity: VeryHigh and Likelihood: High"@en ;
    skos:inScheme risk: ;
    skos:prefLabel "Very High Risk"@en ;
    dpv:isInstanceOf risk:RiskMatrix7x7 .

risk:RM7x7R5C7 a skos:Concept,
        dpv:Concept ;
    dct:created ""^^xsd:date ;
    rdfs:isDefinedBy risk: ;
    sw:term_status "accepted"@en ;
    skos:definition "Node (row: 5 col: 7) in 7x7 risk matrix with Risk Level: ExtremelyHigh Severity: ExtremelyHigh and Likelihood: High"@en ;
    skos:inScheme risk: ;
    skos:prefLabel "Extremely High Risk"@en ;
    dpv:isInstanceOf risk:RiskMatrix7x7 .

risk:RM7x7R6C1 a skos:Concept,
        dpv:Concept ;
    dct:created ""^^xsd:date ;
    rdfs:isDefinedBy risk: ;
    sw:term_status "accepted"@en ;
    skos:definition "Node (row: 6 col: 1) in 7x7 risk matrix with Risk Level: VeryLow Severity: ExtremelyLow and Likelihood: VeryHigh"@en ;
    skos:inScheme risk: ;
    skos:prefLabel "Very Low Risk"@en ;
    dpv:isInstanceOf risk:RiskMatrix7x7 .

risk:RM7x7R6C2 a skos:Concept,
        dpv:Concept ;
    dct:created ""^^xsd:date ;
    rdfs:isDefinedBy risk: ;
    sw:term_status "accepted"@en ;
    skos:definition "Node (row: 6 col: 2) in 7x7 risk matrix with Risk Level: Moderate Severity: VeryLow and Likelihood: VeryHigh"@en ;
    skos:inScheme risk: ;
    skos:prefLabel "Moderate Risk"@en ;
    dpv:isInstanceOf risk:RiskMatrix7x7 .

risk:RM7x7R6C3 a skos:Concept,
        dpv:Concept ;
    dct:created ""^^xsd:date ;
    rdfs:isDefinedBy risk: ;
    sw:term_status "accepted"@en ;
    skos:definition "Node (row: 6 col: 3) in 7x7 risk matrix with Risk Level: High Severity: Low and Likelihood: VeryHigh"@en ;
    skos:inScheme risk: ;
    skos:prefLabel "High Risk"@en ;
    dpv:isInstanceOf risk:RiskMatrix7x7 .

risk:RM7x7R6C4 a skos:Concept,
        dpv:Concept ;
    dct:created ""^^xsd:date ;
    rdfs:isDefinedBy risk: ;
    sw:term_status "accepted"@en ;
    skos:definition "Node (row: 6 col: 4) in 7x7 risk matrix with Risk Level: VeryHigh Severity: Moderate and Likelihood: VeryHigh"@en ;
    skos:inScheme risk: ;
    skos:prefLabel "Very High Risk"@en ;
    dpv:isInstanceOf risk:RiskMatrix7x7 .

risk:RM7x7R6C5 a skos:Concept,
        dpv:Concept ;
    dct:created ""^^xsd:date ;
    rdfs:isDefinedBy risk: ;
    sw:term_status "accepted"@en ;
    skos:definition "Node (row: 6 col: 5) in 7x7 risk matrix with Risk Level: ExtremelyHigh Severity: High and Likelihood: VeryHigh"@en ;
    skos:inScheme risk: ;
    skos:prefLabel "Extremely High Risk"@en ;
    dpv:isInstanceOf risk:RiskMatrix7x7 .

risk:RM7x7R6C6 a skos:Concept,
        dpv:Concept ;
    dct:created ""^^xsd:date ;
    rdfs:isDefinedBy risk: ;
    sw:term_status "accepted"@en ;
    skos:definition "Node (row: 6 col: 6) in 7x7 risk matrix with Risk Level: ExtremelyHigh Severity: VeryHigh and Likelihood: VeryHigh"@en ;
    skos:inScheme risk: ;
    skos:prefLabel "Extremely High Risk"@en ;
    dpv:isInstanceOf risk:RiskMatrix7x7 .

risk:RM7x7R6C7 a skos:Concept,
        dpv:Concept ;
    dct:created ""^^xsd:date ;
    rdfs:isDefinedBy risk: ;
    sw:term_status "accepted"@en ;
    skos:definition "Node (row: 6 col: 7) in 7x7 risk matrix with Risk Level: ExtremelyHigh Severity: ExtremelyHigh and Likelihood: VeryHigh"@en ;
    skos:inScheme risk: ;
    skos:prefLabel "Extremely High Risk"@en ;
    dpv:isInstanceOf risk:RiskMatrix7x7 .

risk:RM7x7R7C1 a skos:Concept,
        dpv:Concept ;
    dct:created ""^^xsd:date ;
    rdfs:isDefinedBy risk: ;
    sw:term_status "accepted"@en ;
    skos:definition "Node (row: 7 col: 1) in 7x7 risk matrix with Risk Level: Low Severity: ExtremelyLow and Likelihood: ExtremelyHigh"@en ;
    skos:inScheme risk: ;
    skos:prefLabel "Low Risk"@en ;
    dpv:isInstanceOf risk:RiskMatrix7x7 .

risk:RM7x7R7C2 a skos:Concept,
        dpv:Concept ;
    dct:created ""^^xsd:date ;
    rdfs:isDefinedBy risk: ;
    sw:term_status "accepted"@en ;
    skos:definition "Node (row: 7 col: 2) in 7x7 risk matrix with Risk Level: Moderate Severity: VeryLow and Likelihood: ExtremelyHigh"@en ;
    skos:inScheme risk: ;
    skos:prefLabel "Moderate Risk"@en ;
    dpv:isInstanceOf risk:RiskMatrix7x7 .

risk:RM7x7R7C3 a skos:Concept,
        dpv:Concept ;
    dct:created ""^^xsd:date ;
    rdfs:isDefinedBy risk: ;
    sw:term_status "accepted"@en ;
    skos:definition "Node (row: 7 col: 3) in 7x7 risk matrix with Risk Level: VeryHigh Severity: Low and Likelihood: ExtremelyHigh"@en ;
    skos:inScheme risk: ;
    skos:prefLabel "Very High Risk"@en ;
    dpv:isInstanceOf risk:RiskMatrix7x7 .

risk:RM7x7R7C4 a skos:Concept,
        dpv:Concept ;
    dct:created ""^^xsd:date ;
    rdfs:isDefinedBy risk: ;
    sw:term_status "accepted"@en ;
    skos:definition "Node (row: 7 col: 4) in 7x7 risk matrix with Risk Level: VeryHigh Severity: Moderate and Likelihood: ExtremelyHigh"@en ;
    skos:inScheme risk: ;
    skos:prefLabel "Very High Risk"@en ;
    dpv:isInstanceOf risk:RiskMatrix7x7 .

risk:RM7x7R7C5 a skos:Concept,
        dpv:Concept ;
    dct:created ""^^xsd:date ;
    rdfs:isDefinedBy risk: ;
    sw:term_status "accepted"@en ;
    skos:definition "Node (row: 7 col: 5) in 7x7 risk matrix with Risk Level: ExtremelyHigh Severity: High and Likelihood: ExtremelyHigh"@en ;
    skos:inScheme risk: ;
    skos:prefLabel "Extremely High Risk"@en ;
    dpv:isInstanceOf risk:RiskMatrix7x7 .

risk:RM7x7R7C6 a skos:Concept,
        dpv:Concept ;
    dct:created ""^^xsd:date ;
    rdfs:isDefinedBy risk: ;
    sw:term_status "accepted"@en ;
    skos:definition "Node (row: 7 col: 6) in 7x7 risk matrix with Risk Level: ExtremelyHigh Severity: VeryHigh and Likelihood: ExtremelyHigh"@en ;
    skos:inScheme risk: ;
    skos:prefLabel "Extremely High Risk"@en ;
    dpv:isInstanceOf risk:RiskMatrix7x7 .

risk:RM7x7R7C7 a skos:Concept,
        dpv:Concept ;
    dct:created ""^^xsd:date ;
    rdfs:isDefinedBy risk: ;
    sw:term_status "accepted"@en ;
    skos:definition "Node (row: 7 col: 7) in 7x7 risk matrix with Risk Level: ExtremelyHigh Severity: ExtremelyHigh and Likelihood: ExtremelyHigh"@en ;
    skos:inScheme risk: ;
    skos:prefLabel "Extremely High Risk"@en ;
    dpv:isInstanceOf risk:RiskMatrix7x7 .

risk:RansomDemand a skos:Concept,
        dpv:Concept ;
    dct:created ""^^xsd:date ;
    dct:source <https://www.iso.org/standard/75281.html> ;
    rdfs:isDefinedBy risk: ;
    sw:term_status "accepted"@en ;
    skos:definition ""@en ;
    skos:inScheme risk: ;
    skos:prefLabel "Ransom Demand"@en ;
    dpv:isSubTypeOf dpv:NonMaterialDamage .

risk:ReduceLikelihood a skos:Concept,
        dpv:Concept ;
    dct:created ""^^xsd:date ;
    rdfs:isDefinedBy risk: ;
    sw:term_status "accepted"@en ;
    skos:definition "Risk Control that reduces the likelihood of an event"@en ;
    skos:inScheme risk: ;
    skos:prefLabel "Reduce Likelihood"@en ;
    dpv:isSubTypeOf dpv:RiskMitigationMeasure .

risk:ReduceSeverity a skos:Concept,
        dpv:Concept ;
    dct:created ""^^xsd:date ;
    rdfs:isDefinedBy risk: ;
    sw:term_status "accepted"@en ;
    skos:definition "Risk Control that reduces the severity of an event"@en ;
    skos:inScheme risk: ;
    skos:prefLabel "Reduce Severity"@en ;
    dpv:isSubTypeOf dpv:RiskMitigationMeasure .

risk:ReliabilityCentredMaintenance a skos:Concept,
        dpv:Concept ;
    dct:created ""^^xsd:date ;
    dct:source <https://www.iso.org/standard/72140.html> ;
    rdfs:isDefinedBy risk: ;
    sw:term_status "accepted"@en ;
    skos:definition "A risk based assessment used to identify the appropriate maintenance tasks for a system and its components."@en ;
    skos:inScheme risk: ;
    skos:prefLabel "Reliability Centred Maintenance"@en ;
    dpv:isInstanceOf risk:QualitativeRiskAssessmentTechnique,
        risk:QuantitativeRiskAssessmentTechnique .

risk:RemoteSpying a skos:Concept,
        dpv:Concept ;
    dct:created ""^^xsd:date ;
    dct:source <https://www.iso.org/standard/75281.html> ;
    rdfs:isDefinedBy risk: ;
    sw:term_status "accepted"@en ;
    skos:definition ""@en ;
    skos:inScheme risk: ;
    skos:prefLabel "Remote Spying"@en ;
    dpv:isSubTypeOf dpv:NonMaterialDamage .

risk:RemoveConsequence a skos:Concept,
        dpv:Concept ;
    dct:created ""^^xsd:date ;
    rdfs:isDefinedBy risk: ;
    sw:term_status "accepted"@en ;
    skos:definition "Risk Control that removes Consequence i.e. prevents it from materialising"@en ;
    skos:inScheme risk: ;
    skos:prefLabel "Remove Consequence"@en ;
    dpv:isSubTypeOf risk:ControlConsequence .

risk:RemoveImpact a skos:Concept,
        dpv:Concept ;
    dct:created ""^^xsd:date ;
    rdfs:isDefinedBy risk: ;
    sw:term_status "accepted"@en ;
    skos:definition "Risk Control that removes Impact i.e. prevents it from materialising"@en ;
    skos:inScheme risk: ;
    skos:prefLabel "Remove Impact"@en ;
    dpv:isSubTypeOf risk:ControlConsequence .

risk:RemoveSource a skos:Concept,
        dpv:Concept ;
    dct:created ""^^xsd:date ;
    rdfs:isDefinedBy risk: ;
    sw:term_status "accepted"@en ;
    skos:definition "Risk Control that removes the risk source"@en ;
    skos:inScheme risk: ;
    skos:prefLabel "Remove Source"@en ;
    dpv:isSubTypeOf risk:ControlRiskSource .

risk:ReplacementCosts a skos:Concept,
        dpv:Concept ;
    dct:created ""^^xsd:date ;
    dct:source <https://www.iso.org/standard/75281.html> ;
    rdfs:isDefinedBy risk: ;
    sw:term_status "accepted"@en ;
    skos:definition ""@en ;
    skos:inScheme risk: ;
    skos:prefLabel "Replacement Costs"@en ;
    dpv:isSubTypeOf dpv:Detriment .

risk:RetrievalDeletedData a skos:Concept,
        dpv:Concept ;
    dct:created ""^^xsd:date ;
    dct:source <https://www.iso.org/standard/75281.html> ;
    rdfs:isDefinedBy risk: ;
    sw:term_status "accepted"@en ;
    skos:definition ""@en ;
    skos:inScheme risk: ;
    skos:prefLabel "Retrieval of Deleted Data"@en ;
    dpv:isSubTypeOf dpv:Detriment .

risk:RetrievalDiscardedEquipment a skos:Concept,
        dpv:Concept ;
    dct:created ""^^xsd:date ;
    dct:source <https://www.iso.org/standard/75281.html> ;
    rdfs:isDefinedBy risk: ;
    sw:term_status "accepted"@en ;
    skos:definition ""@en ;
    skos:inScheme risk: ;
    skos:prefLabel "Retrieval of Discarded Equipment"@en ;
    dpv:isSubTypeOf dpv:Detriment .

risk:RiskIndices a skos:Concept,
        dpv:Concept ;
    dct:created ""^^xsd:date ;
    dct:source <https://www.iso.org/standard/72140.html> ;
    rdfs:isDefinedBy risk: ;
    sw:term_status "accepted"@en ;
    skos:definition "Rates the significance of risks based on ratings applied to factors which are believed to influence the magnitude of the risk."@en ;
    skos:inScheme risk: ;
    skos:prefLabel "Risk Indices"@en ;
    dpv:isInstanceOf risk:QuantitativeRiskAssessmentTechnique .

risk:RiskRegisters a skos:Concept,
        dpv:Concept ;
    dct:created ""^^xsd:date ;
    dct:source <https://www.iso.org/standard/72140.html> ;
    rdfs:isDefinedBy risk: ;
    sw:term_status "accepted"@en ;
    skos:definition "A means of recording information about risks and tracking actions."@en ;
    skos:inScheme risk: ;
    skos:prefLabel "Risk Registers"@en ;
    dpv:isInstanceOf risk:QualitativeRiskAssessmentTechnique .

risk:SCurves a skos:Concept,
        dpv:Concept ;
    dct:created ""^^xsd:date ;
    dct:source <https://www.iso.org/standard/72140.html> ;
    rdfs:isDefinedBy risk: ;
    sw:term_status "accepted"@en ;
    skos:definition "A means of displaying the relationship between consequences and their likelihood plotted as a cumulative distribution function (S-curve)."@en ;
    skos:inScheme risk: ;
    skos:prefLabel "S-curves"@en ;
    dpv:isInstanceOf risk:QuantitativeRiskAssessmentTechnique .

risk:SFAIRP a skos:Concept,
        dpv:Concept ;
    dct:created ""^^xsd:date ;
    dct:source <https://www.iso.org/standard/72140.html> ;
    rdfs:isDefinedBy risk: ;
    sw:term_status "accepted"@en ;
    skos:definition "So far as is Resonably Practiceable (ALARP) - A criteria for deciding significance of risk and means of evaluating tolerability of risk"@en ;
    skos:inScheme risk: ;
    skos:prefLabel "SFAIRP"@en ;
    dpv:isInstanceOf risk:QualitativeRiskAssessmentTechnique,
        risk:QuantitativeRiskAssessmentTechnique .

risk:SWIFT a skos:Concept,
        dpv:Concept ;
    dct:created ""^^xsd:date ;
    dct:source <https://www.iso.org/standard/72140.html> ;
    rdfs:isDefinedBy risk: ;
    sw:term_status "accepted"@en ;
    skos:definition "A simpler form of HAZOP with prompts of \"what if\" to identify deviations from the expected."@en ;
    skos:inScheme risk: ;
    skos:prefLabel "Structured \"What If?\" (SWIFT)"@en ;
    dpv:isInstanceOf risk:QualitativeRiskAssessmentTechnique .

risk:Scam a skos:Concept,
        dpv:Concept ;
    dct:created ""^^xsd:date ;
    dct:source <https://www.iso.org/standard/75281.html> ;
    rdfs:isDefinedBy risk: ;
    sw:term_status "accepted"@en ;
    skos:definition ""@en ;
    skos:inScheme risk: ;
    skos:prefLabel "Scam"@en ;
    dpv:isSubTypeOf dpv:Harm .

risk:ScenarioAnalysis a skos:Concept,
        dpv:Concept ;
    dct:created ""^^xsd:date ;
    dct:source <https://www.iso.org/standard/72140.html> ;
    rdfs:isDefinedBy risk: ;
    sw:term_status "accepted"@en ;
    skos:definition "Identifies possible future scenarios through imagination, extrapolation from the present or modelling. Risk is then considered for each of these scenarios."@en ;
    skos:inScheme risk: ;
    skos:prefLabel "Scenario Analysis"@en ;
    dpv:isInstanceOf risk:QualitativeRiskAssessmentTechnique .

risk:SecurityBreach a skos:Concept,
        dpv:Concept ;
    dct:created ""^^xsd:date ;
    dct:source <https://www.iso.org/standard/75281.html> ;
    rdfs:isDefinedBy risk: ;
    sw:term_status "accepted"@en ;
    skos:definition ""@en ;
    skos:inScheme risk: ;
    skos:prefLabel "Security Breach"@en ;
    dpv:isSubTypeOf dpv:Consequence .

risk:ServiceInterruption a skos:Concept,
        dpv:Concept ;
    dct:created ""^^xsd:date ;
    dct:source <https://www.iso.org/standard/75281.html> ;
    rdfs:isDefinedBy risk: ;
    sw:term_status "accepted"@en ;
    skos:definition ""@en ;
    skos:inScheme risk: ;
    skos:prefLabel "Service Interruption"@en ;
    dpv:isSubTypeOf dpv:Detriment .

risk:ShareRisk a skos:Concept,
        dpv:Concept ;
    dct:created ""^^xsd:date ;
    rdfs:isDefinedBy risk: ;
    sw:term_status "accepted"@en ;
    skos:definition "Risk Mitigation Measure that shares Risk e.g. amongst stakeholders"@en ;
    skos:inScheme risk: ;
    skos:prefLabel "Share Risk"@en ;
    dpv:isSubTypeOf dpv:RiskMitigationMeasure .

risk:SoftwareMalfunction a skos:Concept,
        dpv:Concept ;
    dct:created ""^^xsd:date ;
    dct:source <https://www.iso.org/standard/75281.html> ;
    rdfs:isDefinedBy risk: ;
    sw:term_status "accepted"@en ;
    skos:definition ""@en ;
    skos:inScheme risk: ;
    skos:prefLabel "Software Malfunction"@en ;
    dpv:isSubTypeOf dpv:Detriment .

risk:Spoofing a skos:Concept,
        dpv:Concept ;
    dct:created ""^^xsd:date ;
    dct:source <https://www.iso.org/standard/75281.html> ;
    rdfs:isDefinedBy risk: ;
    sw:term_status "accepted"@en ;
    skos:definition ""@en ;
    skos:inScheme risk: ;
    skos:prefLabel "Spoofing"@en ;
    dpv:isSubTypeOf dpv:Harm .

risk:Spying a skos:Concept,
        dpv:Concept ;
    dct:created ""^^xsd:date ;
    dct:source <https://www.iso.org/standard/75281.html> ;
    rdfs:isDefinedBy risk: ;
    sw:term_status "accepted"@en ;
    skos:definition ""@en ;
    skos:inScheme risk: ;
    skos:prefLabel "Spying"@en ;
    dpv:isSubTypeOf dpv:NonMaterialDamage .

risk:Stalking a skos:Concept,
        dpv:Concept ;
    dct:created ""^^xsd:date ;
    dct:source <https://www.iso.org/standard/75281.html> ;
    rdfs:isDefinedBy risk: ;
    sw:term_status "accepted"@en ;
    skos:definition ""@en ;
    skos:inScheme risk: ;
    skos:prefLabel "Stalking"@en ;
    dpv:isSubTypeOf dpv:NonMaterialDamage .

risk:Surveys a skos:Concept,
        dpv:Concept ;
    dct:created ""^^xsd:date ;
    dct:source <https://www.iso.org/standard/72140.html> ;
    rdfs:isDefinedBy risk: ;
    sw:term_status "accepted"@en ;
    skos:definition "Paper- or computer-based questionnaires to elicit views."@en ;
    skos:inScheme risk: ;
    skos:prefLabel "Surveys"@en ;
    dpv:isInstanceOf risk:QualitativeRiskAssessmentTechnique .

risk:Taxonomies a skos:Concept,
        dpv:Concept ;
    dct:created ""^^xsd:date ;
    dct:source <https://www.iso.org/standard/72140.html> ;
    rdfs:isDefinedBy risk: ;
    sw:term_status "accepted"@en ;
    skos:definition "A taxonomy based on experience or on concepts and models that can be used to help identify risks or controls."@en ;
    skos:inScheme risk: ;
    skos:prefLabel "Taxonomies"@en ;
    dpv:isInstanceOf risk:QualitativeRiskAssessmentTechnique .

risk:Terrorism a skos:Concept,
        dpv:Concept ;
    dct:created ""^^xsd:date ;
    dct:source <https://www.iso.org/standard/75281.html> ;
    rdfs:isDefinedBy risk: ;
    sw:term_status "accepted"@en ;
    skos:definition ""@en ;
    skos:inScheme risk: ;
    skos:prefLabel "Terrorism"@en ;
    dpv:isSubTypeOf dpv:Harm .

risk:Theft a skos:Concept,
        dpv:Concept ;
    dct:created ""^^xsd:date ;
    dct:source <https://www.iso.org/standard/75281.html> ;
    rdfs:isDefinedBy risk: ;
    sw:term_status "accepted"@en ;
    skos:definition ""@en ;
    skos:inScheme risk: ;
    skos:prefLabel "Theft"@en ;
    dpv:isSubTypeOf dpv:MaterialDamage .

risk:TheftEquipment a skos:Concept,
        dpv:Concept ;
    dct:created ""^^xsd:date ;
    dct:source <https://www.iso.org/standard/75281.html> ;
    rdfs:isDefinedBy risk: ;
    sw:term_status "accepted"@en ;
    skos:definition ""@en ;
    skos:inScheme risk: ;
    skos:prefLabel "Theft of Equipment"@en ;
    dpv:isSubTypeOf dpv:MaterialDamage .

risk:TheftMedia a skos:Concept,
        dpv:Concept ;
    dct:created ""^^xsd:date ;
    dct:source <https://www.iso.org/standard/75281.html> ;
    rdfs:isDefinedBy risk: ;
    sw:term_status "accepted"@en ;
    skos:definition ""@en ;
    skos:inScheme risk: ;
    skos:prefLabel "Theft of Media"@en ;
    dpv:isSubTypeOf dpv:MaterialDamage .

risk:ThirdPartyOperationDisruption a skos:Concept,
        dpv:Concept ;
    dct:created ""^^xsd:date ;
    dct:source <https://www.iso.org/standard/75281.html> ;
    rdfs:isDefinedBy risk: ;
    sw:term_status "accepted"@en ;
    skos:definition ""@en ;
    skos:inScheme risk: ;
    skos:prefLabel "Third Party Operation Disruption"@en ;
    dpv:isSubTypeOf dpv:Detriment .

risk:Toxicological a skos:Concept,
        dpv:Concept ;
    dct:created ""^^xsd:date ;
    dct:source <https://www.iso.org/standard/72140.html> ;
    rdfs:isDefinedBy risk: ;
    sw:term_status "accepted"@en ;
    skos:definition "A series of steps taken to obtain a measure for the risk to humans or ecological systems due to exposure to chemicals."@en ;
    skos:inScheme risk: ;
    skos:prefLabel "Toxicological Risk Assessment"@en ;
    dpv:isInstanceOf risk:QuantitativeRiskAssessmentTechnique .

risk:UnauthorisedAccesstoPremises a skos:Concept,
        dpv:Concept ;
    dct:created ""^^xsd:date ;
    dct:source <https://www.iso.org/standard/75281.html> ;
    rdfs:isDefinedBy risk: ;
    sw:term_status "accepted"@en ;
    skos:definition ""@en ;
    skos:inScheme risk: ;
    skos:prefLabel "Unauthorised Access to Premises"@en ;
    dpv:isSubTypeOf dpv:Detriment .

risk:UnauthorisedDisclosureData a skos:Concept,
        dpv:Concept ;
    dct:created ""^^xsd:date ;
    dct:source <https://www.iso.org/standard/75281.html> ;
    rdfs:isDefinedBy risk: ;
    sw:term_status "accepted"@en ;
    skos:definition ""@en ;
    skos:inScheme risk: ;
    skos:prefLabel "Unauthorised Disclosure of Data"@en ;
    dpv:isSubTypeOf dpv:Detriment .

risk:UnauthorisedImpersonation a skos:Concept,
        dpv:Concept ;
    dct:created ""^^xsd:date ;
    dct:source <https://www.iso.org/standard/75281.html> ;
    rdfs:isDefinedBy risk: ;
    sw:term_status "accepted"@en ;
    skos:definition ""@en ;
    skos:inScheme risk: ;
    skos:prefLabel "Unauthorised Impersonation"@en ;
    dpv:isSubTypeOf dpv:NonMaterialDamage .

risk:UnauthorisedSystemAccess a skos:Concept,
        dpv:Concept ;
    dct:created ""^^xsd:date ;
    dct:source <https://www.iso.org/standard/75281.html> ;
    rdfs:isDefinedBy risk: ;
    sw:term_status "accepted"@en ;
    skos:definition ""@en ;
    skos:inScheme risk: ;
    skos:prefLabel "Unauthorised System Access"@en ;
    dpv:isSubTypeOf dpv:Detriment .

risk:UnauthorisedUseEquipment a skos:Concept,
        dpv:Concept ;
    dct:created ""^^xsd:date ;
    dct:source <https://www.iso.org/standard/75281.html> ;
    rdfs:isDefinedBy risk: ;
    sw:term_status "accepted"@en ;
    skos:definition ""@en ;
    skos:inScheme risk: ;
    skos:prefLabel "Unauthorised Use of Equipment"@en ;
    dpv:isSubTypeOf dpv:Detriment .

risk:UnwantedDeletionData a skos:Concept,
        dpv:Concept ;
    dct:created ""^^xsd:date ;
    dct:source <https://www.iso.org/standard/75281.html> ;
    rdfs:isDefinedBy risk: ;
    sw:term_status "accepted"@en ;
    skos:definition ""@en ;
    skos:inScheme risk: ;
    skos:prefLabel "Unwanted Deletion of Data"@en ;
    dpv:isSubTypeOf dpv:Damage .

risk:UnwantedDisclosureData a skos:Concept,
        dpv:Concept ;
    dct:created ""^^xsd:date ;
    dct:source <https://www.iso.org/standard/75281.html> ;
    rdfs:isDefinedBy risk: ;
    sw:term_status "accepted"@en ;
    skos:definition ""@en ;
    skos:inScheme risk: ;
    skos:prefLabel "Unwanted Disclosure of Data"@en ;
    dpv:isSubTypeOf dpv:Detriment .

risk:VaR a skos:Concept,
        dpv:Concept ;
    dct:created ""^^xsd:date ;
    dct:source <https://www.iso.org/standard/72140.html> ;
    rdfs:isDefinedBy risk: ;
    sw:term_status "accepted"@en ;
    skos:definition "Financial measure of risk that uses an assumed probability distribution of losses in a stable market condition to calculate the value of a loss that might occur with a specified probability within a defined time span."@en ;
    skos:inScheme risk: ;
    skos:prefLabel "Value At Risk (VaR)"@en ;
    dpv:isInstanceOf risk:QuantitativeRiskAssessmentTechnique .

risk:VeryHighLikelihood a skos:Concept,
        dpv:Concept ;
    dct:created ""^^xsd:date ;
    rdfs:isDefinedBy risk: ;
    sw:term_status "accepted"@en ;
    skos:definition "Level where Likelihood is Very High"@en ;
    skos:inScheme risk: ;
    skos:note "The suggested quantitative value for this concept is 0.9 on a scale of 0 to 1"@en ;
    skos:prefLabel "Very High Likelihood"@en ;
    dpv:isInstanceOf dpv:Likelihood,
        risk:5LikelihoodLevels,
        risk:7LikelihoodLevels .

risk:VeryHighRisk a skos:Concept,
        dpv:Concept ;
    dct:created ""^^xsd:date ;
    rdfs:isDefinedBy risk: ;
    sw:term_status "accepted"@en ;
    skos:definition "Level where Risk is Very High"@en ;
    skos:inScheme risk: ;
    skos:note "The suggested quantitative value for this concept is 0.9 on a scale of 0 to 1"@en ;
    skos:prefLabel "Very High Risk"@en ;
    dpv:isInstanceOf dpv:RiskLevel,
        risk:5RiskLevels,
        risk:7RiskLevels .

risk:VeryHighSeverity a skos:Concept,
        dpv:Concept ;
    dct:created ""^^xsd:date ;
    rdfs:isDefinedBy risk: ;
    sw:term_status "accepted"@en ;
    skos:definition "Level where Severity is Very High"@en ;
    skos:inScheme risk: ;
    skos:note "The suggested quantitative value for this concept is 0.9 on a scale of 0 to 1"@en ;
    skos:prefLabel "Very High Severity"@en ;
    dpv:isInstanceOf dpv:Severity,
        risk:5SeverityLevels,
        risk:7SeverityLevels .

risk:VeryLowLikelihood a skos:Concept,
        dpv:Concept ;
    dct:created ""^^xsd:date ;
    rdfs:isDefinedBy risk: ;
    sw:term_status "accepted"@en ;
    skos:definition "Level where Likelihood is Very Low"@en ;
    skos:inScheme risk: ;
    skos:note "The suggested quantitative value for this concept is 0.1 on a scale of 0 to 1"@en ;
    skos:prefLabel "Very Low Likelihood"@en ;
    dpv:isInstanceOf dpv:Likelihood,
        risk:5LikelihoodLevels,
        risk:7LikelihoodLevels .

risk:VeryLowRisk a skos:Concept,
        dpv:Concept ;
    dct:created ""^^xsd:date ;
    rdfs:isDefinedBy risk: ;
    sw:term_status "accepted"@en ;
    skos:definition "Level where Risk is Very Low"@en ;
    skos:inScheme risk: ;
    skos:note "The suggested quantitative value for this concept is 0.1 on a scale of 0 to 1"@en ;
    skos:prefLabel "Very Low Risk"@en ;
    dpv:isInstanceOf dpv:RiskLevel,
        risk:5RiskLevels,
        risk:7RiskLevels .

risk:VeryLowSeverity a skos:Concept,
        dpv:Concept ;
    dct:created ""^^xsd:date ;
    rdfs:isDefinedBy risk: ;
    sw:term_status "accepted"@en ;
    skos:definition "Level where Severity is Very Low"@en ;
    skos:inScheme risk: ;
    skos:note "The suggested quantitative value for this concept is 0.1 on a scale of 0 to 1"@en ;
    skos:prefLabel "Very Low Severity"@en ;
    dpv:isInstanceOf dpv:Severity,
        risk:5SeverityLevels,
        risk:7SeverityLevels .

risk:ViolationCodeConduct a skos:Concept,
        dpv:Concept ;
    dct:created ""^^xsd:date ;
    dct:source <https://www.iso.org/standard/75281.html> ;
    rdfs:isDefinedBy risk: ;
    sw:term_status "accepted"@en ;
    skos:definition ""@en ;
    skos:inScheme risk: ;
    skos:prefLabel "Violation of Code of Conduct"@en ;
    dpv:isSubTypeOf dpv:Damage .

risk:ViolationContractualObligations a skos:Concept,
        dpv:Concept ;
    dct:created ""^^xsd:date ;
    dct:source <https://www.iso.org/standard/75281.html> ;
    rdfs:isDefinedBy risk: ;
    sw:term_status "accepted"@en ;
    skos:definition ""@en ;
    skos:inScheme risk: ;
    skos:prefLabel "Violation of Contractual Obligations"@en ;
    dpv:isSubTypeOf dpv:Damage .

risk:ViolationEthicalCode a skos:Concept,
        dpv:Concept ;
    dct:created ""^^xsd:date ;
    dct:source <https://www.iso.org/standard/75281.html> ;
    rdfs:isDefinedBy risk: ;
    sw:term_status "accepted"@en ;
    skos:definition ""@en ;
    skos:inScheme risk: ;
    skos:prefLabel "Violation of Ethical Code"@en ;
    dpv:isSubTypeOf dpv:Damage .

risk:ViolationRegulatoryObligations a skos:Concept,
        dpv:Concept ;
    dct:created ""^^xsd:date ;
    dct:source <https://www.iso.org/standard/75281.html> ;
    rdfs:isDefinedBy risk: ;
    sw:term_status "accepted"@en ;
    skos:definition ""@en ;
    skos:inScheme risk: ;
    skos:prefLabel "Violation of Regulatory Obligations"@en ;
    dpv:isSubTypeOf dpv:Damage .

risk:ViolationStatutoryObligations a skos:Concept,
        dpv:Concept ;
    dct:created ""^^xsd:date ;
    dct:source <https://www.iso.org/standard/75281.html> ;
    rdfs:isDefinedBy risk: ;
    sw:term_status "accepted"@en ;
    skos:definition ""@en ;
    skos:inScheme risk: ;
    skos:prefLabel "Violation of Statutory Obligations"@en ;
    dpv:isSubTypeOf dpv:Damage .

risk:VulnerabilityCreated a skos:Concept,
        dpv:Concept ;
    dct:created ""^^xsd:date ;
    dct:source <https://www.iso.org/standard/75281.html> ;
    rdfs:isDefinedBy risk: ;
    sw:term_status "accepted"@en ;
    skos:definition ""@en ;
    skos:inScheme risk: ;
    skos:prefLabel "Vulnerability Created"@en ;
    dpv:isSubTypeOf dpv:Detriment .

risk:RiskAssessmentTechnique a skos:Concept,
        dpv:Concept ;
    dct:created ""^^xsd:date ;
    dct:source <https://www.iso.org/standard/72140.html> ;
    rdfs:isDefinedBy risk: ;
    sw:term_status "accepted"@en ;
    skos:definition "A technique or method used to analyse and identify risk levels, sources, likelihoods, severities, and other necessary information required to conduct risk management procedures"@en ;
    skos:inScheme risk: ;
    skos:prefLabel "Risk Assessment Technique"@en ;
    dpv:isSubTypeOf dpv:RiskManagementProcedure .

risk:3LikelihoodLevels a skos:Concept,
        dpv:Concept ;
    dct:created ""^^xsd:date ;
    rdfs:isDefinedBy risk: ;
    sw:term_status "accepted"@en ;
    skos:definition "Scale with 3 Likelihood Levels from High to Low"@en ;
    skos:inScheme risk: ;
    skos:prefLabel "3 Likelihood Levels"@en ;
    dpv:isSubTypeOf dpv:Likelihood .

risk:3RiskLevels a skos:Concept,
        dpv:Concept ;
    dct:created ""^^xsd:date ;
    rdfs:isDefinedBy risk: ;
    sw:term_status "accepted"@en ;
    skos:definition "Scale with 3 Risk Levels from High to Low"@en ;
    skos:inScheme risk: ;
    skos:prefLabel "3 Risk Levels"@en ;
    dpv:isSubTypeOf dpv:RiskLevel .

risk:3SeverityLevels a skos:Concept,
        dpv:Concept ;
    dct:created ""^^xsd:date ;
    rdfs:isDefinedBy risk: ;
    sw:term_status "accepted"@en ;
    skos:definition "Scale with 3 Severity Levels from High to Low"@en ;
    skos:inScheme risk: ;
    skos:prefLabel "3 Severity Levels"@en ;
    dpv:isSubTypeOf dpv:Severity .

risk:ControlRiskSource a skos:Concept,
        dpv:Concept ;
    dct:created ""^^xsd:date ;
    rdfs:isDefinedBy risk: ;
    sw:term_status "accepted"@en ;
    skos:definition "Risk Mitigation Measure that controls the Risk Source"@en ;
    skos:inScheme risk: ;
    skos:prefLabel "Control Risk Source"@en ;
    dpv:isSubTypeOf dpv:RiskMitigationMeasure .

risk:RiskMatrix a skos:Concept,
        dpv:Concept ;
    dct:created ""^^xsd:date ;
    dct:source <https://www.iso.org/standard/72140.html> ;
    rdfs:isDefinedBy risk: ;
    sw:term_status "accepted"@en ;
    skos:definition "Compares individual risks by selecting a consequence/ likelihood pair and displaying them on a matrix with consequence on one axis and likelihood on the other."@en ;
    skos:inScheme risk: ;
    skos:prefLabel "Risk Matrix"@en ;
    dpv:isInstanceOf risk:QualitativeRiskAssessmentTechnique,
        risk:QuantitativeRiskAssessmentTechnique .

risk:ControlConsequence a skos:Concept,
        dpv:Concept ;
    dct:created ""^^xsd:date ;
    rdfs:isDefinedBy risk: ;
    sw:term_status "accepted"@en ;
    skos:definition "Risk Mitigation Measure that controls the Consequences and Impacts"@en ;
    skos:inScheme risk: ;
    skos:prefLabel "Control Consequence"@en ;
    dpv:isSubTypeOf dpv:RiskMitigationMeasure .

risk:5LikelihoodLevels a skos:Concept,
        dpv:Concept ;
    dct:created ""^^xsd:date ;
    rdfs:isDefinedBy risk: ;
    sw:term_status "accepted"@en ;
    skos:definition "Scale with 5 Likelihood Levels from Very High to Very Low"@en ;
    skos:inScheme risk: ;
    skos:prefLabel "5 Likelihood Levels"@en ;
    dpv:isSubTypeOf dpv:Likelihood .

risk:5RiskLevels a skos:Concept,
        dpv:Concept ;
    dct:created ""^^xsd:date ;
    rdfs:isDefinedBy risk: ;
    sw:term_status "accepted"@en ;
    skos:definition "Scale with 5 Risk Levels from Very High to Very Low"@en ;
    skos:inScheme risk: ;
    skos:prefLabel "5 Risk Levels"@en ;
    dpv:isSubTypeOf dpv:RiskLevel .

risk:5SeverityLevels a skos:Concept,
        dpv:Concept ;
    dct:created ""^^xsd:date ;
    rdfs:isDefinedBy risk: ;
    sw:term_status "accepted"@en ;
    skos:definition "Scale with 5 Severity Levels from Very High to Very Low"@en ;
    skos:inScheme risk: ;
    skos:prefLabel "5 Severity Levels"@en ;
    dpv:isSubTypeOf dpv:Severity .

risk:ControlMonitors a skos:Concept,
        dpv:Concept ;
    dct:created ""^^xsd:date ;
    rdfs:isDefinedBy risk: ;
    sw:term_status "accepted"@en ;
    skos:definition "Risk Mitigation Measure that uses controls to monitor events"@en ;
    skos:inScheme risk: ;
    skos:note "Monitoring can be associated with characteristics such as assessing or detecting whether something is active, operational, performant, effective, has potential to materialise, is materialising, or has already materialised."@en ;
    skos:prefLabel "Control Monitors"@en ;
    dpv:isSubTypeOf dpv:RiskMitigationMeasure .

risk:7LikelihoodLevels a skos:Concept,
        dpv:Concept ;
    dct:created ""^^xsd:date ;
    rdfs:isDefinedBy risk: ;
    sw:term_status "accepted"@en ;
    skos:definition "Scale with 7 Likelihood Levels from Extremely High to Extremely Low"@en ;
    skos:inScheme risk: ;
    skos:prefLabel "7 Likelihood Levels"@en ;
    dpv:isSubTypeOf dpv:Likelihood .

risk:7RiskLevels a skos:Concept,
        dpv:Concept ;
    dct:created ""^^xsd:date ;
    rdfs:isDefinedBy risk: ;
    sw:term_status "accepted"@en ;
    skos:definition "Scale with 7 Risk Levels from Extremely High to Extremely Low"@en ;
    skos:inScheme risk: ;
    skos:prefLabel "7 Risk Levels"@en ;
    dpv:isSubTypeOf dpv:RiskLevel .

risk:7SeverityLevels a skos:Concept,
        dpv:Concept ;
    dct:created ""^^xsd:date ;
    rdfs:isDefinedBy risk: ;
    sw:term_status "accepted"@en ;
    skos:definition "Scale with 7 Severity Levels from Extremely High to Extremely Low"@en ;
    skos:inScheme risk: ;
    skos:prefLabel "7 Severity Levels"@en ;
    dpv:isSubTypeOf dpv:Severity .

risk:QuantitativeRiskAssessmentTechnique a skos:Concept,
        dpv:Concept ;
    dct:created ""^^xsd:date ;
    dct:source <https://www.iso.org/standard/72140.html> ;
    rdfs:isDefinedBy risk: ;
    sw:term_status "accepted"@en ;
    skos:definition "A risk assessment technique that uses quantitative methods"@en ;
    skos:inScheme risk: ;
    skos:prefLabel "Quantitative Risk Assessment Technique"@en ;
    dpv:isSubTypeOf risk:RiskAssessmentTechnique .

risk:QualitativeRiskAssessmentTechnique a skos:Concept,
        dpv:Concept ;
    dct:created ""^^xsd:date ;
    dct:source <https://www.iso.org/standard/72140.html> ;
    rdfs:isDefinedBy risk: ;
    sw:term_status "accepted"@en ;
    skos:definition "A risk assessment technique that uses qualitative methods"@en ;
    skos:inScheme risk: ;
    skos:prefLabel "Qualitative Risk Assessment Technique"@en ;
    dpv:isSubTypeOf risk:RiskAssessmentTechnique .

risk: a skos:ConceptScheme .

