@prefix dct: <http://purl.org/dc/terms/> .
@prefix dpv: <https://w3id.org/dpv#> .
@prefix dpv-pd: <https://w3id.org/dpv/pd#> .
@prefix owl: <http://www.w3.org/2002/07/owl#> .
@prefix skos: <http://www.w3.org/2004/02/skos/core#> .
@prefix svd: <http://www.specialprivacy.eu/vocabs/data#> .
@prefix sw: <http://www.w3.org/2003/06/sw-vocab-status/ns#> .
@prefix vann: <http://purl.org/vocab/vann/> .
@prefix xsd: <http://www.w3.org/2001/XMLSchema#> .

<https://w3id.org/dpv/dpv-pd> a owl:Ontology ;
    dct:abstract "DPV-PD is an extension to the Data Privacy Vocabulary that provides additional terms related to Personal Data categories."@en ;
    dct:contributor "Beatriz Esteves",
        "Bert Bos",
        "Bud Bruegger",
        "David Hickey",
        "Elmar Kiesling",
        "Eva Schlehahn",
        "Fajar J. Ekaputra",
        "Georg P Krog",
        "Javier D. Fern√°ndez",
        "Mark Lizar",
        "Paul Ryan",
        "Piero Bonatti",
        "Ramisa Gachpaz Hamed",
        "Rigo Wenning",
        "Rob Brennan",
        "Simon Steyskal" ;
    dct:created "2022-02-15"^^xsd:date ;
    dct:creator "Axel Polleres",
        "Harshvardhan J. Pandit" ;
    dct:description "DPV-PD is an extension to the Data Privacy Vocabulary that provides additional terms related to Personal Data categories."@en ;
    dct:modified "2022-02-15"^^xsd:date ;
    dct:source <https://www.w3.org/community/dpvcg/> ;
    dct:title "DPV-PD: Personal Data Extension for DPV"@en ;
    vann:preferredNamespacePrefix "dpv-pd" ;
    vann:preferredNamespaceUri "https://w3id.org/dpv/dpv-pd"^^xsd:string ;
    owl:versionInfo "0.4"^^xsd:string .

dpv-pd:PersonalDataConcepts a skos:Collection ;
    dct:title "Personal Data Concepts"^^xsd:string ;
    skos:member dpv-pd:Accent,
        dpv-pd:AccountIdentifier,
        dpv-pd:Acquantaince,
        dpv-pd:Age,
        dpv-pd:ApartmentOwned,
        dpv-pd:Association,
        dpv-pd:Attitude,
        dpv-pd:Authenticating,
        dpv-pd:AuthenticationHistory,
        dpv-pd:BankAccount,
        dpv-pd:Behavioral,
        dpv-pd:Biometric,
        dpv-pd:BloodType,
        dpv-pd:BrowserFingerprint,
        dpv-pd:BrowsingBehavior,
        dpv-pd:BrowsingReferral,
        dpv-pd:CallLog,
        dpv-pd:CarOwned,
        dpv-pd:Character,
        dpv-pd:Communication,
        dpv-pd:CommunicationsMetadata,
        dpv-pd:Connection,
        dpv-pd:Contact,
        dpv-pd:Country,
        dpv-pd:Credit,
        dpv-pd:CreditCapacity,
        dpv-pd:CreditCardNumber,
        dpv-pd:CreditRecord,
        dpv-pd:CreditScore,
        dpv-pd:CreditStanding,
        dpv-pd:CreditWorthiness,
        dpv-pd:Criminal,
        dpv-pd:CriminalCharge,
        dpv-pd:CriminalConviction,
        dpv-pd:CriminalPardon,
        dpv-pd:DNACode,
        dpv-pd:Demeanor,
        dpv-pd:Demographic,
        dpv-pd:DeviceApplications,
        dpv-pd:DeviceBased,
        dpv-pd:DeviceOperatingSystem,
        dpv-pd:DeviceSoftware,
        dpv-pd:Dialect,
        dpv-pd:Disability,
        dpv-pd:DisciplinaryAction,
        dpv-pd:Dislike,
        dpv-pd:Divorce,
        dpv-pd:DrugTestResult,
        dpv-pd:EmailAddress,
        dpv-pd:EmailContent,
        dpv-pd:EmploymentHistory,
        dpv-pd:EthnicOrigin,
        dpv-pd:Ethnicity,
        dpv-pd:External,
        dpv-pd:Family,
        dpv-pd:FamilyHealthHistory,
        dpv-pd:FamilyStructure,
        dpv-pd:Favorite,
        dpv-pd:FavoriteColor,
        dpv-pd:FavoriteFood,
        dpv-pd:FavoriteMusic,
        dpv-pd:Fetish,
        dpv-pd:Financial,
        dpv-pd:FinancialAccount,
        dpv-pd:FinancialAccountNumber,
        dpv-pd:Fingerprint,
        dpv-pd:Friend,
        dpv-pd:GPSCoordinate,
        dpv-pd:Gender,
        dpv-pd:GeneralReputation,
        dpv-pd:Geographic,
        dpv-pd:GroupMembership,
        dpv-pd:HairColor,
        dpv-pd:Health,
        dpv-pd:HealthHistory,
        dpv-pd:HealthRecord,
        dpv-pd:Height,
        dpv-pd:Historical,
        dpv-pd:HouseOwned,
        dpv-pd:IPAddress,
        dpv-pd:Identifying,
        dpv-pd:Income,
        dpv-pd:IncomeBracket,
        dpv-pd:IndividualHealthHistory,
        dpv-pd:Intention,
        dpv-pd:Interaction,
        dpv-pd:Interest,
        dpv-pd:Internal,
        dpv-pd:Job,
        dpv-pd:KnowledgeBelief,
        dpv-pd:Language,
        dpv-pd:LifeHistory,
        dpv-pd:Like,
        dpv-pd:LinkClicked,
        dpv-pd:LoanRecord,
        dpv-pd:Location,
        dpv-pd:MACAddress,
        dpv-pd:MaritalStatus,
        dpv-pd:Marriage,
        dpv-pd:MedicalHealth,
        dpv-pd:MentalHealth,
        dpv-pd:Name,
        dpv-pd:OfficialID,
        dpv-pd:Offspring,
        dpv-pd:Opinion,
        dpv-pd:Ownership,
        dpv-pd:PINCode,
        dpv-pd:Parent,
        dpv-pd:Password,
        dpv-pd:PaymentCard,
        dpv-pd:PaymentCardExpiry,
        dpv-pd:PaymentCardNumber,
        dpv-pd:PersonalPossession,
        dpv-pd:Personality,
        dpv-pd:PhilosophicalBelief,
        dpv-pd:PhysicalAddress,
        dpv-pd:PhysicalCharacteristic,
        dpv-pd:PhysicalHealth,
        dpv-pd:PhysicalTrait,
        dpv-pd:Picture,
        dpv-pd:Piercing,
        dpv-pd:PoliticalAffiliation,
        dpv-pd:Preference,
        dpv-pd:Prescription,
        dpv-pd:PrivacyPreference,
        dpv-pd:Proclivitie,
        dpv-pd:Professional,
        dpv-pd:ProfessionalCertification,
        dpv-pd:ProfessionalEvaluation,
        dpv-pd:ProfessionalInterview,
        dpv-pd:PublicLife,
        dpv-pd:Purchase,
        dpv-pd:PurchasesAndSpendingHabit,
        dpv-pd:Race,
        dpv-pd:Reference,
        dpv-pd:Relationship,
        dpv-pd:Religion,
        dpv-pd:ReligiousBelief,
        dpv-pd:Retina,
        dpv-pd:RoomNumber,
        dpv-pd:Salary,
        dpv-pd:Sale,
        dpv-pd:School,
        dpv-pd:SecretText,
        dpv-pd:ServiceConsumptionBehavior,
        dpv-pd:Sexual,
        dpv-pd:SexualHistory,
        dpv-pd:SexualPreference,
        dpv-pd:Sibling,
        dpv-pd:SkinTone,
        dpv-pd:Social,
        dpv-pd:SocialMediaCommunication,
        dpv-pd:SocialNetwork,
        dpv-pd:SocialStatus,
        dpv-pd:TVViewingBehavior,
        dpv-pd:Tattoo,
        dpv-pd:Tax,
        dpv-pd:TelephoneNumber,
        dpv-pd:Thought,
        dpv-pd:Tracking,
        dpv-pd:Transaction,
        dpv-pd:Transactional,
        dpv-pd:UID,
        dpv-pd:Username,
        dpv-pd:VoiceCommunicationRecording,
        dpv-pd:VoiceMail,
        dpv-pd:Weight,
        dpv-pd:WorkHistory .

dpv-pd:Accent a skos:Concept,
        dpv:Concept ;
    dct:created "2019-06-04"^^xsd:date ;
    dct:creator "Elmar Kiesling; Harshvardhan J. Pandit"^^xsd:string,
        "Fajar Ekaputra"^^xsd:string ;
    sw:term_status "accepted"@en ;
    skos:definition "Information about linguistic and speech accents."@en ;
    skos:prefLabel "Accent"@en ;
    skos:scopeNote <https://enterprivacy.com/wp-content/uploads/2018/09/Categories-of-Personal-Information.pdf> ;
    dpv:isSubTypeOf dpv-pd:Language .

dpv-pd:Acquantaince a skos:Concept,
        dpv:Concept ;
    dct:created "2019-06-04"^^xsd:date ;
    dct:creator "Elmar Kiesling; Harshvardhan J. Pandit"^^xsd:string,
        "Fajar Ekaputra"^^xsd:string ;
    sw:term_status "accepted"@en ;
    skos:definition "Information about acquaintainces in a social network."@en ;
    skos:prefLabel "Acquantaince"@en ;
    skos:scopeNote <https://enterprivacy.com/wp-content/uploads/2018/09/Categories-of-Personal-Information.pdf> ;
    dpv:isSubTypeOf dpv-pd:SocialNetwork .

dpv-pd:Age a skos:Concept,
        dpv:Concept ;
    dct:created "2019-06-04"^^xsd:date ;
    dct:creator "Elmar Kiesling; Harshvardhan J. Pandit"^^xsd:string,
        "Fajar Ekaputra"^^xsd:string ;
    sw:term_status "accepted"@en ;
    skos:definition "Information about age"@en ;
    skos:prefLabel "Age"@en ;
    skos:scopeNote <https://enterprivacy.com/wp-content/uploads/2018/09/Categories-of-Personal-Information.pdf> ;
    dpv:isSubTypeOf dpv-pd:PhysicalCharacteristic .

dpv-pd:ApartmentOwned a skos:Concept,
        dpv:Concept ;
    dct:created "2019-06-04"^^xsd:date ;
    dct:creator "Elmar Kiesling; Harshvardhan J. Pandit"^^xsd:string,
        "Fajar Ekaputra"^^xsd:string ;
    sw:term_status "accepted"@en ;
    skos:definition "Information about apartment(s) owned and its history"@en ;
    skos:prefLabel "Apartment Owned"@en ;
    skos:scopeNote <https://enterprivacy.com/wp-content/uploads/2018/09/Categories-of-Personal-Information.pdf> ;
    dpv:isSubTypeOf dpv-pd:HouseOwned .

dpv-pd:Association a skos:Concept,
        dpv:Concept ;
    dct:created "2019-06-04"^^xsd:date ;
    dct:creator "Elmar Kiesling; Harshvardhan J. Pandit"^^xsd:string,
        "Fajar Ekaputra"^^xsd:string ;
    sw:term_status "accepted"@en ;
    skos:definition "Information about associations in a social network with other individuals, groups, or entities e.g. friend of a friend"@en ;
    skos:prefLabel "Association"@en ;
    skos:scopeNote <https://enterprivacy.com/wp-content/uploads/2018/09/Categories-of-Personal-Information.pdf> ;
    dpv:isSubTypeOf dpv-pd:SocialNetwork .

dpv-pd:Attitude a skos:Concept,
        dpv:Concept ;
    dct:created "2019-06-04"^^xsd:date ;
    dct:creator "Elmar Kiesling; Harshvardhan J. Pandit"^^xsd:string,
        "Fajar Ekaputra"^^xsd:string ;
    sw:term_status "accepted"@en ;
    skos:definition "Information about attitude."@en ;
    skos:prefLabel "Attitude"@en ;
    skos:scopeNote <https://enterprivacy.com/wp-content/uploads/2018/09/Categories-of-Personal-Information.pdf> ;
    dpv:isSubTypeOf dpv-pd:Behavioral .

dpv-pd:AuthenticationHistory a skos:Concept,
        dpv:Concept ;
    dct:created "2020-11-04"^^xsd:date ;
    dct:creator "Georg P Krog"^^xsd:string ;
    sw:term_status "accepted"@en ;
    skos:definition "Information about prior authentication and its outcomes such as login attempts or location."@en ;
    skos:prefLabel "Authentication History"@en ;
    skos:scopeNote <https://www.w3.org/community/dpvcg/> ;
    dpv:isSubTypeOf dpv-pd:Behavioral .

dpv-pd:BankAccount a skos:Concept,
        dpv:Concept ;
    dct:created "2019-06-04"^^xsd:date ;
    dct:creator "Elmar Kiesling; Harshvardhan J. Pandit"^^xsd:string,
        "Fajar Ekaputra"^^xsd:string ;
    sw:term_status "accepted"@en ;
    skos:definition "Information about bank accounts."@en ;
    skos:prefLabel "Bank Account"@en ;
    skos:scopeNote <https://enterprivacy.com/wp-content/uploads/2018/09/Categories-of-Personal-Information.pdf> ;
    dpv:isSubTypeOf dpv-pd:FinancialAccount .

dpv-pd:BloodType a skos:Concept,
        dpv:Concept ;
    dct:created "2019-06-04"^^xsd:date ;
    dct:creator "Elmar Kiesling; Harshvardhan J. Pandit"^^xsd:string,
        "Fajar Ekaputra"^^xsd:string ;
    sw:term_status "accepted"@en ;
    skos:definition "Information about blood type."@en ;
    skos:prefLabel "Blood Type"@en ;
    skos:scopeNote <https://enterprivacy.com/wp-content/uploads/2018/09/Categories-of-Personal-Information.pdf> ;
    dpv:isSubTypeOf dpv-pd:MedicalHealth .

dpv-pd:BrowserFingerprint a skos:Concept,
        dpv:Concept ;
    dct:created "2019-06-04"^^xsd:date ;
    dct:creator "Elmar Kiesling; Harshvardhan J. Pandit"^^xsd:string,
        "Fajar Ekaputra"^^xsd:string ;
    sw:term_status "accepted"@en ;
    skos:definition "Information about the web browser which is used as a 'fingerprint'"@en ;
    skos:prefLabel "Browser Fingerprint"@en ;
    skos:scopeNote <https://enterprivacy.com/wp-content/uploads/2018/09/Categories-of-Personal-Information.pdf> ;
    dpv:isSubTypeOf dpv-pd:DeviceBased .

dpv-pd:BrowsingReferral a skos:Concept,
        dpv:Concept ;
    dct:created "2020-11-04"^^xsd:date ;
    dct:creator "Georg P Krog"^^xsd:string ;
    sw:term_status "accepted"@en ;
    skos:definition "Information about web browsing referrer or referral, which can be based on location, targeted referrals, direct, organic search, social media or actions, campaigns."@en ;
    skos:prefLabel "Browsing Referral"@en ;
    skos:scopeNote <https://www.w3.org/community/dpvcg/> ;
    dpv:isSubTypeOf dpv-pd:BrowsingBehavior .

dpv-pd:CallLog a skos:Concept,
        dpv:Concept ;
    dct:created "2019-06-04"^^xsd:date ;
    dct:creator "Elmar Kiesling; Harshvardhan J. Pandit"^^xsd:string,
        "Fajar Ekaputra"^^xsd:string ;
    sw:term_status "accepted"@en ;
    skos:definition "Information about the calls that an individual has made."@en ;
    skos:prefLabel "Call Log"@en ;
    skos:scopeNote <https://enterprivacy.com/wp-content/uploads/2018/09/Categories-of-Personal-Information.pdf> ;
    dpv:isSubTypeOf dpv-pd:Behavioral .

dpv-pd:CarOwned a skos:Concept,
        dpv:Concept ;
    dct:created "2019-06-04"^^xsd:date ;
    dct:creator "Elmar Kiesling; Harshvardhan J. Pandit"^^xsd:string,
        "Fajar Ekaputra"^^xsd:string ;
    sw:term_status "accepted"@en ;
    skos:definition "Information about cars ownership and ownership history."@en ;
    skos:prefLabel "Car Owned"@en ;
    skos:scopeNote <https://enterprivacy.com/wp-content/uploads/2018/09/Categories-of-Personal-Information.pdf> ;
    dpv:isSubTypeOf dpv-pd:Ownership .

dpv-pd:Character a skos:Concept,
        dpv:Concept ;
    dct:created "2019-06-04"^^xsd:date ;
    dct:creator "Elmar Kiesling; Harshvardhan J. Pandit"^^xsd:string,
        "Fajar Ekaputra"^^xsd:string ;
    sw:term_status "accepted"@en ;
    skos:definition "Information about character in the public sphere"@en ;
    skos:prefLabel "Character"@en ;
    skos:scopeNote <https://enterprivacy.com/wp-content/uploads/2018/09/Categories-of-Personal-Information.pdf> ;
    dpv:isSubTypeOf dpv-pd:PublicLife .

dpv-pd:CommunicationsMetadata a skos:Concept,
        dpv:Concept ;
    dct:created "2019-06-04"^^xsd:date ;
    dct:creator "Elmar Kiesling; Harshvardhan J. Pandit"^^xsd:string,
        "Fajar Ekaputra"^^xsd:string ;
    sw:term_status "accepted"@en ;
    skos:definition "Information about communication metadata in the public sphere"@en ;
    skos:prefLabel "Communications Metadata"@en ;
    skos:related svd:Interactive ;
    skos:scopeNote <https://enterprivacy.com/wp-content/uploads/2018/09/Categories-of-Personal-Information.pdf> ;
    dpv:isSubTypeOf dpv-pd:PublicLife .

dpv-pd:Connection a skos:Concept,
        dpv:Concept ;
    dct:created "2019-06-04"^^xsd:date ;
    dct:creator "Elmar Kiesling; Harshvardhan J. Pandit"^^xsd:string,
        "Fajar Ekaputra"^^xsd:string ;
    sw:term_status "accepted"@en ;
    skos:definition "Information about and including connections in a social network"@en ;
    skos:prefLabel "Connection"@en ;
    skos:scopeNote <https://enterprivacy.com/wp-content/uploads/2018/09/Categories-of-Personal-Information.pdf> ;
    dpv:isSubTypeOf dpv-pd:SocialNetwork .

dpv-pd:Country a skos:Concept,
        dpv:Concept ;
    dct:created "2019-06-04"^^xsd:date ;
    dct:creator "Elmar Kiesling; Harshvardhan J. Pandit"^^xsd:string,
        "Fajar Ekaputra"^^xsd:string ;
    sw:term_status "accepted"@en ;
    skos:definition "Information about country e.g. residence, travel."@en ;
    skos:prefLabel "Country"@en ;
    skos:scopeNote <https://enterprivacy.com/wp-content/uploads/2018/09/Categories-of-Personal-Information.pdf> ;
    dpv:isSubTypeOf dpv-pd:Location .

dpv-pd:CreditCapacity a skos:Concept,
        dpv:Concept ;
    dct:created "2019-06-04"^^xsd:date ;
    dct:creator "Elmar Kiesling; Harshvardhan J. Pandit"^^xsd:string,
        "Fajar Ekaputra"^^xsd:string ;
    sw:term_status "accepted"@en ;
    skos:definition "Information about credit capacity."@en ;
    skos:prefLabel "Credit Capacity"@en ;
    skos:scopeNote <https://enterprivacy.com/wp-content/uploads/2018/09/Categories-of-Personal-Information.pdf> ;
    dpv:isSubTypeOf dpv-pd:Credit .

dpv-pd:CreditCardNumber a skos:Concept,
        dpv:Concept ;
    dct:created "2019-06-04"^^xsd:date ;
    dct:creator "Elmar Kiesling; Harshvardhan J. Pandit"^^xsd:string,
        "Fajar Ekaputra"^^xsd:string ;
    sw:term_status "accepted"@en ;
    skos:definition "Information about credit card number"@en ;
    skos:prefLabel "Credit Card Number"@en ;
    skos:scopeNote <https://enterprivacy.com/wp-content/uploads/2018/09/Categories-of-Personal-Information.pdf> ;
    dpv:isSubTypeOf dpv-pd:PaymentCardNumber .

dpv-pd:CreditRecord a skos:Concept,
        dpv:Concept ;
    dct:created "2019-06-04"^^xsd:date ;
    dct:creator "Elmar Kiesling; Harshvardhan J. Pandit"^^xsd:string,
        "Fajar Ekaputra"^^xsd:string ;
    sw:term_status "accepted"@en ;
    skos:definition "Information about credit record."@en ;
    skos:prefLabel "Credit Record"@en ;
    skos:scopeNote <https://enterprivacy.com/wp-content/uploads/2018/09/Categories-of-Personal-Information.pdf> ;
    dpv:isSubTypeOf dpv-pd:Credit .

dpv-pd:CreditScore a skos:Concept,
        dpv:Concept ;
    dct:created "2019-06-04"^^xsd:date ;
    dct:creator "Elmar Kiesling; Harshvardhan J. Pandit"^^xsd:string,
        "Fajar Ekaputra"^^xsd:string ;
    sw:term_status "accepted"@en ;
    skos:definition "Information about credit score."@en ;
    skos:prefLabel "Credit Score"@en ;
    skos:scopeNote <https://enterprivacy.com/wp-content/uploads/2018/09/Categories-of-Personal-Information.pdf> ;
    dpv:isSubTypeOf dpv-pd:CreditWorthiness .

dpv-pd:CreditStanding a skos:Concept,
        dpv:Concept ;
    dct:created "2019-06-04"^^xsd:date ;
    dct:creator "Elmar Kiesling; Harshvardhan J. Pandit"^^xsd:string,
        "Fajar Ekaputra"^^xsd:string ;
    sw:term_status "accepted"@en ;
    skos:definition "Information about credit standing."@en ;
    skos:prefLabel "Credit Standing"@en ;
    skos:scopeNote <https://enterprivacy.com/wp-content/uploads/2018/09/Categories-of-Personal-Information.pdf> ;
    dpv:isSubTypeOf dpv-pd:Credit .

dpv-pd:CriminalCharge a skos:Concept,
        dpv:Concept ;
    dct:created "2019-06-04"^^xsd:date ;
    dct:creator "Elmar Kiesling; Harshvardhan J. Pandit"^^xsd:string,
        "Fajar Ekaputra"^^xsd:string ;
    sw:term_status "accepted"@en ;
    skos:definition "Information about criminal charges."@en ;
    skos:prefLabel "Criminal Charge"@en ;
    skos:scopeNote <https://enterprivacy.com/wp-content/uploads/2018/09/Categories-of-Personal-Information.pdf> ;
    dpv:isSubTypeOf dpv-pd:Criminal .

dpv-pd:CriminalConviction a skos:Concept,
        dpv:Concept ;
    dct:created "2019-06-04"^^xsd:date ;
    dct:creator "Elmar Kiesling; Harshvardhan J. Pandit"^^xsd:string,
        "Fajar Ekaputra"^^xsd:string ;
    sw:term_status "accepted"@en ;
    skos:definition "Information about criminal convictions."@en ;
    skos:prefLabel "Criminal Conviction"@en ;
    skos:scopeNote <https://enterprivacy.com/wp-content/uploads/2018/09/Categories-of-Personal-Information.pdf> ;
    dpv:isSubTypeOf dpv-pd:Criminal .

dpv-pd:CriminalPardon a skos:Concept,
        dpv:Concept ;
    dct:created "2019-06-04"^^xsd:date ;
    dct:creator "Elmar Kiesling; Harshvardhan J. Pandit"^^xsd:string,
        "Fajar Ekaputra"^^xsd:string ;
    sw:term_status "accepted"@en ;
    skos:definition "Information about criminal pardons."@en ;
    skos:prefLabel "Criminal Pardon"@en ;
    skos:scopeNote <https://enterprivacy.com/wp-content/uploads/2018/09/Categories-of-Personal-Information.pdf> ;
    dpv:isSubTypeOf dpv-pd:Criminal .

dpv-pd:DNACode a skos:Concept,
        dpv:Concept ;
    dct:created "2019-06-04"^^xsd:date ;
    dct:creator "Elmar Kiesling; Harshvardhan J. Pandit"^^xsd:string,
        "Fajar Ekaputra"^^xsd:string ;
    sw:term_status "accepted"@en ;
    skos:definition "Information about DNA."@en ;
    skos:prefLabel "DNA Code"@en ;
    skos:scopeNote <https://enterprivacy.com/wp-content/uploads/2018/09/Categories-of-Personal-Information.pdf> ;
    dpv:isSubTypeOf dpv-pd:MedicalHealth .

dpv-pd:Demeanor a skos:Concept,
        dpv:Concept ;
    dct:created "2019-06-04"^^xsd:date ;
    dct:creator "Elmar Kiesling; Harshvardhan J. Pandit"^^xsd:string,
        "Fajar Ekaputra"^^xsd:string ;
    sw:term_status "accepted"@en ;
    skos:definition "Information about demeanor."@en ;
    skos:prefLabel "Demeanor"@en ;
    skos:scopeNote <https://enterprivacy.com/wp-content/uploads/2018/09/Categories-of-Personal-Information.pdf> ;
    dpv:isSubTypeOf dpv-pd:Behavioral .

dpv-pd:DeviceApplications a skos:Concept,
        dpv:Concept ;
    dct:created "2020-11-04"^^xsd:date ;
    dct:creator "Beatriz Esteves"^^xsd:string,
        "Georg P Krog"^^xsd:string,
        "Harshvardhan J. Pandit"^^xsd:string,
        "Paul Ryan"^^xsd:string ;
    sw:term_status "accepted"@en ;
    skos:definition "Information about applications or application-like software on a device."@en ;
    skos:prefLabel "Device Applications"@en ;
    skos:scopeNote <https://www.w3.org/community/dpvcg/> ;
    dpv:isSubTypeOf dpv-pd:DeviceSoftware .

dpv-pd:DeviceOperatingSystem a skos:Concept,
        dpv:Concept ;
    dct:created "2020-11-04"^^xsd:date ;
    dct:creator "Beatriz Esteves"^^xsd:string,
        "Georg P Krog"^^xsd:string,
        "Harshvardhan J. Pandit"^^xsd:string,
        "Paul Ryan"^^xsd:string ;
    sw:term_status "accepted"@en ;
    skos:definition "Information about the operating system (OS) or system software that manages hardware or software resources."@en ;
    skos:prefLabel "Device Operating System"@en ;
    skos:scopeNote <https://www.w3.org/community/dpvcg/> ;
    dpv:isSubTypeOf dpv-pd:DeviceSoftware .

dpv-pd:Dialect a skos:Concept,
        dpv:Concept ;
    dct:created "2019-06-04"^^xsd:date ;
    dct:creator "Elmar Kiesling; Harshvardhan J. Pandit"^^xsd:string,
        "Fajar Ekaputra"^^xsd:string ;
    sw:term_status "accepted"@en ;
    skos:definition "Information about linguistic dialects."@en ;
    skos:prefLabel "Dialect"@en ;
    skos:scopeNote <https://enterprivacy.com/wp-content/uploads/2018/09/Categories-of-Personal-Information.pdf> ;
    dpv:isSubTypeOf dpv-pd:Language .

dpv-pd:Disability a skos:Concept,
        dpv:Concept ;
    dct:created "2019-06-04"^^xsd:date ;
    dct:creator "Elmar Kiesling; Harshvardhan J. Pandit"^^xsd:string,
        "Fajar Ekaputra"^^xsd:string ;
    sw:term_status "accepted"@en ;
    skos:definition "Information about disabilities."@en ;
    skos:prefLabel "Disability"@en ;
    skos:scopeNote <https://enterprivacy.com/wp-content/uploads/2018/09/Categories-of-Personal-Information.pdf> ;
    dpv:isSubTypeOf dpv-pd:MedicalHealth .

dpv-pd:DisciplinaryAction a skos:Concept,
        dpv:Concept ;
    dct:created "2019-06-04"^^xsd:date ;
    dct:creator "Elmar Kiesling; Harshvardhan J. Pandit"^^xsd:string,
        "Fajar Ekaputra"^^xsd:string ;
    sw:term_status "accepted"@en ;
    skos:definition "Information about disciplinary actions and its history"@en ;
    skos:prefLabel "Disciplinary Action"@en ;
    skos:scopeNote <https://enterprivacy.com/wp-content/uploads/2018/09/Categories-of-Personal-Information.pdf> ;
    dpv:isSubTypeOf dpv-pd:Professional .

dpv-pd:Dislike a skos:Concept,
        dpv:Concept ;
    dct:created "2019-06-04"^^xsd:date ;
    dct:creator "Elmar Kiesling; Harshvardhan J. Pandit"^^xsd:string,
        "Fajar Ekaputra"^^xsd:string ;
    sw:term_status "accepted"@en ;
    skos:definition "Information about dislikes or preferences regarding repulsions."@en ;
    skos:prefLabel "Dislike"@en ;
    skos:scopeNote <https://enterprivacy.com/wp-content/uploads/2018/09/Categories-of-Personal-Information.pdf> ;
    dpv:isSubTypeOf dpv-pd:Interest .

dpv-pd:Divorce a skos:Concept,
        dpv:Concept ;
    dct:created "2019-06-04"^^xsd:date ;
    dct:creator "Elmar Kiesling; Harshvardhan J. Pandit"^^xsd:string,
        "Fajar Ekaputra"^^xsd:string ;
    sw:term_status "accepted"@en ;
    skos:definition "Information about divorce(s)."@en ;
    skos:prefLabel "Divorce"@en ;
    skos:scopeNote <https://enterprivacy.com/wp-content/uploads/2018/09/Categories-of-Personal-Information.pdf> ;
    dpv:isSubTypeOf dpv-pd:FamilyStructure .

dpv-pd:DrugTestResult a skos:Concept,
        dpv:Concept ;
    dct:created "2019-06-04"^^xsd:date ;
    dct:creator "Elmar Kiesling; Harshvardhan J. Pandit"^^xsd:string,
        "Fajar Ekaputra"^^xsd:string ;
    sw:term_status "accepted"@en ;
    skos:definition "Information about drug test results."@en ;
    skos:prefLabel "Drug Test Result"@en ;
    skos:scopeNote <https://enterprivacy.com/wp-content/uploads/2018/09/Categories-of-Personal-Information.pdf> ;
    dpv:isSubTypeOf dpv-pd:MedicalHealth .

dpv-pd:EmailAddress a skos:Concept,
        dpv:Concept ;
    dct:created "2019-06-04"^^xsd:date ;
    dct:creator "Elmar Kiesling; Harshvardhan J. Pandit"^^xsd:string,
        "Fajar Ekaputra"^^xsd:string ;
    sw:term_status "accepted"@en ;
    skos:definition "Information about Email address."@en ;
    skos:prefLabel "Email Address"@en ;
    skos:scopeNote <https://enterprivacy.com/wp-content/uploads/2018/09/Categories-of-Personal-Information.pdf> ;
    dpv:isSubTypeOf dpv-pd:Contact .

dpv-pd:EmailContent a skos:Concept,
        dpv:Concept ;
    dct:created "2019-06-04"^^xsd:date ;
    dct:creator "Elmar Kiesling; Harshvardhan J. Pandit"^^xsd:string,
        "Fajar Ekaputra"^^xsd:string ;
    sw:term_status "accepted"@en ;
    skos:definition "Information about the contents of Emails sent or received"@en ;
    skos:prefLabel "Email Content"@en ;
    skos:scopeNote <https://enterprivacy.com/wp-content/uploads/2018/09/Categories-of-Personal-Information.pdf> ;
    dpv:isSubTypeOf dpv-pd:Communication .

dpv-pd:EmploymentHistory a skos:Concept,
        dpv:Concept ;
    dct:created "2019-06-04"^^xsd:date ;
    dct:creator "Elmar Kiesling; Harshvardhan J. Pandit"^^xsd:string,
        "Fajar Ekaputra"^^xsd:string ;
    sw:term_status "accepted"@en ;
    skos:definition "Information about employment history"@en ;
    skos:prefLabel "Employment History"@en ;
    skos:scopeNote <https://enterprivacy.com/wp-content/uploads/2018/09/Categories-of-Personal-Information.pdf> ;
    dpv:isSubTypeOf dpv-pd:Professional .

dpv-pd:EthnicOrigin a skos:Concept,
        dpv:Concept ;
    dct:created "2019-06-04"^^xsd:date ;
    dct:creator "Elmar Kiesling; Harshvardhan J. Pandit"^^xsd:string,
        "Fajar Ekaputra"^^xsd:string ;
    sw:term_status "accepted"@en ;
    skos:definition "Information about ethnic origin"@en ;
    skos:prefLabel "Ethnic Origin"@en ;
    skos:scopeNote <https://enterprivacy.com/wp-content/uploads/2018/09/Categories-of-Personal-Information.pdf> ;
    dpv:isSubTypeOf dpv:SpecialCategoryPersonalData,
        dpv-pd:Ethnicity .

dpv-pd:FamilyHealthHistory a skos:Concept,
        dpv:Concept ;
    dct:created "2019-06-04"^^xsd:date ;
    dct:creator "Elmar Kiesling; Harshvardhan J. Pandit"^^xsd:string,
        "Fajar Ekaputra"^^xsd:string ;
    sw:term_status "accepted"@en ;
    skos:definition "Information about family health history."@en ;
    skos:prefLabel "Family Health History"@en ;
    skos:scopeNote <https://enterprivacy.com/wp-content/uploads/2018/09/Categories-of-Personal-Information.pdf> ;
    dpv:isSubTypeOf dpv-pd:HealthHistory .

dpv-pd:FavoriteColor a skos:Concept,
        dpv:Concept ;
    dct:created "2019-06-04"^^xsd:date ;
    dct:creator "Elmar Kiesling; Harshvardhan J. Pandit"^^xsd:string,
        "Fajar Ekaputra"^^xsd:string ;
    sw:term_status "accepted"@en ;
    skos:definition "Information about favorite color."@en ;
    skos:prefLabel "Favorite Color"@en ;
    skos:scopeNote <https://enterprivacy.com/wp-content/uploads/2018/09/Categories-of-Personal-Information.pdf> ;
    dpv:isSubTypeOf dpv-pd:Favorite .

dpv-pd:FavoriteFood a skos:Concept,
        dpv:Concept ;
    dct:created "2019-06-04"^^xsd:date ;
    dct:creator "Elmar Kiesling; Harshvardhan J. Pandit"^^xsd:string,
        "Fajar Ekaputra"^^xsd:string ;
    sw:term_status "accepted"@en ;
    skos:definition "Information about favorite food."@en ;
    skos:prefLabel "Favorite Food"@en ;
    skos:scopeNote <https://enterprivacy.com/wp-content/uploads/2018/09/Categories-of-Personal-Information.pdf> ;
    dpv:isSubTypeOf dpv-pd:Favorite .

dpv-pd:FavoriteMusic a skos:Concept,
        dpv:Concept ;
    dct:created "2019-06-04"^^xsd:date ;
    dct:creator "Elmar Kiesling; Harshvardhan J. Pandit"^^xsd:string,
        "Fajar Ekaputra"^^xsd:string ;
    sw:term_status "accepted"@en ;
    skos:definition "Information about favorite music."@en ;
    skos:prefLabel "Favorite Music"@en ;
    skos:scopeNote <https://enterprivacy.com/wp-content/uploads/2018/09/Categories-of-Personal-Information.pdf> ;
    dpv:isSubTypeOf dpv-pd:Favorite .

dpv-pd:Fetish a skos:Concept,
        dpv:Concept ;
    dct:created "2019-06-04"^^xsd:date ;
    dct:creator "Elmar Kiesling; Harshvardhan J. Pandit"^^xsd:string,
        "Fajar Ekaputra"^^xsd:string ;
    sw:term_status "accepted"@en ;
    skos:definition "Information an individual's sexual fetishes"@en ;
    skos:prefLabel "Fetish"@en ;
    skos:scopeNote <https://enterprivacy.com/wp-content/uploads/2018/09/Categories-of-Personal-Information.pdf> ;
    dpv:isSubTypeOf dpv-pd:Sexual .

dpv-pd:FinancialAccountNumber a skos:Concept,
        dpv:Concept ;
    dct:created "2019-06-04"^^xsd:date ;
    dct:creator "Elmar Kiesling; Harshvardhan J. Pandit"^^xsd:string,
        "Fajar Ekaputra"^^xsd:string ;
    sw:term_status "accepted"@en ;
    skos:definition "Information about financial account number"@en ;
    skos:prefLabel "Financial Account Number"@en ;
    skos:scopeNote <https://enterprivacy.com/wp-content/uploads/2018/09/Categories-of-Personal-Information.pdf> ;
    dpv:isSubTypeOf dpv-pd:AccountIdentifier .

dpv-pd:Fingerprint a skos:Concept,
        dpv:Concept ;
    dct:created "2019-06-04"^^xsd:date ;
    dct:creator "Elmar Kiesling; Harshvardhan J. Pandit"^^xsd:string,
        "Fajar Ekaputra"^^xsd:string ;
    sw:term_status "accepted"@en ;
    skos:definition "Information about fingerprint used for biometric purposes."@en ;
    skos:prefLabel "Fingerprint"@en ;
    skos:scopeNote <https://enterprivacy.com/wp-content/uploads/2018/09/Categories-of-Personal-Information.pdf> ;
    dpv:isSubTypeOf dpv-pd:Biometric .

dpv-pd:Friend a skos:Concept,
        dpv:Concept ;
    dct:created "2019-06-04"^^xsd:date ;
    dct:creator "Elmar Kiesling; Harshvardhan J. Pandit"^^xsd:string,
        "Fajar Ekaputra"^^xsd:string ;
    sw:term_status "accepted"@en ;
    skos:definition "Information about friends in a social network, including aspects of friendships such as years together or nature of friendship."@en ;
    skos:prefLabel "Friend"@en ;
    skos:scopeNote <https://enterprivacy.com/wp-content/uploads/2018/09/Categories-of-Personal-Information.pdf> ;
    dpv:isSubTypeOf dpv-pd:SocialNetwork .

dpv-pd:GPSCoordinate a skos:Concept,
        dpv:Concept ;
    dct:created "2019-06-04"^^xsd:date ;
    dct:creator "Elmar Kiesling; Harshvardhan J. Pandit"^^xsd:string,
        "Fajar Ekaputra"^^xsd:string ;
    sw:term_status "accepted"@en ;
    skos:definition "Information about location expressed using Global Position System coordinates (GPS)"@en ;
    skos:prefLabel "GPS Coordinate"@en ;
    skos:scopeNote <https://enterprivacy.com/wp-content/uploads/2018/09/Categories-of-Personal-Information.pdf> ;
    dpv:isSubTypeOf dpv-pd:Location .

dpv-pd:Gender a skos:Concept,
        dpv:Concept ;
    dct:created "2019-06-04"^^xsd:date ;
    dct:creator "Elmar Kiesling; Harshvardhan J. Pandit"^^xsd:string,
        "Fajar Ekaputra"^^xsd:string ;
    sw:term_status "accepted"@en ;
    skos:definition "Information about gender"@en ;
    skos:prefLabel "Gender"@en ;
    skos:scopeNote <https://enterprivacy.com/wp-content/uploads/2018/09/Categories-of-Personal-Information.pdf> ;
    dpv:isSubTypeOf dpv-pd:PhysicalCharacteristic .

dpv-pd:GeneralReputation a skos:Concept,
        dpv:Concept ;
    dct:created "2019-06-04"^^xsd:date ;
    dct:creator "Elmar Kiesling; Harshvardhan J. Pandit"^^xsd:string,
        "Fajar Ekaputra"^^xsd:string ;
    sw:term_status "accepted"@en ;
    skos:definition "Information about reputation in the public sphere"@en ;
    skos:prefLabel "General Reputation"@en ;
    skos:scopeNote <https://enterprivacy.com/wp-content/uploads/2018/09/Categories-of-Personal-Information.pdf> ;
    dpv:isSubTypeOf dpv-pd:PublicLife .

dpv-pd:Geographic a skos:Concept,
        dpv:Concept ;
    dct:created "2019-06-04"^^xsd:date ;
    dct:creator "Elmar Kiesling; Harshvardhan J. Pandit"^^xsd:string,
        "Fajar Ekaputra"^^xsd:string ;
    sw:term_status "accepted"@en ;
    skos:definition "Information about location or based on geography (e.g. home address)"@en ;
    skos:prefLabel "Geographic"@en ;
    skos:scopeNote <https://enterprivacy.com/wp-content/uploads/2018/09/Categories-of-Personal-Information.pdf> ;
    dpv:isSubTypeOf dpv-pd:Demographic .

dpv-pd:GroupMembership a skos:Concept,
        dpv:Concept ;
    dct:created "2019-06-04"^^xsd:date ;
    dct:creator "Elmar Kiesling; Harshvardhan J. Pandit"^^xsd:string,
        "Fajar Ekaputra"^^xsd:string ;
    sw:term_status "accepted"@en ;
    skos:definition "Information about groups and memberships included or associated with a social network"@en ;
    skos:prefLabel "Group Membership"@en ;
    skos:scopeNote <https://enterprivacy.com/wp-content/uploads/2018/09/Categories-of-Personal-Information.pdf> ;
    dpv:isSubTypeOf dpv-pd:SocialNetwork .

dpv-pd:HairColor a skos:Concept,
        dpv:Concept ;
    dct:created "2019-06-04"^^xsd:date ;
    dct:creator "Elmar Kiesling; Harshvardhan J. Pandit"^^xsd:string,
        "Fajar Ekaputra"^^xsd:string ;
    sw:term_status "accepted"@en ;
    skos:definition "Information about hair color"@en ;
    skos:prefLabel "Hair Color"@en ;
    skos:scopeNote <https://enterprivacy.com/wp-content/uploads/2018/09/Categories-of-Personal-Information.pdf> ;
    dpv:isSubTypeOf dpv-pd:PhysicalCharacteristic .

dpv-pd:HealthRecord a skos:Concept,
        dpv:Concept ;
    dct:created "2019-06-04"^^xsd:date ;
    dct:creator "Elmar Kiesling; Harshvardhan J. Pandit"^^xsd:string,
        "Fajar Ekaputra"^^xsd:string ;
    sw:term_status "accepted"@en ;
    skos:definition "Information about health record."@en ;
    skos:prefLabel "Health Record"@en ;
    skos:scopeNote <https://enterprivacy.com/wp-content/uploads/2018/09/Categories-of-Personal-Information.pdf> ;
    dpv:isSubTypeOf dpv-pd:MedicalHealth .

dpv-pd:Height a skos:Concept,
        dpv:Concept ;
    dct:created "2019-06-04"^^xsd:date ;
    dct:creator "Elmar Kiesling; Harshvardhan J. Pandit"^^xsd:string,
        "Fajar Ekaputra"^^xsd:string ;
    sw:term_status "accepted"@en ;
    skos:definition "Information about physical height"@en ;
    skos:prefLabel "Height"@en ;
    skos:scopeNote <https://enterprivacy.com/wp-content/uploads/2018/09/Categories-of-Personal-Information.pdf> ;
    dpv:isSubTypeOf dpv-pd:PhysicalCharacteristic .

dpv-pd:IPAddress a skos:Concept,
        dpv:Concept ;
    dct:created "2019-06-04"^^xsd:date ;
    dct:creator "Elmar Kiesling; Harshvardhan J. Pandit"^^xsd:string,
        "Fajar Ekaputra"^^xsd:string ;
    sw:term_status "accepted"@en ;
    skos:definition "Information about the Internet protocol (IP) address of a device"@en ;
    skos:prefLabel "IP Address"@en ;
    skos:scopeNote <https://enterprivacy.com/wp-content/uploads/2018/09/Categories-of-Personal-Information.pdf> ;
    dpv:isSubTypeOf dpv-pd:DeviceBased .

dpv-pd:Income a skos:Concept,
        dpv:Concept ;
    dct:created "2019-06-04"^^xsd:date ;
    dct:creator "Elmar Kiesling; Harshvardhan J. Pandit"^^xsd:string,
        "Fajar Ekaputra"^^xsd:string ;
    sw:term_status "accepted"@en ;
    skos:definition "Information about financial income e.g. for individual or household or family"@en ;
    skos:prefLabel "Income"@en ;
    skos:scopeNote <https://enterprivacy.com/wp-content/uploads/2018/09/Categories-of-Personal-Information.pdf> ;
    dpv:isSubTypeOf dpv-pd:Transactional .

dpv-pd:IncomeBracket a skos:Concept,
        dpv:Concept ;
    dct:created "2019-06-04"^^xsd:date ;
    dct:creator "Elmar Kiesling; Harshvardhan J. Pandit"^^xsd:string,
        "Fajar Ekaputra"^^xsd:string ;
    sw:term_status "accepted"@en ;
    skos:definition "Information about income bracket."@en ;
    skos:prefLabel "Income Bracket"@en ;
    skos:scopeNote <https://enterprivacy.com/wp-content/uploads/2018/09/Categories-of-Personal-Information.pdf> ;
    dpv:isSubTypeOf dpv-pd:Demographic .

dpv-pd:IndividualHealthHistory a skos:Concept,
        dpv:Concept ;
    dct:created "2019-06-04"^^xsd:date ;
    dct:creator "Elmar Kiesling; Harshvardhan J. Pandit"^^xsd:string,
        "Fajar Ekaputra"^^xsd:string ;
    sw:term_status "accepted"@en ;
    skos:definition "Information about information health history."@en ;
    skos:prefLabel "Individual Health History"@en ;
    skos:scopeNote <https://enterprivacy.com/wp-content/uploads/2018/09/Categories-of-Personal-Information.pdf> ;
    dpv:isSubTypeOf dpv-pd:HealthHistory .

dpv-pd:Intention a skos:Concept,
        dpv:Concept ;
    dct:created "2019-06-04"^^xsd:date ;
    dct:creator "Elmar Kiesling; Harshvardhan J. Pandit"^^xsd:string,
        "Fajar Ekaputra"^^xsd:string ;
    sw:term_status "accepted"@en ;
    skos:definition "Information about intentions"@en ;
    skos:prefLabel "Intention"@en ;
    skos:scopeNote <https://enterprivacy.com/wp-content/uploads/2018/09/Categories-of-Personal-Information.pdf> ;
    dpv:isSubTypeOf dpv-pd:Preference .

dpv-pd:Interaction a skos:Concept,
        dpv:Concept ;
    dct:created "2019-06-04"^^xsd:date ;
    dct:creator "Elmar Kiesling; Harshvardhan J. Pandit"^^xsd:string,
        "Fajar Ekaputra"^^xsd:string ;
    sw:term_status "accepted"@en ;
    skos:definition "Information about interactions in the public sphere"@en ;
    skos:prefLabel "Interaction"@en ;
    skos:scopeNote <https://enterprivacy.com/wp-content/uploads/2018/09/Categories-of-Personal-Information.pdf> ;
    dpv:isSubTypeOf dpv-pd:PublicLife .

dpv-pd:Job a skos:Concept,
        dpv:Concept ;
    dct:created "2019-06-04"^^xsd:date ;
    dct:creator "Elmar Kiesling; Harshvardhan J. Pandit"^^xsd:string,
        "Fajar Ekaputra"^^xsd:string ;
    sw:term_status "accepted"@en ;
    skos:definition "Information about professional jobs"@en ;
    skos:prefLabel "Job"@en ;
    skos:scopeNote <https://enterprivacy.com/wp-content/uploads/2018/09/Categories-of-Personal-Information.pdf> ;
    dpv:isSubTypeOf dpv-pd:Professional .

dpv-pd:LifeHistory a skos:Concept,
        dpv:Concept ;
    dct:created "2019-06-04"^^xsd:date ;
    dct:creator "Elmar Kiesling; Harshvardhan J. Pandit"^^xsd:string,
        "Fajar Ekaputra"^^xsd:string ;
    sw:term_status "accepted"@en ;
    skos:definition "Information about personal history regarding events or activities - including  their occurrences that might be directly related or have had an influence (e.g. World War, 9/11)"@en ;
    skos:prefLabel "Life History"@en ;
    skos:scopeNote <https://enterprivacy.com/wp-content/uploads/2018/09/Categories-of-Personal-Information.pdf> ;
    dpv:isSubTypeOf dpv-pd:Historical .

dpv-pd:Like a skos:Concept,
        dpv:Concept ;
    dct:created "2019-06-04"^^xsd:date ;
    dct:creator "Elmar Kiesling; Harshvardhan J. Pandit"^^xsd:string,
        "Fajar Ekaputra"^^xsd:string ;
    sw:term_status "accepted"@en ;
    skos:definition "Information about likes or preferences regarding attractions."@en ;
    skos:prefLabel "Like"@en ;
    skos:scopeNote <https://enterprivacy.com/wp-content/uploads/2018/09/Categories-of-Personal-Information.pdf> ;
    dpv:isSubTypeOf dpv-pd:Interest .

dpv-pd:LinkClicked a skos:Concept,
        dpv:Concept ;
    dct:created "2019-06-04"^^xsd:date ;
    dct:creator "Elmar Kiesling; Harshvardhan J. Pandit"^^xsd:string,
        "Fajar Ekaputra"^^xsd:string ;
    sw:term_status "accepted"@en ;
    skos:definition "Information about the links that an individual has clicked."@en ;
    skos:prefLabel "LinkClicked"@en ;
    skos:related svd:Navigation ;
    skos:scopeNote <https://enterprivacy.com/wp-content/uploads/2018/09/Categories-of-Personal-Information.pdf> ;
    dpv:isSubTypeOf dpv-pd:Behavioral .

dpv-pd:LoanRecord a skos:Concept,
        dpv:Concept ;
    dct:created "2019-06-04"^^xsd:date ;
    dct:creator "Elmar Kiesling; Harshvardhan J. Pandit"^^xsd:string,
        "Fajar Ekaputra"^^xsd:string ;
    sw:term_status "accepted"@en ;
    skos:definition "Information about loans, whether applied, provided or rejected, and its history"@en ;
    skos:prefLabel "Loan Record"@en ;
    skos:scopeNote <https://enterprivacy.com/wp-content/uploads/2018/09/Categories-of-Personal-Information.pdf> ;
    dpv:isSubTypeOf dpv-pd:Transactional .

dpv-pd:MACAddress a skos:Concept,
        dpv:Concept ;
    dct:created "2019-06-04"^^xsd:date ;
    dct:creator "Elmar Kiesling; Harshvardhan J. Pandit"^^xsd:string,
        "Fajar Ekaputra"^^xsd:string ;
    sw:term_status "accepted"@en ;
    skos:definition "Information about the Media Access Control (MAC) address of a device"@en ;
    skos:prefLabel "MAC Address"@en ;
    skos:scopeNote <https://enterprivacy.com/wp-content/uploads/2018/09/Categories-of-Personal-Information.pdf> ;
    dpv:isSubTypeOf dpv-pd:DeviceBased .

dpv-pd:MaritalStatus a skos:Concept,
        dpv:Concept ;
    dct:created "2019-06-04"^^xsd:date ;
    dct:creator "Elmar Kiesling; Harshvardhan J. Pandit"^^xsd:string,
        "Fajar Ekaputra"^^xsd:string ;
    sw:term_status "accepted"@en ;
    skos:definition "Information about marital status and history"@en ;
    skos:prefLabel "Marital Status"@en ;
    skos:scopeNote <https://enterprivacy.com/wp-content/uploads/2018/09/Categories-of-Personal-Information.pdf> ;
    dpv:isSubTypeOf dpv-pd:PublicLife .

dpv-pd:Marriage a skos:Concept,
        dpv:Concept ;
    dct:created "2019-06-04"^^xsd:date ;
    dct:creator "Elmar Kiesling; Harshvardhan J. Pandit"^^xsd:string,
        "Fajar Ekaputra"^^xsd:string ;
    sw:term_status "accepted"@en ;
    skos:definition "Information about marriage(s)."@en ;
    skos:prefLabel "Marriage"@en ;
    skos:scopeNote <https://enterprivacy.com/wp-content/uploads/2018/09/Categories-of-Personal-Information.pdf> ;
    dpv:isSubTypeOf dpv-pd:FamilyStructure .

dpv-pd:MentalHealth a skos:Concept,
        dpv:Concept ;
    dct:created "2019-06-04"^^xsd:date ;
    dct:creator "Elmar Kiesling; Harshvardhan J. Pandit"^^xsd:string,
        "Fajar Ekaputra"^^xsd:string ;
    sw:term_status "accepted"@en ;
    skos:definition "Information about mental health."@en ;
    skos:prefLabel "Mental Health"@en ;
    skos:scopeNote <https://enterprivacy.com/wp-content/uploads/2018/09/Categories-of-Personal-Information.pdf> ;
    dpv:isSubTypeOf dpv-pd:Health .

dpv-pd:Name a skos:Concept,
        dpv:Concept ;
    dct:created "2019-06-04"^^xsd:date ;
    dct:creator "Elmar Kiesling; Harshvardhan J. Pandit"^^xsd:string,
        "Fajar Ekaputra"^^xsd:string ;
    sw:term_status "accepted"@en ;
    skos:definition "Information about names associated or used as given name or nickname."@en ;
    skos:prefLabel "Name"@en ;
    skos:scopeNote <https://enterprivacy.com/wp-content/uploads/2018/09/Categories-of-Personal-Information.pdf> ;
    dpv:isSubTypeOf dpv-pd:Identifying .

dpv-pd:OfficialID a skos:Concept,
        dpv:Concept ;
    dct:created "2019-06-04"^^xsd:date ;
    dct:creator "Elmar Kiesling; Harshvardhan J. Pandit"^^xsd:string,
        "Fajar Ekaputra"^^xsd:string ;
    sw:term_status "accepted"@en ;
    skos:definition "Information about an official identifier or identification document"@en ;
    skos:prefLabel "Official ID"@en ;
    skos:related svd:Government ;
    skos:scopeNote <https://enterprivacy.com/wp-content/uploads/2018/09/Categories-of-Personal-Information.pdf> ;
    dpv:isSubTypeOf dpv-pd:Identifying .

dpv-pd:Offspring a skos:Concept,
        dpv:Concept ;
    dct:created "2019-06-04"^^xsd:date ;
    dct:creator "Elmar Kiesling; Harshvardhan J. Pandit"^^xsd:string,
        "Fajar Ekaputra"^^xsd:string ;
    sw:term_status "accepted"@en ;
    skos:definition "Information about offspring(s)."@en ;
    skos:prefLabel "Offspring"@en ;
    skos:scopeNote <https://enterprivacy.com/wp-content/uploads/2018/09/Categories-of-Personal-Information.pdf> ;
    dpv:isSubTypeOf dpv-pd:FamilyStructure .

dpv-pd:Opinion a skos:Concept,
        dpv:Concept ;
    dct:created "2019-06-04"^^xsd:date ;
    dct:creator "Elmar Kiesling; Harshvardhan J. Pandit"^^xsd:string,
        "Fajar Ekaputra"^^xsd:string ;
    sw:term_status "accepted"@en ;
    skos:definition "Information about opinions"@en ;
    skos:prefLabel "Opinion"@en ;
    skos:scopeNote <https://enterprivacy.com/wp-content/uploads/2018/09/Categories-of-Personal-Information.pdf> ;
    dpv:isSubTypeOf dpv-pd:Preference .

dpv-pd:PINCode a skos:Concept,
        dpv:Concept ;
    dct:created "2019-06-04"^^xsd:date ;
    dct:creator "Elmar Kiesling; Harshvardhan J. Pandit"^^xsd:string,
        "Fajar Ekaputra"^^xsd:string ;
    sw:term_status "accepted"@en ;
    skos:definition "Information about Personal identification number (PIN), which is usually used in the process of authenticating the individual as an user accessing a system."@en ;
    skos:prefLabel "PIN Code"@en ;
    skos:scopeNote <https://enterprivacy.com/wp-content/uploads/2018/09/Categories-of-Personal-Information.pdf> ;
    dpv:isSubTypeOf dpv-pd:Authenticating .

dpv-pd:Parent a skos:Concept,
        dpv:Concept ;
    dct:created "2019-06-04"^^xsd:date ;
    dct:creator "Elmar Kiesling; Harshvardhan J. Pandit"^^xsd:string,
        "Fajar Ekaputra"^^xsd:string ;
    sw:term_status "accepted"@en ;
    skos:definition "Information about parent(s)."@en ;
    skos:prefLabel "Parent"@en ;
    skos:scopeNote <https://enterprivacy.com/wp-content/uploads/2018/09/Categories-of-Personal-Information.pdf> ;
    dpv:isSubTypeOf dpv-pd:FamilyStructure .

dpv-pd:Password a skos:Concept,
        dpv:Concept ;
    dct:created "2019-06-04"^^xsd:date ;
    dct:creator "Elmar Kiesling; Harshvardhan J. Pandit"^^xsd:string,
        "Fajar Ekaputra"^^xsd:string ;
    sw:term_status "accepted"@en ;
    skos:definition "Information about password used in the process of authenticating the individual as an user accessing a system."@en ;
    skos:prefLabel "Password"@en ;
    skos:scopeNote <https://enterprivacy.com/wp-content/uploads/2018/09/Categories-of-Personal-Information.pdf> ;
    dpv:isSubTypeOf dpv-pd:Authenticating .

dpv-pd:PaymentCardExpiry a skos:Concept,
        dpv:Concept ;
    dct:created "2020-11-04"^^xsd:date ;
    dct:creator "Georg P Krog"^^xsd:string ;
    sw:term_status "accepted"@en ;
    skos:definition "Information about payment card expiry such as a date."@en ;
    skos:prefLabel "Payment Card Expiry"@en ;
    skos:scopeNote <https://www.w3.org/community/dpvcg/> ;
    dpv:isSubTypeOf dpv-pd:PaymentCard .

dpv-pd:PersonalPossession a skos:Concept,
        dpv:Concept ;
    dct:created "2019-06-04"^^xsd:date ;
    dct:creator "Elmar Kiesling; Harshvardhan J. Pandit"^^xsd:string,
        "Fajar Ekaputra"^^xsd:string ;
    sw:term_status "accepted"@en ;
    skos:definition "Information about personal possessions."@en ;
    skos:prefLabel "Personal Possession"@en ;
    skos:scopeNote <https://enterprivacy.com/wp-content/uploads/2018/09/Categories-of-Personal-Information.pdf> ;
    dpv:isSubTypeOf dpv-pd:Ownership .

dpv-pd:Personality a skos:Concept,
        dpv:Concept ;
    dct:created "2019-06-04"^^xsd:date ;
    dct:creator "Elmar Kiesling; Harshvardhan J. Pandit"^^xsd:string,
        "Fajar Ekaputra"^^xsd:string ;
    sw:term_status "accepted"@en ;
    skos:definition "Information about personality (e.g., categorization in terms of the Big Five personality traits)"@en ;
    skos:prefLabel "Personality"@en ;
    skos:scopeNote <https://enterprivacy.com/wp-content/uploads/2018/09/Categories-of-Personal-Information.pdf> ;
    dpv:isSubTypeOf dpv-pd:Behavioral .

dpv-pd:PhilosophicalBelief a skos:Concept,
        dpv:Concept ;
    dct:created "2019-06-04"^^xsd:date ;
    dct:creator "Elmar Kiesling; Harshvardhan J. Pandit"^^xsd:string,
        "Fajar Ekaputra"^^xsd:string ;
    sw:term_status "accepted"@en ;
    skos:definition "Information about philosophical beliefs."@en ;
    skos:prefLabel "Philosophical Belief"@en ;
    skos:scopeNote <https://enterprivacy.com/wp-content/uploads/2018/09/Categories-of-Personal-Information.pdf> ;
    dpv:isSubTypeOf dpv:SpecialCategoryPersonalData,
        dpv-pd:KnowledgeBelief .

dpv-pd:PhysicalAddress a skos:Concept,
        dpv:Concept ;
    dct:created "2019-06-04"^^xsd:date ;
    dct:creator "Elmar Kiesling; Harshvardhan J. Pandit"^^xsd:string,
        "Fajar Ekaputra"^^xsd:string ;
    sw:term_status "accepted"@en ;
    skos:definition "Information about physical address."@en ;
    skos:prefLabel "Physical Address"@en ;
    skos:scopeNote <https://enterprivacy.com/wp-content/uploads/2018/09/Categories-of-Personal-Information.pdf> ;
    dpv:isSubTypeOf dpv-pd:Contact .

dpv-pd:PhysicalHealth a skos:Concept,
        dpv:Concept ;
    dct:created "2019-06-04"^^xsd:date ;
    dct:creator "Elmar Kiesling; Harshvardhan J. Pandit"^^xsd:string,
        "Fajar Ekaputra"^^xsd:string ;
    sw:term_status "accepted"@en ;
    skos:definition "Information about physical health."@en ;
    skos:prefLabel "Physical Health"@en ;
    skos:scopeNote <https://enterprivacy.com/wp-content/uploads/2018/09/Categories-of-Personal-Information.pdf> ;
    dpv:isSubTypeOf dpv-pd:Health .

dpv-pd:PhysicalTrait a skos:Concept,
        dpv:Concept ;
    dct:created "2019-06-04"^^xsd:date ;
    dct:creator "Elmar Kiesling; Harshvardhan J. Pandit"^^xsd:string,
        "Fajar Ekaputra"^^xsd:string ;
    sw:term_status "accepted"@en ;
    skos:definition "Information about defining traits or features regarding the body."@en ;
    skos:prefLabel "Physical Trait"@en ;
    skos:scopeNote <https://enterprivacy.com/wp-content/uploads/2018/09/Categories-of-Personal-Information.pdf> ;
    dpv:isSubTypeOf dpv-pd:Demographic .

dpv-pd:Picture a skos:Concept,
        dpv:Concept ;
    dct:created "2019-06-04"^^xsd:date ;
    dct:creator "Elmar Kiesling; Harshvardhan J. Pandit"^^xsd:string,
        "Fajar Ekaputra"^^xsd:string ;
    sw:term_status "accepted"@en ;
    skos:definition "Information about visual representation or image e.g. profile photo."@en ;
    skos:prefLabel "Picture"@en ;
    skos:scopeNote <https://enterprivacy.com/wp-content/uploads/2018/09/Categories-of-Personal-Information.pdf> ;
    dpv:isSubTypeOf dpv-pd:Identifying .

dpv-pd:Piercing a skos:Concept,
        dpv:Concept ;
    dct:created "2019-06-04"^^xsd:date ;
    dct:creator "Elmar Kiesling; Harshvardhan J. Pandit"^^xsd:string,
        "Fajar Ekaputra"^^xsd:string ;
    sw:term_status "accepted"@en ;
    skos:definition "Information about piercings"@en ;
    skos:prefLabel "Piercing"@en ;
    skos:scopeNote <https://enterprivacy.com/wp-content/uploads/2018/09/Categories-of-Personal-Information.pdf> ;
    dpv:isSubTypeOf dpv-pd:PhysicalCharacteristic .

dpv-pd:PoliticalAffiliation a skos:Concept,
        dpv:Concept ;
    dct:created "2019-06-04"^^xsd:date ;
    dct:creator "Elmar Kiesling; Harshvardhan J. Pandit"^^xsd:string,
        "Fajar Ekaputra"^^xsd:string ;
    sw:term_status "accepted"@en ;
    skos:definition "Information about political affiliation and history"@en ;
    skos:prefLabel "Political Affiliation"@en ;
    skos:related svd:Political ;
    skos:scopeNote <https://enterprivacy.com/wp-content/uploads/2018/09/Categories-of-Personal-Information.pdf> ;
    dpv:isSubTypeOf dpv:SpecialCategoryPersonalData,
        dpv-pd:PublicLife .

dpv-pd:Prescription a skos:Concept,
        dpv:Concept ;
    dct:created "2019-06-04"^^xsd:date ;
    dct:creator "Elmar Kiesling; Harshvardhan J. Pandit"^^xsd:string,
        "Fajar Ekaputra"^^xsd:string ;
    sw:term_status "accepted"@en ;
    skos:definition "Information about medical and pharmaceutical prescriptions"@en ;
    skos:prefLabel "Prescription"@en ;
    skos:scopeNote <https://enterprivacy.com/wp-content/uploads/2018/09/Categories-of-Personal-Information.pdf> ;
    dpv:isSubTypeOf dpv-pd:MedicalHealth .

dpv-pd:PrivacyPreference a skos:Concept,
        dpv:Concept ;
    dct:created "2019-06-04"^^xsd:date ;
    dct:creator "Elmar Kiesling; Harshvardhan J. Pandit"^^xsd:string,
        "Fajar Ekaputra"^^xsd:string ;
    sw:term_status "accepted"@en ;
    skos:definition "Information about privacy preferences"@en ;
    skos:prefLabel "Privacy Preference"@en ;
    skos:scopeNote <https://enterprivacy.com/wp-content/uploads/2018/09/Categories-of-Personal-Information.pdf> ;
    dpv:isSubTypeOf dpv-pd:Preference .

dpv-pd:Proclivitie a skos:Concept,
        dpv:Concept ;
    dct:created "2019-06-04"^^xsd:date ;
    dct:creator "Elmar Kiesling; Harshvardhan J. Pandit"^^xsd:string,
        "Fajar Ekaputra"^^xsd:string ;
    sw:term_status "accepted"@en ;
    skos:definition "Information about proclivities in a sexual context"@en ;
    skos:prefLabel "Proclivitie"@en ;
    skos:scopeNote <https://enterprivacy.com/wp-content/uploads/2018/09/Categories-of-Personal-Information.pdf> ;
    dpv:isSubTypeOf dpv-pd:Sexual .

dpv-pd:ProfessionalCertification a skos:Concept,
        dpv:Concept ;
    dct:created "2019-06-04"^^xsd:date ;
    dct:creator "Elmar Kiesling; Harshvardhan J. Pandit"^^xsd:string,
        "Fajar Ekaputra"^^xsd:string ;
    sw:term_status "accepted"@en ;
    skos:definition "Information about professional certifications"@en ;
    skos:prefLabel "Professional Certification"@en ;
    skos:scopeNote <https://enterprivacy.com/wp-content/uploads/2018/09/Categories-of-Personal-Information.pdf> ;
    dpv:isSubTypeOf dpv-pd:Professional .

dpv-pd:ProfessionalEvaluation a skos:Concept,
        dpv:Concept ;
    dct:created "2019-06-04"^^xsd:date ;
    dct:creator "Elmar Kiesling; Harshvardhan J. Pandit"^^xsd:string,
        "Fajar Ekaputra"^^xsd:string ;
    sw:term_status "accepted"@en ;
    skos:definition "Information about professional evaluations"@en ;
    skos:prefLabel "Professional Evaluation"@en ;
    skos:scopeNote <https://enterprivacy.com/wp-content/uploads/2018/09/Categories-of-Personal-Information.pdf> ;
    dpv:isSubTypeOf dpv-pd:Professional .

dpv-pd:ProfessionalInterview a skos:Concept,
        dpv:Concept ;
    dct:created "2019-06-04"^^xsd:date ;
    dct:creator "Elmar Kiesling; Harshvardhan J. Pandit"^^xsd:string,
        "Fajar Ekaputra"^^xsd:string ;
    sw:term_status "accepted"@en ;
    skos:definition "Information about professional interviews"@en ;
    skos:prefLabel "Professional Interview"@en ;
    skos:scopeNote <https://enterprivacy.com/wp-content/uploads/2018/09/Categories-of-Personal-Information.pdf> ;
    dpv:isSubTypeOf dpv-pd:Professional .

dpv-pd:Purchase a skos:Concept,
        dpv:Concept ;
    dct:created "2019-06-04"^^xsd:date ;
    dct:creator "Elmar Kiesling; Harshvardhan J. Pandit"^^xsd:string,
        "Fajar Ekaputra"^^xsd:string ;
    sw:term_status "accepted"@en ;
    skos:definition "Information about purchases such as items bought e.g. grocery or clothing"@en ;
    skos:prefLabel "Purchase"@en ;
    skos:related svd:Purchase ;
    skos:scopeNote <https://enterprivacy.com/wp-content/uploads/2018/09/Categories-of-Personal-Information.pdf> ;
    dpv:isSubTypeOf dpv-pd:Transactional .

dpv-pd:PurchasesAndSpendingHabit a skos:Concept,
        dpv:Concept ;
    dct:created "2019-06-04"^^xsd:date ;
    dct:creator "Elmar Kiesling; Harshvardhan J. Pandit"^^xsd:string,
        "Fajar Ekaputra"^^xsd:string ;
    sw:term_status "accepted"@en ;
    skos:definition "Information about analysis of purchases made and money spent expressed as a habit e.g. monthly shopping trends"@en ;
    skos:prefLabel "Purchases and Spending Habit"@en ;
    skos:scopeNote <https://enterprivacy.com/wp-content/uploads/2018/09/Categories-of-Personal-Information.pdf> ;
    dpv:isSubTypeOf dpv-pd:Transactional .

dpv-pd:Race a skos:Concept,
        dpv:Concept ;
    dct:created "2019-06-04"^^xsd:date ;
    dct:creator "Elmar Kiesling; Harshvardhan J. Pandit"^^xsd:string,
        "Fajar Ekaputra"^^xsd:string ;
    sw:term_status "accepted"@en ;
    skos:definition "Information about race or racial history."@en ;
    skos:prefLabel "Race"@en ;
    skos:scopeNote <https://enterprivacy.com/wp-content/uploads/2018/09/Categories-of-Personal-Information.pdf> ;
    dpv:isSubTypeOf dpv:SpecialCategoryPersonalData,
        dpv-pd:Ethnicity .

dpv-pd:Reference a skos:Concept,
        dpv:Concept ;
    dct:created "2019-06-04"^^xsd:date ;
    dct:creator "Elmar Kiesling; Harshvardhan J. Pandit"^^xsd:string,
        "Fajar Ekaputra"^^xsd:string ;
    sw:term_status "accepted"@en ;
    skos:definition "Information about references in the professional context"@en ;
    skos:prefLabel "Reference"@en ;
    skos:scopeNote <https://enterprivacy.com/wp-content/uploads/2018/09/Categories-of-Personal-Information.pdf> ;
    dpv:isSubTypeOf dpv-pd:Professional .

dpv-pd:Relationship a skos:Concept,
        dpv:Concept ;
    dct:created "2019-06-04"^^xsd:date ;
    dct:creator "Elmar Kiesling; Harshvardhan J. Pandit"^^xsd:string,
        "Fajar Ekaputra"^^xsd:string ;
    sw:term_status "accepted"@en ;
    skos:definition "Information about relationships and relationship history."@en ;
    skos:prefLabel "Relationship"@en ;
    skos:scopeNote <https://enterprivacy.com/wp-content/uploads/2018/09/Categories-of-Personal-Information.pdf> ;
    dpv:isSubTypeOf dpv-pd:Family .

dpv-pd:Religion a skos:Concept,
        dpv:Concept ;
    dct:created "2019-06-04"^^xsd:date ;
    dct:creator "Elmar Kiesling; Harshvardhan J. Pandit"^^xsd:string,
        "Fajar Ekaputra"^^xsd:string ;
    sw:term_status "accepted"@en ;
    skos:definition "Information about religion, religious inclinations, and religious history."@en ;
    skos:prefLabel "Religion"@en ;
    skos:scopeNote <https://enterprivacy.com/wp-content/uploads/2018/09/Categories-of-Personal-Information.pdf> ;
    dpv:isSubTypeOf dpv:SpecialCategoryPersonalData,
        dpv-pd:PublicLife .

dpv-pd:ReligiousBelief a skos:Concept,
        dpv:Concept ;
    dct:created "2019-06-04"^^xsd:date ;
    dct:creator "Elmar Kiesling; Harshvardhan J. Pandit"^^xsd:string,
        "Fajar Ekaputra"^^xsd:string ;
    sw:term_status "accepted"@en ;
    skos:definition "Information about religion and religious beliefs."@en ;
    skos:prefLabel "Religious Belief"@en ;
    skos:scopeNote <https://enterprivacy.com/wp-content/uploads/2018/09/Categories-of-Personal-Information.pdf> ;
    dpv:isSubTypeOf dpv:SpecialCategoryPersonalData,
        dpv-pd:KnowledgeBelief .

dpv-pd:Retina a skos:Concept,
        dpv:Concept ;
    dct:created "2019-06-04"^^xsd:date ;
    dct:creator "Elmar Kiesling; Harshvardhan J. Pandit"^^xsd:string,
        "Fajar Ekaputra"^^xsd:string ;
    sw:term_status "accepted"@en ;
    skos:definition "Information about retina and the retinal patterns."@en ;
    skos:prefLabel "Retina"@en ;
    skos:scopeNote <https://enterprivacy.com/wp-content/uploads/2018/09/Categories-of-Personal-Information.pdf> ;
    dpv:isSubTypeOf dpv-pd:Biometric .

dpv-pd:RoomNumber a skos:Concept,
        dpv:Concept ;
    dct:created "2019-06-04"^^xsd:date ;
    dct:creator "Elmar Kiesling; Harshvardhan J. Pandit"^^xsd:string,
        "Fajar Ekaputra"^^xsd:string ;
    sw:term_status "accepted"@en ;
    skos:definition "Information about location expressed as Room number or similar numbering systems"@en ;
    skos:prefLabel "Room Number"@en ;
    skos:scopeNote <https://enterprivacy.com/wp-content/uploads/2018/09/Categories-of-Personal-Information.pdf> ;
    dpv:isSubTypeOf dpv-pd:Location .

dpv-pd:Salary a skos:Concept,
        dpv:Concept ;
    dct:created "2019-06-04"^^xsd:date ;
    dct:creator "Elmar Kiesling; Harshvardhan J. Pandit"^^xsd:string,
        "Fajar Ekaputra"^^xsd:string ;
    sw:term_status "accepted"@en ;
    skos:definition "Information about salary"@en ;
    skos:prefLabel "Salary"@en ;
    skos:scopeNote <https://enterprivacy.com/wp-content/uploads/2018/09/Categories-of-Personal-Information.pdf> ;
    dpv:isSubTypeOf dpv-pd:Professional .

dpv-pd:Sale a skos:Concept,
        dpv:Concept ;
    dct:created "2019-06-04"^^xsd:date ;
    dct:creator "Elmar Kiesling; Harshvardhan J. Pandit"^^xsd:string,
        "Fajar Ekaputra"^^xsd:string ;
    sw:term_status "accepted"@en ;
    skos:definition "Information about sales e.g. selling of goods or services"@en ;
    skos:prefLabel "Sale"@en ;
    skos:scopeNote <https://enterprivacy.com/wp-content/uploads/2018/09/Categories-of-Personal-Information.pdf> ;
    dpv:isSubTypeOf dpv-pd:Transactional .

dpv-pd:School a skos:Concept,
        dpv:Concept ;
    dct:created "2019-06-04"^^xsd:date ;
    dct:creator "Elmar Kiesling; Harshvardhan J. Pandit"^^xsd:string,
        "Fajar Ekaputra"^^xsd:string ;
    sw:term_status "accepted"@en ;
    skos:definition "Information about school such as name of school, conduct, or grades obtained."@en ;
    skos:prefLabel "School"@en ;
    skos:scopeNote <https://enterprivacy.com/wp-content/uploads/2018/09/Categories-of-Personal-Information.pdf> ;
    dpv:isSubTypeOf dpv-pd:Professional .

dpv-pd:SecretText a skos:Concept,
        dpv:Concept ;
    dct:created "2019-06-04"^^xsd:date ;
    dct:creator "Elmar Kiesling; Harshvardhan J. Pandit"^^xsd:string,
        "Fajar Ekaputra"^^xsd:string ;
    sw:term_status "accepted"@en ;
    skos:definition "Information about secret text used in the process of authenticating the individual as an user accessing a system, e.g., when recovering a lost password."@en ;
    skos:prefLabel "Secret Text"@en ;
    skos:scopeNote <https://enterprivacy.com/wp-content/uploads/2018/09/Categories-of-Personal-Information.pdf> ;
    dpv:isSubTypeOf dpv-pd:Authenticating .

dpv-pd:SexualHistory a skos:Concept,
        dpv:Concept ;
    dct:created "2019-06-04"^^xsd:date ;
    dct:creator "Elmar Kiesling; Harshvardhan J. Pandit"^^xsd:string,
        "Fajar Ekaputra"^^xsd:string ;
    sw:term_status "accepted"@en ;
    skos:definition "Information about sexual history"@en ;
    skos:prefLabel "Sexual History"@en ;
    skos:scopeNote <https://enterprivacy.com/wp-content/uploads/2018/09/Categories-of-Personal-Information.pdf> ;
    dpv:isSubTypeOf dpv-pd:Sexual .

dpv-pd:SexualPreference a skos:Concept,
        dpv:Concept ;
    dct:created "2019-06-04"^^xsd:date ;
    dct:creator "Elmar Kiesling; Harshvardhan J. Pandit"^^xsd:string,
        "Fajar Ekaputra"^^xsd:string ;
    sw:term_status "accepted"@en ;
    skos:definition "Information about sexual preferences"@en ;
    skos:prefLabel "Sexual Preference"@en ;
    skos:scopeNote <https://enterprivacy.com/wp-content/uploads/2018/09/Categories-of-Personal-Information.pdf> ;
    dpv:isSubTypeOf dpv-pd:Sexual .

dpv-pd:Sibling a skos:Concept,
        dpv:Concept ;
    dct:created "2019-06-04"^^xsd:date ;
    dct:creator "Elmar Kiesling; Harshvardhan J. Pandit"^^xsd:string,
        "Fajar Ekaputra"^^xsd:string ;
    sw:term_status "accepted"@en ;
    skos:definition "Information about sibling(s)."@en ;
    skos:prefLabel "Sibling"@en ;
    skos:scopeNote <https://enterprivacy.com/wp-content/uploads/2018/09/Categories-of-Personal-Information.pdf> ;
    dpv:isSubTypeOf dpv-pd:FamilyStructure .

dpv-pd:SkinTone a skos:Concept,
        dpv:Concept ;
    dct:created "2019-06-04"^^xsd:date ;
    dct:creator "Elmar Kiesling; Harshvardhan J. Pandit"^^xsd:string,
        "Fajar Ekaputra"^^xsd:string ;
    sw:term_status "accepted"@en ;
    skos:definition "Information about skin tone"@en ;
    skos:prefLabel "Skin Tone"@en ;
    skos:scopeNote <https://enterprivacy.com/wp-content/uploads/2018/09/Categories-of-Personal-Information.pdf> ;
    dpv:isSubTypeOf dpv-pd:PhysicalCharacteristic .

dpv-pd:SocialMediaCommunication a skos:Concept,
        dpv:Concept ;
    dct:created "2019-06-04"^^xsd:date ;
    dct:creator "Elmar Kiesling; Harshvardhan J. Pandit"^^xsd:string,
        "Fajar Ekaputra"^^xsd:string ;
    sw:term_status "accepted"@en ;
    skos:definition "Information about social media communication, including the communication itself and metadata."@en ;
    skos:prefLabel "Social Media Communication"@en ;
    skos:related svd:Social ;
    skos:scopeNote <https://enterprivacy.com/wp-content/uploads/2018/09/Categories-of-Personal-Information.pdf> ;
    dpv:isSubTypeOf dpv-pd:Communication .

dpv-pd:SocialStatus a skos:Concept,
        dpv:Concept ;
    dct:created "2019-06-04"^^xsd:date ;
    dct:creator "Elmar Kiesling; Harshvardhan J. Pandit"^^xsd:string,
        "Fajar Ekaputra"^^xsd:string ;
    sw:term_status "accepted"@en ;
    skos:definition "Information about social status"@en ;
    skos:prefLabel "Social Status"@en ;
    skos:scopeNote <https://enterprivacy.com/wp-content/uploads/2018/09/Categories-of-Personal-Information.pdf> ;
    dpv:isSubTypeOf dpv-pd:PublicLife .

dpv-pd:TVViewingBehavior a skos:Concept,
        dpv:Concept ;
    dct:created "2019-11-26"^^xsd:date ;
    dct:creator "Harshvardhan J. Pandit"^^xsd:string,
        "Rudy Jacob"^^xsd:string ;
    sw:term_status "accepted"@en ;
    skos:definition "Information about TV viewing Behavior, such as timestamps of channel change, duration of viewership, content consumed"@en ;
    skos:prefLabel "TV Viewing Behavior"@en ;
    skos:scopeNote <https://www.specialprivacy.eu/> ;
    dpv:isSubTypeOf dpv-pd:ServiceConsumptionBehavior .

dpv-pd:Tattoo a skos:Concept,
        dpv:Concept ;
    dct:created "2019-06-04"^^xsd:date ;
    dct:creator "Elmar Kiesling; Harshvardhan J. Pandit"^^xsd:string,
        "Fajar Ekaputra"^^xsd:string ;
    sw:term_status "accepted"@en ;
    skos:definition "Information about tattoos"@en ;
    skos:prefLabel "Tattoo"@en ;
    skos:scopeNote <https://enterprivacy.com/wp-content/uploads/2018/09/Categories-of-Personal-Information.pdf> ;
    dpv:isSubTypeOf dpv-pd:PhysicalCharacteristic .

dpv-pd:Tax a skos:Concept,
        dpv:Concept ;
    dct:created "2019-06-04"^^xsd:date ;
    dct:creator "Elmar Kiesling; Harshvardhan J. Pandit"^^xsd:string,
        "Fajar Ekaputra"^^xsd:string ;
    sw:term_status "accepted"@en ;
    skos:definition "Information about financial tax e.g. tax records or tax due"@en ;
    skos:prefLabel "Tax"@en ;
    skos:scopeNote <https://enterprivacy.com/wp-content/uploads/2018/09/Categories-of-Personal-Information.pdf> ;
    dpv:isSubTypeOf dpv-pd:Transactional .

dpv-pd:TelephoneNumber a skos:Concept,
        dpv:Concept ;
    dct:created "2019-06-04"^^xsd:date ;
    dct:creator "Elmar Kiesling; Harshvardhan J. Pandit"^^xsd:string,
        "Fajar Ekaputra"^^xsd:string ;
    sw:term_status "accepted"@en ;
    skos:definition "Information about telephone number."@en ;
    skos:prefLabel "Telephone Number"@en ;
    skos:scopeNote <https://enterprivacy.com/wp-content/uploads/2018/09/Categories-of-Personal-Information.pdf> ;
    dpv:isSubTypeOf dpv-pd:Contact .

dpv-pd:Thought a skos:Concept,
        dpv:Concept ;
    dct:created "2019-06-04"^^xsd:date ;
    dct:creator "Elmar Kiesling; Harshvardhan J. Pandit"^^xsd:string,
        "Fajar Ekaputra"^^xsd:string ;
    sw:term_status "accepted"@en ;
    skos:definition "Information about thoughts"@en ;
    skos:prefLabel "Thought"@en ;
    skos:scopeNote <https://enterprivacy.com/wp-content/uploads/2018/09/Categories-of-Personal-Information.pdf> ;
    dpv:isSubTypeOf dpv-pd:KnowledgeBelief .

dpv-pd:Transaction a skos:Concept,
        dpv:Concept ;
    dct:created "2019-06-04"^^xsd:date ;
    dct:creator "Elmar Kiesling; Harshvardhan J. Pandit"^^xsd:string,
        "Fajar Ekaputra"^^xsd:string ;
    sw:term_status "accepted"@en ;
    skos:definition "Information about financial transactions e.g. bank transfers"@en ;
    skos:prefLabel "Transaction"@en ;
    skos:scopeNote <https://enterprivacy.com/wp-content/uploads/2018/09/Categories-of-Personal-Information.pdf> ;
    dpv:isSubTypeOf dpv-pd:Transactional .

dpv-pd:UID a skos:Concept,
        dpv:Concept ;
    dct:created "2019-06-04"^^xsd:date ;
    dct:creator "Elmar Kiesling; Harshvardhan J. Pandit"^^xsd:string,
        "Fajar Ekaputra"^^xsd:string ;
    sw:term_status "accepted"@en ;
    skos:definition "Information about unique identifiers."@en ;
    skos:prefLabel "UID"@en ;
    skos:related svd:UniqueId ;
    skos:scopeNote <https://enterprivacy.com/wp-content/uploads/2018/09/Categories-of-Personal-Information.pdf> ;
    dpv:isSubTypeOf dpv-pd:Identifying .

dpv-pd:Username a skos:Concept,
        dpv:Concept ;
    dct:created "2019-06-04"^^xsd:date ;
    dct:creator "Elmar Kiesling; Harshvardhan J. Pandit"^^xsd:string,
        "Fajar Ekaputra"^^xsd:string ;
    sw:term_status "accepted"@en ;
    skos:definition "Information about usernames."@en ;
    skos:prefLabel "Username"@en ;
    skos:scopeNote <https://enterprivacy.com/wp-content/uploads/2018/09/Categories-of-Personal-Information.pdf> ;
    dpv:isSubTypeOf dpv-pd:Identifying .

dpv-pd:VoiceCommunicationRecording a skos:Concept,
        dpv:Concept ;
    dct:created "2019-06-04"^^xsd:date ;
    dct:creator "Elmar Kiesling; Harshvardhan J. Pandit"^^xsd:string,
        "Fajar Ekaputra"^^xsd:string ;
    sw:term_status "accepted"@en ;
    skos:definition "Information about vocal recorded communication (e.g. telephony, VoIP)"@en ;
    skos:prefLabel "Voice Communication Recording"@en ;
    skos:scopeNote <https://enterprivacy.com/wp-content/uploads/2018/09/Categories-of-Personal-Information.pdf> ;
    dpv:isSubTypeOf dpv-pd:Communication .

dpv-pd:VoiceMail a skos:Concept,
        dpv:Concept ;
    dct:created "2019-06-04"^^xsd:date ;
    dct:creator "Elmar Kiesling; Harshvardhan J. Pandit"^^xsd:string,
        "Fajar Ekaputra"^^xsd:string ;
    sw:term_status "accepted"@en ;
    skos:definition "Information about voice mail messages."@en ;
    skos:prefLabel "Voice Mail"@en ;
    skos:scopeNote <https://enterprivacy.com/wp-content/uploads/2018/09/Categories-of-Personal-Information.pdf> ;
    dpv:isSubTypeOf dpv-pd:Communication .

dpv-pd:Weight a skos:Concept,
        dpv:Concept ;
    dct:created "2019-06-04"^^xsd:date ;
    dct:creator "Elmar Kiesling; Harshvardhan J. Pandit"^^xsd:string,
        "Fajar Ekaputra"^^xsd:string ;
    sw:term_status "accepted"@en ;
    skos:definition "Information about physical weight"@en ;
    skos:prefLabel "Weight"@en ;
    skos:scopeNote <https://enterprivacy.com/wp-content/uploads/2018/09/Categories-of-Personal-Information.pdf> ;
    dpv:isSubTypeOf dpv-pd:PhysicalCharacteristic .

dpv-pd:WorkHistory a skos:Concept,
        dpv:Concept ;
    dct:created "2019-06-04"^^xsd:date ;
    dct:creator "Elmar Kiesling; Harshvardhan J. Pandit"^^xsd:string,
        "Fajar Ekaputra"^^xsd:string ;
    sw:term_status "accepted"@en ;
    skos:definition "Information about work history in a professional context"@en ;
    skos:prefLabel "Work History"@en ;
    skos:scopeNote <https://enterprivacy.com/wp-content/uploads/2018/09/Categories-of-Personal-Information.pdf> ;
    dpv:isSubTypeOf dpv-pd:Professional .

dpv-pd:BrowsingBehavior a skos:Concept,
        dpv:Concept ;
    dct:created "2019-06-04"^^xsd:date ;
    dct:creator "Elmar Kiesling; Harshvardhan J. Pandit"^^xsd:string,
        "Fajar Ekaputra"^^xsd:string ;
    sw:term_status "accepted"@en ;
    skos:definition "Information about browsing Behavior."@en ;
    skos:prefLabel "Browsing Behavior"@en ;
    skos:related svd:OnlineActivity ;
    skos:scopeNote <https://enterprivacy.com/wp-content/uploads/2018/09/Categories-of-Personal-Information.pdf> ;
    dpv:isSubTypeOf dpv-pd:Behavioral .

dpv-pd:CreditWorthiness a skos:Concept,
        dpv:Concept ;
    dct:created "2019-06-04"^^xsd:date ;
    dct:creator "Elmar Kiesling; Harshvardhan J. Pandit"^^xsd:string,
        "Fajar Ekaputra"^^xsd:string ;
    sw:term_status "accepted"@en ;
    skos:definition "Information about credit worthiness."@en ;
    skos:prefLabel "Credit Worthiness"@en ;
    skos:scopeNote <https://enterprivacy.com/wp-content/uploads/2018/09/Categories-of-Personal-Information.pdf> ;
    dpv:isSubTypeOf dpv-pd:Credit .

dpv-pd:Historical a skos:Concept,
        dpv:Concept ;
    dct:created "2019-06-04"^^xsd:date ;
    dct:creator "Elmar Kiesling; Harshvardhan J. Pandit"^^xsd:string,
        "Fajar Ekaputra"^^xsd:string ;
    sw:term_status "accepted"@en ;
    skos:definition "Information about historical data related to or relevant regarding history or past events"@en ;
    skos:prefLabel "Historical"@en ;
    skos:scopeNote <https://enterprivacy.com/wp-content/uploads/2018/09/Categories-of-Personal-Information.pdf> ;
    dpv:isSubTypeOf dpv:PersonalData .

dpv-pd:HouseOwned a skos:Concept,
        dpv:Concept ;
    dct:created "2019-06-04"^^xsd:date ;
    dct:creator "Elmar Kiesling; Harshvardhan J. Pandit"^^xsd:string,
        "Fajar Ekaputra"^^xsd:string ;
    sw:term_status "accepted"@en ;
    skos:definition "Information about house(s) owned and ownership history."@en ;
    skos:prefLabel "House Owned"@en ;
    skos:scopeNote <https://enterprivacy.com/wp-content/uploads/2018/09/Categories-of-Personal-Information.pdf> ;
    dpv:isSubTypeOf dpv-pd:Ownership .

dpv-pd:PaymentCardNumber a skos:Concept,
        dpv:Concept ;
    dct:created "2020-11-04"^^xsd:date ;
    dct:creator "Georg P Krog"^^xsd:string ;
    sw:term_status "accepted"@en ;
    skos:definition "Information about payment card number."@en ;
    skos:prefLabel "Payment Card Number"@en ;
    skos:scopeNote <https://www.w3.org/community/dpvcg/> ;
    dpv:isSubTypeOf dpv-pd:AccountIdentifier,
        dpv-pd:PaymentCard .

dpv-pd:ServiceConsumptionBehavior a skos:Concept,
        dpv:Concept ;
    dct:created "2019-11-26"^^xsd:date ;
    dct:creator "Harshvardhan J. Pandit"^^xsd:string,
        "Rudy Jacob"^^xsd:string ;
    sw:term_status "accepted"@en ;
    skos:definition "Information about the consumption of a service, e.g. time and duration of consumption."@en ;
    skos:prefLabel "Service Consumption Behavior"@en ;
    skos:scopeNote <https://www.specialprivacy.eu/> ;
    dpv:isSubTypeOf dpv-pd:Behavioral .

dpv-pd:AccountIdentifier a skos:Concept,
        dpv:Concept ;
    dct:created "2019-06-04"^^xsd:date ;
    dct:creator "Elmar Kiesling; Harshvardhan J. Pandit"^^xsd:string,
        "Fajar Ekaputra"^^xsd:string ;
    sw:term_status "accepted"@en ;
    skos:definition "Information about financial account identifier."@en ;
    skos:prefLabel "Account Identifier"@en ;
    skos:scopeNote <https://enterprivacy.com/wp-content/uploads/2018/09/Categories-of-Personal-Information.pdf> ;
    dpv:isSubTypeOf dpv-pd:FinancialAccount .

dpv-pd:Biometric a skos:Concept,
        dpv:Concept ;
    dct:created "2019-06-04"^^xsd:date ;
    dct:creator "Elmar Kiesling; Harshvardhan J. Pandit"^^xsd:string,
        "Fajar Ekaputra"^^xsd:string ;
    sw:term_status "accepted"@en ;
    skos:definition "Information about biometrics and biometric characteristics."@en ;
    skos:prefLabel "Biometric"@en ;
    skos:scopeNote <https://enterprivacy.com/wp-content/uploads/2018/09/Categories-of-Personal-Information.pdf> ;
    dpv:isSubTypeOf dpv:SpecialCategoryPersonalData,
        dpv-pd:Identifying .

dpv-pd:DeviceSoftware a skos:Concept,
        dpv:Concept ;
    dct:created "2020-11-04"^^xsd:date ;
    dct:creator "Beatriz Esteves"^^xsd:string,
        "Georg P Krog"^^xsd:string,
        "Harshvardhan J. Pandit"^^xsd:string,
        "Paul Ryan"^^xsd:string ;
    sw:term_status "accepted"@en ;
    skos:definition "Information about software on or related to a device."@en ;
    skos:prefLabel "Device Software"@en ;
    skos:scopeNote <https://www.w3.org/community/dpvcg/> ;
    dpv:isSubTypeOf dpv-pd:DeviceBased .

dpv-pd:Family a skos:Concept,
        dpv:Concept ;
    dct:created "2019-06-04"^^xsd:date ;
    dct:creator "Elmar Kiesling; Harshvardhan J. Pandit"^^xsd:string,
        "Fajar Ekaputra"^^xsd:string ;
    sw:term_status "accepted"@en ;
    skos:definition "Information about family and relationships"@en ;
    skos:prefLabel "Family"@en ;
    skos:scopeNote <https://enterprivacy.com/wp-content/uploads/2018/09/Categories-of-Personal-Information.pdf> ;
    dpv:isSubTypeOf dpv-pd:Social .

dpv-pd:Health a skos:Concept,
        dpv:Concept ;
    dct:created "2019-06-04"^^xsd:date ;
    dct:creator "Elmar Kiesling; Harshvardhan J. Pandit"^^xsd:string,
        "Fajar Ekaputra"^^xsd:string ;
    sw:term_status "accepted"@en ;
    skos:definition "Information about health."@en ;
    skos:prefLabel "Health"@en ;
    skos:related svd:Health ;
    skos:scopeNote <https://enterprivacy.com/wp-content/uploads/2018/09/Categories-of-Personal-Information.pdf> ;
    dpv:isSubTypeOf dpv-pd:MedicalHealth .

dpv-pd:HealthHistory a skos:Concept,
        dpv:Concept ;
    dct:created "2019-06-04"^^xsd:date ;
    dct:creator "Elmar Kiesling; Harshvardhan J. Pandit"^^xsd:string,
        "Fajar Ekaputra"^^xsd:string ;
    sw:term_status "accepted"@en ;
    skos:definition "Information about health history."@en ;
    skos:prefLabel "Health History"@en ;
    skos:scopeNote <https://enterprivacy.com/wp-content/uploads/2018/09/Categories-of-Personal-Information.pdf> ;
    dpv:isSubTypeOf dpv-pd:MedicalHealth .

dpv-pd:Interest a skos:Concept,
        dpv:Concept ;
    dct:created "2019-06-04"^^xsd:date ;
    dct:creator "Elmar Kiesling; Harshvardhan J. Pandit"^^xsd:string,
        "Fajar Ekaputra"^^xsd:string ;
    sw:term_status "accepted"@en ;
    skos:definition "Information about interests"@en ;
    skos:prefLabel "Interest"@en ;
    skos:scopeNote <https://enterprivacy.com/wp-content/uploads/2018/09/Categories-of-Personal-Information.pdf> ;
    dpv:isSubTypeOf dpv-pd:Preference .

dpv-pd:Language a skos:Concept,
        dpv:Concept ;
    dct:created "2019-06-04"^^xsd:date ;
    dct:creator "Elmar Kiesling; Harshvardhan J. Pandit"^^xsd:string,
        "Fajar Ekaputra"^^xsd:string ;
    sw:term_status "accepted"@en ;
    skos:definition "Information about language and lingual history."@en ;
    skos:prefLabel "Language"@en ;
    skos:scopeNote <https://enterprivacy.com/wp-content/uploads/2018/09/Categories-of-Personal-Information.pdf> ;
    dpv:isSubTypeOf dpv-pd:Ethnicity .

dpv-pd:PaymentCard a skos:Concept,
        dpv:Concept ;
    dct:created "2020-11-04"^^xsd:date ;
    dct:creator "Harshvardhan J. Pandit"^^xsd:string ;
    sw:term_status "accepted"@en ;
    skos:definition "Information about payment card such as Credit Card, Debit Card."@en ;
    skos:prefLabel "Payment Card"@en ;
    skos:scopeNote <https://www.w3.org/community/dpvcg/> ;
    dpv:isSubTypeOf dpv-pd:FinancialAccount .

dpv-pd:Authenticating a skos:Concept,
        dpv:Concept ;
    dct:created "2019-06-04"^^xsd:date ;
    dct:creator "Elmar Kiesling; Harshvardhan J. Pandit"^^xsd:string,
        "Fajar Ekaputra"^^xsd:string ;
    sw:term_status "accepted"@en ;
    skos:definition "Information about authentication and information used for authenticating"@en ;
    skos:prefLabel "Authenticating"@en ;
    skos:scopeNote <https://enterprivacy.com/wp-content/uploads/2018/09/Categories-of-Personal-Information.pdf> ;
    dpv:isSubTypeOf dpv-pd:Internal .

dpv-pd:Contact a skos:Concept,
        dpv:Concept ;
    dct:created "2019-06-04"^^xsd:date ;
    dct:creator "Elmar Kiesling; Harshvardhan J. Pandit"^^xsd:string,
        "Fajar Ekaputra"^^xsd:string ;
    sw:term_status "accepted"@en ;
    skos:definition "Information about contacts or used for contacting e.g. email address or phone number"@en ;
    skos:prefLabel "Contact"@en ;
    skos:related svd:Physical ;
    skos:scopeNote <https://enterprivacy.com/wp-content/uploads/2018/09/Categories-of-Personal-Information.pdf> ;
    dpv:isSubTypeOf dpv-pd:Tracking .

dpv-pd:Criminal a skos:Concept,
        dpv:Concept ;
    dct:created "2019-06-04"^^xsd:date ;
    dct:creator "Elmar Kiesling; Harshvardhan J. Pandit"^^xsd:string,
        "Fajar Ekaputra"^^xsd:string ;
    sw:term_status "accepted"@en ;
    skos:definition "Information about criminal activity e.g. criminal convictions or jail time"@en ;
    skos:prefLabel "Criminal"@en ;
    skos:related svd:Judicial ;
    skos:scopeNote <https://enterprivacy.com/wp-content/uploads/2018/09/Categories-of-Personal-Information.pdf> ;
    dpv:isSubTypeOf dpv-pd:Social .

dpv-pd:Demographic a skos:Concept,
        dpv:Concept ;
    dct:created "2019-06-04"^^xsd:date ;
    dct:creator "Elmar Kiesling; Harshvardhan J. Pandit"^^xsd:string,
        "Fajar Ekaputra"^^xsd:string ;
    sw:term_status "accepted"@en ;
    skos:definition "Information about demography and demographic characteristics"@en ;
    skos:prefLabel "Demographic"@en ;
    skos:scopeNote <https://enterprivacy.com/wp-content/uploads/2018/09/Categories-of-Personal-Information.pdf> ;
    dpv:isSubTypeOf dpv-pd:External .

dpv-pd:Ethnicity a skos:Concept,
        dpv:Concept ;
    dct:created "2019-06-04"^^xsd:date ;
    dct:creator "Elmar Kiesling; Harshvardhan J. Pandit"^^xsd:string,
        "Fajar Ekaputra"^^xsd:string ;
    sw:term_status "accepted"@en ;
    skos:definition "Information about ethnic origins and lineage"@en ;
    skos:prefLabel "Ethnicity"@en ;
    skos:scopeNote <https://enterprivacy.com/wp-content/uploads/2018/09/Categories-of-Personal-Information.pdf> ;
    dpv:isSubTypeOf dpv-pd:External .

dpv-pd:Favorite a skos:Concept,
        dpv:Concept ;
    dct:created "2019-06-04"^^xsd:date ;
    dct:creator "Elmar Kiesling; Harshvardhan J. Pandit"^^xsd:string,
        "Fajar Ekaputra"^^xsd:string ;
    sw:term_status "accepted"@en ;
    skos:definition "Information about favorites"@en ;
    skos:prefLabel "Favorite"@en ;
    skos:scopeNote <https://enterprivacy.com/wp-content/uploads/2018/09/Categories-of-Personal-Information.pdf> ;
    dpv:isSubTypeOf dpv-pd:Preference .

dpv-pd:Financial a skos:Concept,
        dpv:Concept ;
    dct:created "2019-06-04"^^xsd:date ;
    dct:creator "Elmar Kiesling; Harshvardhan J. Pandit"^^xsd:string,
        "Fajar Ekaputra"^^xsd:string ;
    sw:term_status "accepted"@en ;
    skos:definition "Information about finance including monetary characteristics and transactions"@en ;
    skos:prefLabel "Financial"@en ;
    skos:related svd:Financial ;
    skos:scopeNote <https://enterprivacy.com/wp-content/uploads/2018/09/Categories-of-Personal-Information.pdf> ;
    dpv:isSubTypeOf dpv:PersonalData .

dpv-pd:FinancialAccount a skos:Concept,
        dpv:Concept ;
    dct:created "2019-06-04"^^xsd:date ;
    dct:creator "Elmar Kiesling; Harshvardhan J. Pandit"^^xsd:string,
        "Fajar Ekaputra"^^xsd:string ;
    sw:term_status "accepted"@en ;
    skos:definition "Information about financial accounts."@en ;
    skos:prefLabel "Financial Account"@en ;
    skos:scopeNote <https://enterprivacy.com/wp-content/uploads/2018/09/Categories-of-Personal-Information.pdf> ;
    dpv:isSubTypeOf dpv-pd:Financial .

dpv-pd:Internal a skos:Concept,
        dpv:Concept ;
    dct:created "2019-06-04"^^xsd:date ;
    dct:creator "Elmar Kiesling; Harshvardhan J. Pandit"^^xsd:string,
        "Fajar Ekaputra"^^xsd:string ;
    sw:term_status "accepted"@en ;
    skos:definition "Informatoin about internal characteristics that cannot be seen or observed"@en ;
    skos:prefLabel "Internal"@en ;
    skos:scopeNote <https://enterprivacy.com/wp-content/uploads/2018/09/Categories-of-Personal-Information.pdf> ;
    dpv:isSubTypeOf dpv:PersonalData .

dpv-pd:KnowledgeBelief a skos:Concept,
        dpv:Concept ;
    dct:created "2019-06-04"^^xsd:date ;
    dct:creator "Elmar Kiesling; Harshvardhan J. Pandit"^^xsd:string,
        "Fajar Ekaputra"^^xsd:string ;
    sw:term_status "accepted"@en ;
    skos:definition "Information about knowledge and beliefs"@en ;
    skos:prefLabel "Knowledge and Beliefs"@en ;
    skos:scopeNote <https://enterprivacy.com/wp-content/uploads/2018/09/Categories-of-Personal-Information.pdf> ;
    dpv:isSubTypeOf dpv-pd:Internal .

dpv-pd:Location a skos:Concept,
        dpv:Concept ;
    dct:created "2019-06-04"^^xsd:date ;
    dct:creator "Elmar Kiesling; Harshvardhan J. Pandit"^^xsd:string,
        "Fajar Ekaputra"^^xsd:string ;
    sw:term_status "accepted"@en ;
    skos:definition "Information about location"@en ;
    skos:prefLabel "Location"@en ;
    skos:related svd:Location ;
    skos:scopeNote <https://enterprivacy.com/wp-content/uploads/2018/09/Categories-of-Personal-Information.pdf> ;
    dpv:isSubTypeOf dpv-pd:Tracking .

dpv-pd:Ownership a skos:Concept,
        dpv:Concept ;
    dct:created "2019-06-04"^^xsd:date ;
    dct:creator "Elmar Kiesling; Harshvardhan J. Pandit"^^xsd:string,
        "Fajar Ekaputra"^^xsd:string ;
    sw:term_status "accepted"@en ;
    skos:definition "Information about ownership and history, including renting, borrowing, possessions."@en ;
    skos:prefLabel "Ownership"@en ;
    skos:scopeNote <https://enterprivacy.com/wp-content/uploads/2018/09/Categories-of-Personal-Information.pdf> ;
    dpv:isSubTypeOf dpv-pd:Financial .

dpv-pd:Tracking a skos:Concept,
        dpv:Concept ;
    dct:created "2019-06-04"^^xsd:date ;
    dct:creator "Elmar Kiesling; Harshvardhan J. Pandit"^^xsd:string,
        "Fajar Ekaputra"^^xsd:string ;
    sw:term_status "accepted"@en ;
    skos:definition "Information used to track an individual or group e.g. location or email"@en ;
    skos:prefLabel "Tracking"@en ;
    skos:scopeNote <https://enterprivacy.com/wp-content/uploads/2018/09/Categories-of-Personal-Information.pdf> ;
    dpv:isSubTypeOf dpv:PersonalData .

dpv-pd:Communication a skos:Concept,
        dpv:Concept ;
    dct:created "2019-06-04"^^xsd:date ;
    dct:creator "Elmar Kiesling; Harshvardhan J. Pandit"^^xsd:string,
        "Fajar Ekaputra"^^xsd:string ;
    sw:term_status "accepted"@en ;
    skos:definition "Information communicated from or to an individual"@en ;
    skos:prefLabel "Communication"@en ;
    skos:scopeNote <https://enterprivacy.com/wp-content/uploads/2018/09/Categories-of-Personal-Information.pdf> ;
    dpv:isSubTypeOf dpv-pd:Social .

dpv-pd:Credit a skos:Concept,
        dpv:Concept ;
    dct:created "2019-06-04"^^xsd:date ;
    dct:creator "Elmar Kiesling; Harshvardhan J. Pandit"^^xsd:string,
        "Fajar Ekaputra"^^xsd:string ;
    sw:term_status "accepted"@en ;
    skos:definition "Information about reputation with regards to money"@en ;
    skos:prefLabel "Credit"@en ;
    skos:scopeNote <https://enterprivacy.com/wp-content/uploads/2018/09/Categories-of-Personal-Information.pdf> ;
    dpv:isSubTypeOf dpv-pd:Transactional .

dpv-pd:DeviceBased a skos:Concept,
        dpv:Concept ;
    dct:created "2019-06-04"^^xsd:date ;
    dct:creator "Elmar Kiesling; Harshvardhan J. Pandit"^^xsd:string,
        "Fajar Ekaputra"^^xsd:string ;
    sw:term_status "accepted"@en ;
    skos:definition "Information about devices"@en ;
    skos:prefLabel "Device Based"@en ;
    skos:related svd:Computer ;
    skos:scopeNote <https://enterprivacy.com/wp-content/uploads/2018/09/Categories-of-Personal-Information.pdf> ;
    dpv:isSubTypeOf dpv-pd:Tracking .

dpv-pd:Sexual a skos:Concept,
        dpv:Concept ;
    dct:created "2019-06-04"^^xsd:date ;
    dct:creator "Elmar Kiesling; Harshvardhan J. Pandit"^^xsd:string,
        "Fajar Ekaputra"^^xsd:string ;
    sw:term_status "accepted"@en ;
    skos:definition "Information about sexuality and sexual history"@en ;
    skos:prefLabel "Sexual"@en ;
    skos:scopeNote <https://enterprivacy.com/wp-content/uploads/2018/09/Categories-of-Personal-Information.pdf> ;
    dpv:isSubTypeOf dpv:SpecialCategoryPersonalData,
        dpv-pd:External .

dpv-pd:FamilyStructure a skos:Concept,
        dpv:Concept ;
    dct:created "2019-06-04"^^xsd:date ;
    dct:creator "Elmar Kiesling; Harshvardhan J. Pandit"^^xsd:string,
        "Fajar Ekaputra"^^xsd:string ;
    sw:term_status "accepted"@en ;
    skos:definition "Information about family and familial structure."@en ;
    skos:prefLabel "Family Structure"@en ;
    skos:scopeNote <https://enterprivacy.com/wp-content/uploads/2018/09/Categories-of-Personal-Information.pdf> ;
    dpv:isSubTypeOf dpv-pd:Family .

dpv-pd:Preference a skos:Concept,
        dpv:Concept ;
    dct:created "2019-06-04"^^xsd:date ;
    dct:creator "Elmar Kiesling; Harshvardhan J. Pandit"^^xsd:string,
        "Fajar Ekaputra"^^xsd:string ;
    sw:term_status "accepted"@en ;
    skos:definition "Information about preferences or interests"@en ;
    skos:prefLabel "Preference"@en ;
    skos:related svd:Preference ;
    skos:scopeNote <https://enterprivacy.com/wp-content/uploads/2018/09/Categories-of-Personal-Information.pdf> ;
    dpv:isSubTypeOf dpv-pd:Internal .

dpv-pd:SocialNetwork a skos:Concept,
        dpv:Concept ;
    dct:created "2019-06-04"^^xsd:date ;
    dct:creator "Elmar Kiesling; Harshvardhan J. Pandit"^^xsd:string,
        "Fajar Ekaputra"^^xsd:string ;
    sw:term_status "accepted"@en ;
    skos:definition "Information about friends or connections expressed as a social network"@en ;
    skos:prefLabel "Social Network"@en ;
    skos:scopeNote <https://enterprivacy.com/wp-content/uploads/2018/09/Categories-of-Personal-Information.pdf> ;
    dpv:isSubTypeOf dpv-pd:Social .

dpv-pd:Identifying a skos:Concept,
        dpv:Concept ;
    dct:created "2019-06-04"^^xsd:date ;
    dct:creator "Elmar Kiesling; Harshvardhan J. Pandit"^^xsd:string,
        "Fajar Ekaputra"^^xsd:string ;
    sw:term_status "accepted"@en ;
    skos:definition "Information that uniquely or semi-uniquely identifies an individual or a group"@en ;
    skos:prefLabel "Identifying"@en ;
    skos:scopeNote <https://enterprivacy.com/wp-content/uploads/2018/09/Categories-of-Personal-Information.pdf> ;
    dpv:isSubTypeOf dpv-pd:External .

dpv-pd:Social a skos:Concept,
        dpv:Concept ;
    dct:created "2019-06-04"^^xsd:date ;
    dct:creator "Elmar Kiesling; Harshvardhan J. Pandit"^^xsd:string,
        "Fajar Ekaputra"^^xsd:string ;
    sw:term_status "accepted"@en ;
    skos:definition "Information about social aspects such as family, public life, or professional networks."@en ;
    skos:prefLabel "Social"@en ;
    skos:scopeNote <https://enterprivacy.com/wp-content/uploads/2018/09/Categories-of-Personal-Information.pdf> ;
    dpv:isSubTypeOf dpv:PersonalData .

dpv-pd:External a skos:Concept,
        dpv:Concept ;
    dct:created "2019-06-04"^^xsd:date ;
    dct:creator "Elmar Kiesling; Harshvardhan J. Pandit"^^xsd:string,
        "Fajar Ekaputra"^^xsd:string ;
    sw:term_status "accepted"@en ;
    skos:definition "Information about external characteristics that can be observed"@en ;
    skos:prefLabel "External"@en ;
    skos:scopeNote <https://enterprivacy.com/wp-content/uploads/2018/09/Categories-of-Personal-Information.pdf> ;
    dpv:isSubTypeOf dpv:PersonalData .

dpv-pd:Behavioral a skos:Concept,
        dpv:Concept ;
    dct:created "2019-06-04"^^xsd:date ;
    dct:creator "Elmar Kiesling; Harshvardhan J. Pandit"^^xsd:string,
        "Fajar Ekaputra"^^xsd:string ;
    sw:term_status "accepted"@en ;
    skos:definition "Information about Behavior or activity"@en ;
    skos:prefLabel "Behavioral"@en ;
    skos:related svd:Activity ;
    skos:scopeNote <https://enterprivacy.com/wp-content/uploads/2018/09/Categories-of-Personal-Information.pdf> ;
    dpv:isSubTypeOf dpv-pd:External .

dpv-pd:MedicalHealth a skos:Concept,
        dpv:Concept ;
    dct:created "2019-06-04"^^xsd:date ;
    dct:creator "Elmar Kiesling; Harshvardhan J. Pandit"^^xsd:string,
        "Fajar Ekaputra"^^xsd:string ;
    sw:term_status "accepted"@en ;
    skos:definition "Information about health, medical conditions or health care"@en ;
    skos:prefLabel "MedicalHealth"@en ;
    skos:scopeNote <https://enterprivacy.com/wp-content/uploads/2018/09/Categories-of-Personal-Information.pdf> ;
    dpv:isSubTypeOf dpv:SpecialCategoryPersonalData,
        dpv-pd:External .

dpv-pd:PhysicalCharacteristic a skos:Concept,
        dpv:Concept ;
    dct:created "2019-06-04"^^xsd:date ;
    dct:creator "Elmar Kiesling; Harshvardhan J. Pandit"^^xsd:string,
        "Fajar Ekaputra"^^xsd:string ;
    sw:term_status "accepted"@en ;
    skos:definition "Information about physical characteristics"@en ;
    skos:prefLabel "PhysicalCharacteristic"@en ;
    skos:related svd:Demographic ;
    skos:scopeNote <https://enterprivacy.com/wp-content/uploads/2018/09/Categories-of-Personal-Information.pdf> ;
    dpv:isSubTypeOf dpv-pd:External .

dpv-pd:PublicLife a skos:Concept,
        dpv:Concept ;
    dct:created "2019-06-04"^^xsd:date ;
    dct:creator "Elmar Kiesling; Harshvardhan J. Pandit"^^xsd:string,
        "Fajar Ekaputra"^^xsd:string ;
    sw:term_status "accepted"@en ;
    skos:definition "Information about public life"@en ;
    skos:prefLabel "Public Life"@en ;
    skos:scopeNote <https://enterprivacy.com/wp-content/uploads/2018/09/Categories-of-Personal-Information.pdf> ;
    dpv:isSubTypeOf dpv-pd:Social .

dpv-pd:Transactional a skos:Concept,
        dpv:Concept ;
    dct:created "2019-06-04"^^xsd:date ;
    dct:creator "Elmar Kiesling; Harshvardhan J. Pandit"^^xsd:string,
        "Fajar Ekaputra"^^xsd:string ;
    sw:term_status "accepted"@en ;
    skos:definition "Information about a purchasing, spending or income"@en ;
    skos:prefLabel "Transactional"@en ;
    skos:scopeNote <https://enterprivacy.com/wp-content/uploads/2018/09/Categories-of-Personal-Information.pdf> ;
    dpv:isSubTypeOf dpv-pd:Financial .

dpv-pd:Professional a skos:Concept,
        dpv:Concept ;
    dct:created "2019-06-04"^^xsd:date ;
    dct:creator "Elmar Kiesling; Harshvardhan J. Pandit"^^xsd:string,
        "Fajar Ekaputra"^^xsd:string ;
    sw:term_status "accepted"@en ;
    skos:definition "Information about educational or professional career"@en ;
    skos:prefLabel "Professional"@en ;
    skos:scopeNote <https://enterprivacy.com/wp-content/uploads/2018/09/Categories-of-Personal-Information.pdf> ;
    dpv:isSubTypeOf dpv-pd:Social .

