@prefix dct: <http://purl.org/dc/terms/> .
@prefix dpv: <http://www.w3.org/ns/dpv#> .
@prefix rdf: <http://www.w3.org/1999/02/22-rdf-syntax-ns#> .
@prefix rdfs: <http://www.w3.org/2000/01/rdf-schema#> .
@prefix svpu: <http://www.specialprivacy.eu/vocabs/purposes#> .
@prefix sw: <http://www.w3.org/2003/06/sw-vocab-status/ns#> .
@prefix xsd: <http://www.w3.org/2001/XMLSchema#> .

dpv:AcademicResearch a rdfs:Class ;
    rdfs:label "Academic Research"@en ;
    dct:created "2019-04-05"^^xsd:date ;
    dct:creator "Axel Polleres"^^xsd:string,
        "Elmar Kiesling"^^xsd:string,
        "Fajar Ekaputra"^^xsd:string,
        "Harshvardhan J. Pandit"^^xsd:string,
        "Javier Fernandez"^^xsd:string,
        "Simon Steyskal"^^xsd:string ;
    dct:description "conduct or assist with research conducted in an academic context e.g. within universities"@en ;
    rdfs:seeAlso svpu:Education ;
    rdfs:subClassOf dpv:ResearchAndDevelopment ;
    sw:term_status "accepted"@en .

dpv:AccountManagement a rdfs:Class ;
    rdfs:label "Account Management"@en ;
    dct:created "2021-08-18"^^xsd:date ;
    dct:description "to create, maintain, and manage accounts for purposes of providing services"@en ;
    rdfs:subClassOf dpv:Purpose ;
    sw:term_status "proposed"@en .

dpv:Advertising a rdfs:Class ;
    rdfs:label "Advertising"@en ;
    dct:created "2020-11-04"^^xsd:date ;
    dct:creator "Beatriz Esteves"^^xsd:string,
        "Georg P Krog"^^xsd:string,
        "Harshvardhan J. Pandit"^^xsd:string ;
    dct:description "carry out advertising i.e. process or artefact used to call attention to a product, service, etc. through announcements, notices, or other forms of communication."@en ;
    rdfs:comment "Advertising is a subset of Marketing. Advertising by itself does not indicate 'personalisation' i.e. personalised ads."@en ;
    rdfs:subClassOf dpv:Marketing ;
    sw:term_status "accepted"@en .

dpv:Beneficiary a rdfs:Class ;
    rdfs:label "Beneficiary"@en ;
    dct:created "2019-04-05"^^xsd:date ;
    dct:creator "Axel Polleres"^^xsd:string ;
    dct:description "Indicates who is the beneficiary in context of purpose and its benefit"@en ;
    rdfs:comment "This needs further details, the group is asking feedback about whether Beneficiaries of a specific purposes hould be specified separately or not. self.DataSubject, self.DataController, society ? ( --- under consideration ---)"@en ;
    sw:term_status "proposed"@en .

dpv:Benefit a rdfs:Class ;
    rdfs:label "Benefit"@en ;
    dct:created "2021-01-06"^^xsd:date ;
    dct:description "The benefits obtained or derived or provided from a purpose."@en ;
    sw:term_status "proposed"@en .

dpv:CommercialResearch a rdfs:Class ;
    rdfs:label "Commercial Research"@en ;
    dct:created "2019-04-05"^^xsd:date ;
    dct:creator "Axel Polleres"^^xsd:string,
        "Elmar Kiesling"^^xsd:string,
        "Fajar Ekaputra"^^xsd:string,
        "Harshvardhan J. Pandit"^^xsd:string,
        "Javier Fernandez"^^xsd:string,
        "Simon Steyskal"^^xsd:string ;
    dct:description "conduct research in a commercial setting e.g. in a company"@en ;
    rdfs:seeAlso svpu:Develop ;
    rdfs:subClassOf dpv:ResearchAndDevelopment ;
    sw:term_status "accepted"@en .

dpv:Communication a rdfs:Class ;
    rdfs:label "Communication"@en ;
    dct:created "2021-08-18"^^xsd:date ;
    dct:description "to communicate or provide means for communication"@en ;
    rdfs:subClassOf dpv:Purpose ;
    sw:term_status "proposed"@en .

dpv:CommunicationForCustomerCare a rdfs:Class ;
    rdfs:label "Communication for Customer Care"@en ;
    dct:created "2020-11-04"^^xsd:date ;
    dct:creator "Beatriz Esteves"^^xsd:string,
        "Georg P Krog"^^xsd:string,
        "Harshvardhan J. Pandit"^^xsd:string ;
    dct:description "communicate with users via email, phone, sms, chat or push messages regarding your requests."@en ;
    rdfs:subClassOf dpv:CustomerCare ;
    sw:term_status "accepted"@en .

dpv:Context a rdfs:Class ;
    rdfs:label "Context"@en ;
    dct:created "2019-04-05"^^xsd:date ;
    dct:creator "Axel Polleres"^^xsd:string,
        "Elmar Kiesling"^^xsd:string,
        "Fajar Ekaputra"^^xsd:string,
        "Harshvardhan J. Pandit"^^xsd:string,
        "Javier Fernandez"^^xsd:string,
        "Simon Steyskal"^^xsd:string ;
    dct:description "The 'context' or 'scope' of the purpose, e.g. restriction to a certain business sector"@en ;
    sw:term_status "accepted"@en .

dpv:CreateEventRecommendations a rdfs:Class ;
    rdfs:label "Create Event Recommendations"@en ;
    dct:created "2019-11-26"^^xsd:date ;
    dct:creator "Harshvardhan J. Pandit"^^xsd:string,
        "Rudy Jacob"^^xsd:string ;
    dct:description "create and provide personalised recommendations for events"@en ;
    rdfs:isDefinedBy <https://www.specialprivacy.eu/> ;
    rdfs:subClassOf dpv:CreatePersonalizedRecommendations ;
    sw:term_status "accepted"@en .

dpv:CreatePersonalizedRecommendations a rdfs:Class ;
    rdfs:label "Create Personalized Recommendations"@en ;
    dct:created "2019-11-26"^^xsd:date ;
    dct:creator "Harshvardhan J. Pandit"^^xsd:string,
        "Rudy Jacob"^^xsd:string ;
    dct:description "create and provide personalised recommendations"@en ;
    rdfs:isDefinedBy <https://www.specialprivacy.eu/> ;
    rdfs:subClassOf dpv:ServicePersonalization ;
    sw:term_status "accepted"@en .

dpv:CreateProductRecommendations a rdfs:Class ;
    rdfs:label "Create Product Recommendations"@en ;
    dct:created "2019-04-05"^^xsd:date ;
    dct:creator "Axel Polleres"^^xsd:string,
        "Elmar Kiesling"^^xsd:string,
        "Fajar Ekaputra"^^xsd:string,
        "Harshvardhan J. Pandit"^^xsd:string,
        "Javier Fernandez"^^xsd:string,
        "Simon Steyskal"^^xsd:string ;
    dct:description "create and provide product recommendations e.g. suggest similar products"@en ;
    rdfs:seeAlso svpu:Marketing ;
    rdfs:subClassOf dpv:CreatePersonalizedRecommendations ;
    sw:term_status "accepted"@en .

dpv:CustomerCare a rdfs:Class ;
    rdfs:label "Customer Care"@en ;
    dct:created "2019-04-05"^^xsd:date ;
    dct:creator "Axel Polleres"^^xsd:string,
        "Elmar Kiesling"^^xsd:string,
        "Fajar Ekaputra"^^xsd:string,
        "Harshvardhan J. Pandit"^^xsd:string,
        "Javier Fernandez"^^xsd:string,
        "Simon Steyskal"^^xsd:string ;
    dct:description "provide assistance for customer complaints and satisfaction"@en ;
    rdfs:seeAlso svpu:Feedback ;
    rdfs:subClassOf dpv:CustomerManagement ;
    sw:term_status "proposed"@en .

dpv:CustomerManagement a rdfs:Class ;
    rdfs:label "Customer Management"@en ;
    dct:created "2021-08-18"^^xsd:date ;
    dct:description "Management of past, current, and future customers"@en ;
    rdfs:subClassOf dpv:Purpose ;
    sw:term_status "proposed"@en .

dpv:CustomerRelationshipManagement a rdfs:Class ;
    rdfs:label "Customer Relationship Management"@en ;
    dct:created "2021-08-18"^^xsd:date ;
    dct:creator "Beatriz"^^xsd:string,
        "Georg P Krog"^^xsd:string,
        "Harshvardhan J. Pandit"^^xsd:string ;
    dct:description "Process by which a company can manage and analyse its own interactions with its past, current and potential customers"@en ;
    rdfs:subClassOf dpv:CustomerManagement ;
    sw:term_status "proposed"@en .

dpv:DeliveryOfGoods a rdfs:Class ;
    rdfs:label "Delivery of Goods"@en ;
    dct:created "2019-04-05"^^xsd:date ;
    dct:creator "Axel Polleres"^^xsd:string,
        "Elmar Kiesling"^^xsd:string,
        "Fajar Ekaputra"^^xsd:string,
        "Harshvardhan J. Pandit"^^xsd:string,
        "Javier Fernandez"^^xsd:string,
        "Simon Steyskal"^^xsd:string ;
    dct:description "deliver goods and services"@en ;
    rdfs:seeAlso svpu:Delivery ;
    rdfs:subClassOf dpv:RequestedServiceProvision ;
    sw:term_status "proposed"@en .

dpv:DirectMarketing a rdfs:Class ;
    rdfs:label "Direct Marketing"@en ;
    dct:created "2020-11-04"^^xsd:date ;
    dct:creator "Beatriz Esteves"^^xsd:string,
        "Georg P Krog"^^xsd:string,
        "Harshvardhan J. Pandit"^^xsd:string ;
    dct:description "carry out direct marketing i.e. marketing communicated directly to the individual"@en ;
    rdfs:subClassOf dpv:Marketing ;
    sw:term_status "accepted"@en .

dpv:EnforceAccessControl a rdfs:Class ;
    rdfs:label "Enforce Access Control"@en ;
    dct:created "2019-04-05"^^xsd:date ;
    dct:creator "Axel Polleres"^^xsd:string,
        "Elmar Kiesling"^^xsd:string,
        "Fajar Ekaputra"^^xsd:string,
        "Harshvardhan J. Pandit"^^xsd:string,
        "Javier Fernandez"^^xsd:string,
        "Simon Steyskal"^^xsd:string ;
    dct:description "conduct or enforce access control"@en ;
    rdfs:comment "Was previously \"Access Control\". Prefixed to distinguish from Technical Measure."@en ;
    rdfs:seeAlso svpu:Login ;
    rdfs:subClassOf dpv:Security ;
    sw:term_status "proposed"@en .

dpv:FraudPreventionAndDetection a rdfs:Class ;
    rdfs:label "Fraud Prevention and Detection"@en ;
    dct:created "2019-04-05"^^xsd:date ;
    dct:creator "Axel Polleres"^^xsd:string,
        "Elmar Kiesling"^^xsd:string,
        "Fajar Ekaputra"^^xsd:string,
        "Harshvardhan J. Pandit"^^xsd:string,
        "Javier Fernandez"^^xsd:string,
        "Simon Steyskal"^^xsd:string ;
    dct:description "detect and prevent fraud"@en ;
    rdfs:seeAlso svpu:Government ;
    rdfs:subClassOf dpv:Security ;
    sw:term_status "accepted"@en .

dpv:IdentityVerification a rdfs:Class ;
    rdfs:label "Identity Verification"@en ;
    dct:created "2019-04-05"^^xsd:date ;
    dct:creator "Axel Polleres"^^xsd:string,
        "Elmar Kiesling"^^xsd:string,
        "Fajar Ekaputra"^^xsd:string,
        "Harshvardhan J. Pandit"^^xsd:string,
        "Javier Fernandez"^^xsd:string,
        "Simon Steyskal"^^xsd:string ;
    dct:description "verify and authorise identity"@en ;
    rdfs:subClassOf dpv:Security ;
    sw:term_status "accepted"@en .

dpv:ImproveExistingProductsAndServices a rdfs:Class ;
    rdfs:label "Improve Existing Products and Services"@en ;
    dct:created "2019-04-05"^^xsd:date ;
    dct:creator "Axel Polleres"^^xsd:string,
        "Elmar Kiesling"^^xsd:string,
        "Fajar Ekaputra"^^xsd:string,
        "Harshvardhan J. Pandit"^^xsd:string,
        "Javier Fernandez"^^xsd:string,
        "Simon Steyskal"^^xsd:string ;
    dct:description "improve existing products and services"@en ;
    rdfs:subClassOf dpv:OptimisationForController ;
    sw:term_status "accepted"@en .

dpv:ImproveInternalCRMProcesses a rdfs:Class ;
    rdfs:label "Improve Internal CRM Processes"@en ;
    dct:created "2019-04-05"^^xsd:date ;
    dct:creator "Axel Polleres"^^xsd:string,
        "Elmar Kiesling"^^xsd:string,
        "Fajar Ekaputra"^^xsd:string,
        "Harshvardhan J. Pandit"^^xsd:string,
        "Javier Fernandez"^^xsd:string,
        "Simon Steyskal"^^xsd:string ;
    dct:description "improve customer-relationship management (CRM) processes"@en ;
    rdfs:subClassOf dpv:CustomerRelationshipManagement,
        dpv:OptimisationForController ;
    sw:term_status "accepted"@en .

dpv:IncreaseServiceRobustness a rdfs:Class ;
    rdfs:label "Increase Service Robustness"@en ;
    dct:created "2019-04-05"^^xsd:date ;
    dct:creator "Axel Polleres"^^xsd:string,
        "Elmar Kiesling"^^xsd:string,
        "Fajar Ekaputra"^^xsd:string,
        "Harshvardhan J. Pandit"^^xsd:string,
        "Javier Fernandez"^^xsd:string,
        "Simon Steyskal"^^xsd:string ;
    dct:description "improve the robustness and resilience of services"@en ;
    rdfs:subClassOf dpv:OptimisationForController ;
    sw:term_status "accepted"@en .

dpv:InternalResourceOptimisation a rdfs:Class ;
    rdfs:label "Internal Resource Optimisation"@en ;
    dct:created "2019-04-05"^^xsd:date ;
    dct:creator "Axel Polleres"^^xsd:string,
        "Elmar Kiesling"^^xsd:string,
        "Fajar Ekaputra"^^xsd:string,
        "Harshvardhan J. Pandit"^^xsd:string,
        "Javier Fernandez"^^xsd:string,
        "Simon Steyskal"^^xsd:string ;
    dct:description "optimise internal resources used by the organisation e.g. resource usage"@en ;
    rdfs:subClassOf dpv:OptimisationForController ;
    sw:term_status "accepted"@en .

dpv:LegalCompliance a rdfs:Class ;
    rdfs:label "Legal Compliance"@en ;
    dct:created "2020-11-04"^^xsd:date ;
    dct:creator "Beatriz Esteves"^^xsd:string,
        "Georg P Krog"^^xsd:string,
        "Harshvardhan J. Pandit"^^xsd:string ;
    dct:description "fulfill obligations or requirements towards achieving compliance with law or regulations."@en ;
    rdfs:subClassOf dpv:Purpose ;
    sw:term_status "accepted"@en .

dpv:Marketing a rdfs:Class ;
    rdfs:label "Marketing"@en ;
    dct:created "2020-11-04"^^xsd:date ;
    dct:creator "Beatriz Esteves"^^xsd:string,
        "Georg P Krog"^^xsd:string,
        "Harshvardhan J. Pandit"^^xsd:string ;
    dct:description "carry out marketing i.e. promoting, selling, and distributing a product or service"@en ;
    rdfs:comment "Was commercial interest, changed to consider Marketing a separate Purpose category by itself."@en ;
    rdfs:subClassOf dpv:Purpose ;
    sw:term_status "proposed"@en .

dpv:NonCommercialResearch a rdfs:Class ;
    rdfs:label "Non-Commercial Research"@en ;
    dct:created "2019-04-05"^^xsd:date ;
    dct:creator "Axel Polleres"^^xsd:string,
        "Elmar Kiesling"^^xsd:string,
        "Fajar Ekaputra"^^xsd:string,
        "Harshvardhan J. Pandit"^^xsd:string,
        "Javier Fernandez"^^xsd:string,
        "Simon Steyskal"^^xsd:string ;
    dct:description "conduct research in a non-commercial setting e.g. for a non-profit-organisation (NGO)"@en ;
    rdfs:subClassOf dpv:ResearchAndDevelopment ;
    sw:term_status "accepted"@en .

dpv:OptimisationForConsumer a rdfs:Class ;
    rdfs:label "Optimisation for Consumer"@en ;
    dct:created "2019-04-05"^^xsd:date ;
    dct:creator "Axel Polleres"^^xsd:string,
        "Elmar Kiesling"^^xsd:string,
        "Fajar Ekaputra"^^xsd:string,
        "Harshvardhan J. Pandit"^^xsd:string,
        "Javier Fernandez"^^xsd:string,
        "Simon Steyskal"^^xsd:string ;
    dct:description "optimise activities and services for the consumer or user"@en ;
    rdfs:seeAlso svpu:Custom ;
    rdfs:subClassOf dpv:ServiceOptimization ;
    sw:term_status "accepted"@en .

dpv:OptimisationForController a rdfs:Class ;
    rdfs:label "Optimisation for Controller"@en ;
    dct:created "2019-04-05"^^xsd:date ;
    dct:creator "Axel Polleres"^^xsd:string,
        "Elmar Kiesling"^^xsd:string,
        "Fajar Ekaputra"^^xsd:string,
        "Harshvardhan J. Pandit"^^xsd:string,
        "Javier Fernandez"^^xsd:string,
        "Simon Steyskal"^^xsd:string ;
    dct:description "optimise activities and services for the Controller"@en ;
    rdfs:subClassOf dpv:ServiceOptimization ;
    sw:term_status "accepted"@en .

dpv:OptimiseUserInterface a rdfs:Class ;
    rdfs:label "Optimise User Interface"@en ;
    dct:created "2019-04-05"^^xsd:date ;
    dct:creator "Axel Polleres"^^xsd:string,
        "Elmar Kiesling"^^xsd:string,
        "Fajar Ekaputra"^^xsd:string,
        "Harshvardhan J. Pandit"^^xsd:string,
        "Javier Fernandez"^^xsd:string,
        "Simon Steyskal"^^xsd:string ;
    dct:description "optimise interfaces presented to the user"@en ;
    rdfs:subClassOf dpv:OptimisationForConsumer ;
    sw:term_status "accepted"@en .

dpv:Payment a rdfs:Class ;
    rdfs:label "Payment"@en ;
    dct:created "2020-11-04"^^xsd:date ;
    dct:creator "Beatriz Esteves"^^xsd:string,
        "Georg P Krog"^^xsd:string,
        "Harshvardhan J. Pandit"^^xsd:string ;
    dct:description "process usersâ€™ payment transactions."@en ;
    rdfs:subClassOf dpv:ServiceProvision ;
    sw:term_status "accepted"@en .

dpv:PersonalisedAdvertising a rdfs:Class ;
    rdfs:label "Personalised Advertising"@en ;
    dct:created "2020-11-04"^^xsd:date ;
    dct:creator "Beatriz Esteves"^^xsd:string,
        "Georg P Krog"^^xsd:string,
        "Harshvardhan J. Pandit"^^xsd:string ;
    dct:description "provide personalised advertising"@en ;
    rdfs:subClassOf dpv:Advertising ;
    sw:term_status "proposed"@en .

dpv:PersonalisedBenefits a rdfs:Class ;
    rdfs:label "Personalised Benefits"@en ;
    dct:created "2019-04-05"^^xsd:date ;
    dct:creator "Axel Polleres"^^xsd:string,
        "Elmar Kiesling"^^xsd:string,
        "Fajar Ekaputra"^^xsd:string,
        "Harshvardhan J. Pandit"^^xsd:string,
        "Javier Fernandez"^^xsd:string,
        "Simon Steyskal"^^xsd:string ;
    dct:description "personalise benefits received by the user"@en ;
    rdfs:subClassOf dpv:ServicePersonalization ;
    sw:term_status "accepted"@en .

dpv:RecordManagement a rdfs:Class ;
    rdfs:label "Record Management"@en ;
    dct:created "2021-08-18"^^xsd:date ;
    dct:description "to record or manage records of operations, events, and processes"@en ;
    rdfs:subClassOf dpv:Purpose ;
    sw:term_status "proposed"@en .

dpv:RegistrationAuthentication a rdfs:Class ;
    rdfs:label "Registration and Authentication"@en ;
    dct:created "2020-11-04"^^xsd:date ;
    dct:creator "Beatriz Esteves"^^xsd:string,
        "Georg P Krog"^^xsd:string,
        "Harshvardhan J. Pandit"^^xsd:string ;
    dct:description "register, authenticate, and identify in context of a service."@en ;
    rdfs:subClassOf dpv:ServiceProvision ;
    sw:term_status "accepted"@en .

dpv:RequestedServiceProvision a rdfs:Class ;
    rdfs:label "Requested Service Provision"@en ;
    dct:created ""^^xsd:date ;
    dct:description "to deliver service as requested by the user or consumer."@en ;
    rdfs:subClassOf dpv:ServiceProvision ;
    sw:term_status "proposed"@en .

dpv:ResearchAndDevelopment a rdfs:Class ;
    rdfs:label "Research and Development"@en ;
    dct:created "2019-04-05"^^xsd:date ;
    dct:creator "Axel Polleres"^^xsd:string,
        "Elmar Kiesling"^^xsd:string,
        "Fajar Ekaputra"^^xsd:string,
        "Harshvardhan J. Pandit"^^xsd:string,
        "Javier Fernandez"^^xsd:string,
        "Simon Steyskal"^^xsd:string ;
    dct:description "conduct research and development for new methods, products, or services"@en ;
    rdfs:subClassOf dpv:Purpose ;
    sw:term_status "accepted"@en .

dpv:Sector a rdfs:Class ;
    rdfs:label "Sector"@en ;
    dct:created "2019-04-05"^^xsd:date ;
    dct:creator "Axel Polleres"^^xsd:string,
        "Elmar Kiesling"^^xsd:string,
        "Fajar Ekaputra"^^xsd:string,
        "Harshvardhan J. Pandit"^^xsd:string,
        "Javier Fernandez"^^xsd:string,
        "Simon Steyskal"^^xsd:string ;
    dct:description "The 'sector' or 'domain' of a purpose e.g. Agriculture, Advertising"@en ;
    rdfs:comment "There are various sector codes used commonly to indicate the domain of an organisation or business. Examples include NACE (EU), ISIC (UN), SIC and NAICS (USA)."@en ;
    sw:term_status "accepted"@en .

dpv:Security a rdfs:Class ;
    rdfs:label "Security"@en ;
    dct:created "2019-04-05"^^xsd:date ;
    dct:creator "Axel Polleres"^^xsd:string,
        "Elmar Kiesling"^^xsd:string,
        "Fajar Ekaputra"^^xsd:string,
        "Harshvardhan J. Pandit"^^xsd:string,
        "Javier Fernandez"^^xsd:string,
        "Simon Steyskal"^^xsd:string ;
    dct:description "ensure and enforce security e.g. of data"@en ;
    rdfs:subClassOf dpv:Purpose ;
    sw:term_status "accepted"@en .

dpv:SellDataToThirdParties a rdfs:Class ;
    rdfs:label "Sell Data to Third Parties"@en ;
    dct:created "2019-04-05"^^xsd:date ;
    dct:creator "Axel Polleres"^^xsd:string,
        "Elmar Kiesling"^^xsd:string,
        "Fajar Ekaputra"^^xsd:string,
        "Harshvardhan J. Pandit"^^xsd:string,
        "Javier Fernandez"^^xsd:string,
        "Simon Steyskal"^^xsd:string ;
    dct:description "sell data or information to third parties"@en ;
    rdfs:comment "Was subclass of commercial interest, changed to reflect selling something"@en ;
    rdfs:subClassOf dpv:SellProducts ;
    sw:term_status "proposed"@en .

dpv:SellInsightsFromData a rdfs:Class ;
    rdfs:label "Sell Insights from Data"@en ;
    dct:created "2019-04-05"^^xsd:date ;
    dct:creator "Axel Polleres"^^xsd:string,
        "Elmar Kiesling"^^xsd:string,
        "Fajar Ekaputra"^^xsd:string,
        "Harshvardhan J. Pandit"^^xsd:string,
        "Javier Fernandez"^^xsd:string,
        "Simon Steyskal"^^xsd:string ;
    dct:description "sell or commercially provide insights obtained from analysis of data"@en ;
    rdfs:comment "Was subclass of commercial interest, changed to reflect selling something"@en ;
    rdfs:subClassOf dpv:SellProducts ;
    sw:term_status "proposed"@en .

dpv:SellProducts a rdfs:Class ;
    rdfs:label "Sell Products"@en ;
    dct:created ""^^xsd:date ;
    dct:description "Sell products or services"@en ;
    rdfs:comment "Was commercial interest, changed to reflect selling something"@en ;
    rdfs:subClassOf dpv:ServiceProvision ;
    sw:term_status "proposed"@en .

dpv:SellProductsToDataSubject a rdfs:Class ;
    rdfs:label "Sell Products to Data Subject"@en ;
    dct:created "2019-04-05"^^xsd:date ;
    dct:creator "Axel Polleres"^^xsd:string,
        "Elmar Kiesling"^^xsd:string,
        "Fajar Ekaputra"^^xsd:string,
        "Harshvardhan J. Pandit"^^xsd:string,
        "Javier Fernandez"^^xsd:string,
        "Simon Steyskal"^^xsd:string ;
    dct:description "sell products or services"@en ;
    rdfs:comment "Was subclass of commercial interest, changed to reflect selling something"@en ;
    rdfs:subClassOf dpv:SellProducts ;
    sw:term_status "proposed"@en .

dpv:ServiceOptimization a rdfs:Class ;
    rdfs:label "Service Optimization"@en ;
    dct:created "2019-04-05"^^xsd:date ;
    dct:creator "Axel Polleres"^^xsd:string,
        "Elmar Kiesling"^^xsd:string,
        "Fajar Ekaputra"^^xsd:string,
        "Harshvardhan J. Pandit"^^xsd:string,
        "Javier Fernandez"^^xsd:string,
        "Simon Steyskal"^^xsd:string ;
    dct:description "optimise service or activity"@en ;
    rdfs:comment "Subclass of ServiceProvision since optimisation is usually considered part of providing services"@en ;
    rdfs:subClassOf dpv:ServiceProvision ;
    sw:term_status "proposed"@en .

dpv:ServicePersonalization a rdfs:Class ;
    rdfs:label "Service Personalization"@en ;
    dct:created "2019-04-05"^^xsd:date ;
    dct:creator "Axel Polleres"^^xsd:string,
        "Elmar Kiesling"^^xsd:string,
        "Fajar Ekaputra"^^xsd:string,
        "Harshvardhan J. Pandit"^^xsd:string,
        "Javier Fernandez"^^xsd:string,
        "Simon Steyskal"^^xsd:string ;
    dct:description "personalise service or activity"@en ;
    rdfs:comment "Subclass of ServiceProvision since personalisation is usually considered part of providing services"@en ;
    rdfs:subClassOf dpv:ServiceProvision ;
    sw:term_status "proposed"@en .

dpv:ServiceProvision a rdfs:Class ;
    rdfs:label "Service Provision"@en ;
    dct:created "2019-04-05"^^xsd:date ;
    dct:creator "Axel Polleres"^^xsd:string,
        "Elmar Kiesling"^^xsd:string,
        "Fajar Ekaputra"^^xsd:string,
        "Harshvardhan J. Pandit"^^xsd:string,
        "Javier Fernandez"^^xsd:string,
        "Simon Steyskal"^^xsd:string ;
    dct:description "provide service or activity"@en ;
    rdfs:subClassOf dpv:Purpose ;
    sw:term_status "accepted"@en .

dpv:ServiceRecordManagement a rdfs:Class ;
    rdfs:label "Service Order Management"@en ;
    dct:created ""^^xsd:date ;
    dct:description "management of invoicing, orders, and records for service"@en ;
    rdfs:subClassOf dpv:ServiceProvision ;
    sw:term_status "proposed"@en .

dpv:ServiceUsageAnalytics a rdfs:Class ;
    rdfs:label "Analytics"@en ;
    dct:created "2020-11-04"^^xsd:date ;
    dct:creator "Beatriz Esteves"^^xsd:string,
        "Georg P Krog"^^xsd:string,
        "Harshvardhan J. Pandit"^^xsd:string ;
    dct:description "calculate, analyse, and report usage of service or product."@en ;
    rdfs:comment "Was \"UsageAnalytics\", prefixed with Service to better reflect scope"@en ;
    rdfs:subClassOf dpv:ServiceProvision ;
    sw:term_status "proposed"@en .

dpv:SocialMediaMarketing a rdfs:Class ;
    rdfs:label "Social Media"@en ;
    dct:created "2020-11-04"^^xsd:date ;
    dct:creator "Beatriz Esteves"^^xsd:string,
        "Georg P Krog"^^xsd:string,
        "Harshvardhan J. Pandit"^^xsd:string ;
    dct:description "market through and on social media."@en ;
    rdfs:subClassOf dpv:Marketing ;
    sw:term_status "accepted"@en .

dpv:TechnicalServiceProvision a rdfs:Class ;
    rdfs:label "Technical Service Provision"@en ;
    dct:created ""^^xsd:date ;
    dct:description "technical processes necessary for delivering service"@en ;
    rdfs:subClassOf dpv:ServiceProvision ;
    sw:term_status "proposed"@en .

dpv:UserInterfacePersonalisation a rdfs:Class ;
    rdfs:label "User Interface Personalisation"@en ;
    dct:created "2019-04-05"^^xsd:date ;
    dct:creator "Axel Polleres"^^xsd:string,
        "Elmar Kiesling"^^xsd:string,
        "Fajar Ekaputra"^^xsd:string,
        "Harshvardhan J. Pandit"^^xsd:string,
        "Javier Fernandez"^^xsd:string,
        "Simon Steyskal"^^xsd:string ;
    dct:description "personalise interfaces presented to the user"@en ;
    rdfs:subClassOf dpv:ServicePersonalization ;
    sw:term_status "accepted"@en .

dpv:hasContext a rdf:Property ;
    rdfs:label "has context"@en ;
    dct:created "2019-04-05"^^xsd:date ;
    dct:description "Indicates a purpose is restricted to the specified context(s)"@en ;
    rdfs:domain dpv:Purpose ;
    rdfs:range dpv:Context ;
    sw:term_status "accepted"@en .

dpv:hasSector a rdf:Property ;
    rdfs:label "has sector"@en ;
    dct:created "2019-04-05"^^xsd:date ;
    dct:description "Indicates the purpose is associated with activities in the indicated (Economic) Sector(s)"@en ;
    rdfs:domain dpv:Context ;
    rdfs:range dpv:Sector ;
    sw:term_status "accepted"@en .

